<?xml version="1.0"?>
<rdf:RDF xmlns="http://www.semanticweb.org/afshar87/ontologies/2024/3/Laser-Plasma_ontology/"
     xml:base="http://www.semanticweb.org/afshar87/ontologies/2024/3/Laser-Plasma_ontology/"
     xmlns:owl="http://www.w3.org/2002/07/owl#"
     xmlns:rdf="http://www.w3.org/1999/02/22-rdf-syntax-ns#"
     xmlns:xml="http://www.w3.org/XML/1998/namespace"
     xmlns:xsd="http://www.w3.org/2001/XMLSchema#"
     xmlns:rdfs="http://www.w3.org/2000/01/rdf-schema#"
     xmlns:Laser-Plasma_ontology="http://www.semanticweb.org/afshar87/ontologies/2024/3/Laser-Plasma_ontology#">
    <owl:Ontology rdf:about="http://www.semanticweb.org/afshar87/ontologies/2024/3/Laser-Plasma_ontology">
        <rdfs:comment>This is an Ontology for Laser-Plasma and its Applications.</rdfs:comment>
    </owl:Ontology>
    


    <!-- 
    ///////////////////////////////////////////////////////////////////////////////////////
    //
    // Datatypes
    //
    ///////////////////////////////////////////////////////////////////////////////////////
     -->

    


    <!-- http://www.semanticweb.org/afshar87/ontologies/2024/3/Laser-Plasma_ontology#BoundaryConditionType -->

    <rdfs:Datatype rdf:about="http://www.semanticweb.org/afshar87/ontologies/2024/3/Laser-Plasma_ontology#BoundaryConditionType"/>
    


    <!-- 
    ///////////////////////////////////////////////////////////////////////////////////////
    //
    // Object Properties
    //
    ///////////////////////////////////////////////////////////////////////////////////////
     -->

    


    <!-- http://www.semanticweb.org/afshar87/ontologies/2024/3/Laser-Plasma_ontology#Laser-Driven_Shocks_creates_WDM_HEDP -->

    <owl:ObjectProperty rdf:about="http://www.semanticweb.org/afshar87/ontologies/2024/3/Laser-Plasma_ontology#Laser-Driven_Shocks_creates_WDM_HEDP">
        <rdfs:subPropertyOf rdf:resource="http://www.semanticweb.org/afshar87/ontologies/2024/3/Laser-Plasma_ontology#WDM"/>
        <rdfs:domain rdf:resource="http://www.semanticweb.org/afshar87/ontologies/2024/3/Laser-Plasma_ontology#Laser-Driven_Shocks"/>
        <rdfs:range rdf:resource="http://www.semanticweb.org/afshar87/ontologies/2024/3/Laser-Plasma_ontology#High_Energy_Density_Physics_(HEDP)"/>
        <rdfs:range rdf:resource="http://www.semanticweb.org/afshar87/ontologies/2024/3/Laser-Plasma_ontology#Warm_Dense_Matter_(WDM)"/>
        <rdfs:comment>Laser-Driven Shocks creates WDM</rdfs:comment>
    </owl:ObjectProperty>
    


    <!-- http://www.semanticweb.org/afshar87/ontologies/2024/3/Laser-Plasma_ontology#Laser_Ablation_creates_WDM_HEDP -->

    <owl:ObjectProperty rdf:about="http://www.semanticweb.org/afshar87/ontologies/2024/3/Laser-Plasma_ontology#Laser_Ablation_creates_WDM_HEDP">
        <rdfs:subPropertyOf rdf:resource="http://www.semanticweb.org/afshar87/ontologies/2024/3/Laser-Plasma_ontology#WDM"/>
        <rdfs:domain rdf:resource="http://www.semanticweb.org/afshar87/ontologies/2024/3/Laser-Plasma_ontology#Laser_Ablation"/>
        <rdfs:range rdf:resource="http://www.semanticweb.org/afshar87/ontologies/2024/3/Laser-Plasma_ontology#High_Energy_Density_Physics_(HEDP)"/>
        <rdfs:range rdf:resource="http://www.semanticweb.org/afshar87/ontologies/2024/3/Laser-Plasma_ontology#Warm_Dense_Matter_(WDM)"/>
        <rdfs:comment>Laser Ablation creates WDM  states
.</rdfs:comment>
    </owl:ObjectProperty>
    


    <!-- http://www.semanticweb.org/afshar87/ontologies/2024/3/Laser-Plasma_ontology#Particle_diagnostics_for_measuring_Laser_Matter_Interaction -->

    <owl:ObjectProperty rdf:about="http://www.semanticweb.org/afshar87/ontologies/2024/3/Laser-Plasma_ontology#Particle_diagnostics_for_measuring_Laser_Matter_Interaction">
        <rdfs:domain rdf:resource="http://www.semanticweb.org/afshar87/ontologies/2024/3/Laser-Plasma_ontology#Particle_Beam_Generation"/>
        <rdfs:range rdf:resource="http://www.semanticweb.org/afshar87/ontologies/2024/3/Laser-Plasma_ontology#Laser_Plasma_Application"/>
        <rdfs:comment>Particle diagnostics for measuring particle energies and distributions.</rdfs:comment>
    </owl:ObjectProperty>
    


    <!-- http://www.semanticweb.org/afshar87/ontologies/2024/3/Laser-Plasma_ontology#Simulation -->

    <owl:ObjectProperty rdf:about="http://www.semanticweb.org/afshar87/ontologies/2024/3/Laser-Plasma_ontology#Simulation"/>
    


    <!-- http://www.semanticweb.org/afshar87/ontologies/2024/3/Laser-Plasma_ontology#WDM -->

    <owl:ObjectProperty rdf:about="http://www.semanticweb.org/afshar87/ontologies/2024/3/Laser-Plasma_ontology#WDM">
        <rdfs:subPropertyOf rdf:resource="http://www.w3.org/2002/07/owl#topObjectProperty"/>
    </owl:ObjectProperty>
    


    <!-- http://www.semanticweb.org/afshar87/ontologies/2024/3/Laser-Plasma_ontology#X-ray_diagnostics_to_study_WDM_and_HEDP -->

    <owl:ObjectProperty rdf:about="http://www.semanticweb.org/afshar87/ontologies/2024/3/Laser-Plasma_ontology#X-ray_diagnostics_to_study_WDM_and_HEDP">
        <rdfs:subPropertyOf rdf:resource="http://www.semanticweb.org/afshar87/ontologies/2024/3/Laser-Plasma_ontology#WDM"/>
        <rdfs:domain rdf:resource="http://www.semanticweb.org/afshar87/ontologies/2024/3/Laser-Plasma_ontology#X-ray_radiography"/>
        <rdfs:domain rdf:resource="http://www.semanticweb.org/afshar87/ontologies/2024/3/Laser-Plasma_ontology#X-ray_spectroscopy"/>
        <rdfs:range rdf:resource="http://www.semanticweb.org/afshar87/ontologies/2024/3/Laser-Plasma_ontology#High_Energy_Density_Physics_(HEDP)"/>
        <rdfs:range rdf:resource="http://www.semanticweb.org/afshar87/ontologies/2024/3/Laser-Plasma_ontology#Warm_Dense_Matter_(WDM)"/>
        <rdfs:comment>X-ray diagnostics is used to study WDM and HED physics</rdfs:comment>
    </owl:ObjectProperty>
    


    <!-- http://www.semanticweb.org/afshar87/ontologies/2024/3/Laser-Plasma_ontology#accelerates -->

    <owl:ObjectProperty rdf:about="http://www.semanticweb.org/afshar87/ontologies/2024/3/Laser-Plasma_ontology#accelerates">
        <rdfs:domain rdf:resource="http://www.semanticweb.org/afshar87/ontologies/2024/3/Laser-Plasma_ontology#Laser"/>
        <rdfs:range rdf:resource="http://www.semanticweb.org/afshar87/ontologies/2024/3/Laser-Plasma_ontology#Species"/>
        <rdfs:comment>Laser accelerates species.</rdfs:comment>
    </owl:ObjectProperty>
    


    <!-- http://www.semanticweb.org/afshar87/ontologies/2024/3/Laser-Plasma_ontology#has_Input_Parameters -->

    <owl:ObjectProperty rdf:about="http://www.semanticweb.org/afshar87/ontologies/2024/3/Laser-Plasma_ontology#has_Input_Parameters">
        <rdfs:subPropertyOf rdf:resource="http://www.semanticweb.org/afshar87/ontologies/2024/3/Laser-Plasma_ontology#Simulation"/>
        <rdfs:domain rdf:resource="http://www.semanticweb.org/afshar87/ontologies/2024/3/Laser-Plasma_ontology#Simulation"/>
        <rdfs:range rdf:resource="http://www.semanticweb.org/afshar87/ontologies/2024/3/Laser-Plasma_ontology#Laser"/>
        <rdfs:range rdf:resource="http://www.semanticweb.org/afshar87/ontologies/2024/3/Laser-Plasma_ontology#Simulation"/>
        <rdfs:range rdf:resource="http://www.semanticweb.org/afshar87/ontologies/2024/3/Laser-Plasma_ontology#Species"/>
        <rdfs:range rdf:resource="http://www.semanticweb.org/afshar87/ontologies/2024/3/Laser-Plasma_ontology#Target"/>
        <rdfs:comment>simulation  has Input Parameters  (e.g., laser intensity, plasma density).</rdfs:comment>
    </owl:ObjectProperty>
    


    <!-- http://www.semanticweb.org/afshar87/ontologies/2024/3/Laser-Plasma_ontology#has_Output_Data -->

    <owl:ObjectProperty rdf:about="http://www.semanticweb.org/afshar87/ontologies/2024/3/Laser-Plasma_ontology#has_Output_Data">
        <rdfs:subPropertyOf rdf:resource="http://www.semanticweb.org/afshar87/ontologies/2024/3/Laser-Plasma_ontology#Simulation"/>
        <rdfs:domain rdf:resource="http://www.semanticweb.org/afshar87/ontologies/2024/3/Laser-Plasma_ontology#Simulation"/>
        <rdfs:range rdf:resource="http://www.semanticweb.org/afshar87/ontologies/2024/3/Laser-Plasma_ontology#Data"/>
        <rdfs:range rdf:resource="http://www.semanticweb.org/afshar87/ontologies/2024/3/Laser-Plasma_ontology#Laser_Plasma_Application"/>
        <rdfs:range rdf:resource="http://www.semanticweb.org/afshar87/ontologies/2024/3/Laser-Plasma_ontology#Laser_Plasma_Physics"/>
        <rdfs:comment>simulation  has Output Parameters  (e.g.,  particles energy gain).</rdfs:comment>
    </owl:ObjectProperty>
    


    <!-- http://www.semanticweb.org/afshar87/ontologies/2024/3/Laser-Plasma_ontology#has_Simulation_Type -->

    <owl:ObjectProperty rdf:about="http://www.semanticweb.org/afshar87/ontologies/2024/3/Laser-Plasma_ontology#has_Simulation_Type">
        <rdfs:subPropertyOf rdf:resource="http://www.semanticweb.org/afshar87/ontologies/2024/3/Laser-Plasma_ontology#Simulation"/>
        <rdfs:domain rdf:resource="http://www.semanticweb.org/afshar87/ontologies/2024/3/Laser-Plasma_ontology#Simulation"/>
        <rdfs:range rdf:resource="http://www.semanticweb.org/afshar87/ontologies/2024/3/Laser-Plasma_ontology#Simulation"/>
        <rdfs:comment>simulation has simulation type of (e.g., PIC, MHD, Fluid).</rdfs:comment>
    </owl:ObjectProperty>
    


    <!-- http://www.semanticweb.org/afshar87/ontologies/2024/3/Laser-Plasma_ontology#has_attribute_momentum -->

    <owl:ObjectProperty rdf:about="http://www.semanticweb.org/afshar87/ontologies/2024/3/Laser-Plasma_ontology#has_attribute_momentum">
        <rdfs:subPropertyOf rdf:resource="http://www.semanticweb.org/afshar87/ontologies/2024/3/Laser-Plasma_ontology#has_attributes"/>
        <rdfs:domain rdf:resource="http://www.semanticweb.org/afshar87/ontologies/2024/3/Laser-Plasma_ontology#Macroparticle"/>
        <rdfs:range rdf:resource="http://www.semanticweb.org/afshar87/ontologies/2024/3/Laser-Plasma_ontology#Macroparticle"/>
    </owl:ObjectProperty>
    


    <!-- http://www.semanticweb.org/afshar87/ontologies/2024/3/Laser-Plasma_ontology#has_attributes -->

    <owl:ObjectProperty rdf:about="http://www.semanticweb.org/afshar87/ontologies/2024/3/Laser-Plasma_ontology#has_attributes">
        <rdfs:subPropertyOf rdf:resource="http://www.semanticweb.org/afshar87/ontologies/2024/3/Laser-Plasma_ontology#Simulation"/>
    </owl:ObjectProperty>
    


    <!-- http://www.semanticweb.org/afshar87/ontologies/2024/3/Laser-Plasma_ontology#has_attributes_position -->

    <owl:ObjectProperty rdf:about="http://www.semanticweb.org/afshar87/ontologies/2024/3/Laser-Plasma_ontology#has_attributes_position">
        <rdfs:subPropertyOf rdf:resource="http://www.semanticweb.org/afshar87/ontologies/2024/3/Laser-Plasma_ontology#has_attributes"/>
        <rdfs:domain rdf:resource="http://www.semanticweb.org/afshar87/ontologies/2024/3/Laser-Plasma_ontology#Macroparticle"/>
        <rdfs:range rdf:resource="http://www.semanticweb.org/afshar87/ontologies/2024/3/Laser-Plasma_ontology#Macroparticle"/>
    </owl:ObjectProperty>
    


    <!-- http://www.semanticweb.org/afshar87/ontologies/2024/3/Laser-Plasma_ontology#has_attributes_weighting -->

    <owl:ObjectProperty rdf:about="http://www.semanticweb.org/afshar87/ontologies/2024/3/Laser-Plasma_ontology#has_attributes_weighting">
        <rdfs:subPropertyOf rdf:resource="http://www.semanticweb.org/afshar87/ontologies/2024/3/Laser-Plasma_ontology#has_attributes"/>
        <rdfs:domain rdf:resource="http://www.semanticweb.org/afshar87/ontologies/2024/3/Laser-Plasma_ontology#Macroparticle"/>
        <rdfs:range rdf:resource="http://www.semanticweb.org/afshar87/ontologies/2024/3/Laser-Plasma_ontology#Macroparticle"/>
    </owl:ObjectProperty>
    


    <!-- http://www.semanticweb.org/afshar87/ontologies/2024/3/Laser-Plasma_ontology#has_boundary_condition -->

    <owl:ObjectProperty rdf:about="http://www.semanticweb.org/afshar87/ontologies/2024/3/Laser-Plasma_ontology#has_boundary_condition">
        <rdfs:subPropertyOf rdf:resource="http://www.semanticweb.org/afshar87/ontologies/2024/3/Laser-Plasma_ontology#Simulation"/>
        <rdfs:range rdf:resource="http://www.semanticweb.org/afshar87/ontologies/2024/3/Laser-Plasma_ontology#BoundaryConditionType"/>
    </owl:ObjectProperty>
    


    <!-- http://www.semanticweb.org/afshar87/ontologies/2024/3/Laser-Plasma_ontology#has_polarization -->

    <owl:ObjectProperty rdf:about="http://www.semanticweb.org/afshar87/ontologies/2024/3/Laser-Plasma_ontology#has_polarization">
        <rdfs:domain rdf:resource="http://www.semanticweb.org/afshar87/ontologies/2024/3/Laser-Plasma_ontology#Laser"/>
        <rdfs:comment>Laser hasPolarization laserPolarizationType</rdfs:comment>
    </owl:ObjectProperty>
    


    <!-- http://www.semanticweb.org/afshar87/ontologies/2024/3/Laser-Plasma_ontology#interact_with -->

    <owl:ObjectProperty rdf:about="http://www.semanticweb.org/afshar87/ontologies/2024/3/Laser-Plasma_ontology#interact_with">
        <rdfs:domain rdf:resource="http://www.semanticweb.org/afshar87/ontologies/2024/3/Laser-Plasma_ontology#Laser"/>
        <rdfs:range rdf:resource="http://www.semanticweb.org/afshar87/ontologies/2024/3/Laser-Plasma_ontology#Target"/>
        <rdfs:comment>laser interact_with target.</rdfs:comment>
    </owl:ObjectProperty>
    


    <!-- http://www.semanticweb.org/afshar87/ontologies/2024/3/Laser-Plasma_ontology#uses_diagnostic -->

    <owl:ObjectProperty rdf:about="http://www.semanticweb.org/afshar87/ontologies/2024/3/Laser-Plasma_ontology#uses_diagnostic"/>
    


    <!-- 
    ///////////////////////////////////////////////////////////////////////////////////////
    //
    // Data properties
    //
    ///////////////////////////////////////////////////////////////////////////////////////
     -->

    


    <!-- http://www.semanticweb.org/afshar87/ontologies/2024/3/Laser-Plasma_ontology#Creator -->

    <owl:DatatypeProperty rdf:about="http://www.semanticweb.org/afshar87/ontologies/2024/3/Laser-Plasma_ontology#Creator">
        <rdfs:domain rdf:resource="http://www.semanticweb.org/afshar87/ontologies/2024/3/Laser-Plasma_ontology#Owner"/>
        <rdfs:range rdf:resource="http://www.w3.org/2001/XMLSchema#string"/>
        <rdfs:comment>The information about the creator of this laser plasma ontology.</rdfs:comment>
    </owl:DatatypeProperty>
    


    <!-- http://www.semanticweb.org/afshar87/ontologies/2024/3/Laser-Plasma_ontology#Creator_affiliation -->

    <owl:DatatypeProperty rdf:about="http://www.semanticweb.org/afshar87/ontologies/2024/3/Laser-Plasma_ontology#Creator_affiliation">
        <rdfs:subPropertyOf rdf:resource="http://www.semanticweb.org/afshar87/ontologies/2024/3/Laser-Plasma_ontology#Creator"/>
        <rdfs:domain rdf:resource="http://www.semanticweb.org/afshar87/ontologies/2024/3/Laser-Plasma_ontology#Owner"/>
        <rdfs:range rdf:resource="http://www.w3.org/2001/XMLSchema#string"/>
        <rdfs:comment>Creator Affiliation: HZDR â€“ Helmholtz-Zentrum Dresden-Rossendorf</rdfs:comment>
    </owl:DatatypeProperty>
    


    <!-- http://www.semanticweb.org/afshar87/ontologies/2024/3/Laser-Plasma_ontology#Creator_name -->

    <owl:DatatypeProperty rdf:about="http://www.semanticweb.org/afshar87/ontologies/2024/3/Laser-Plasma_ontology#Creator_name">
        <rdfs:subPropertyOf rdf:resource="http://www.semanticweb.org/afshar87/ontologies/2024/3/Laser-Plasma_ontology#Creator"/>
        <rdfs:domain rdf:resource="http://www.semanticweb.org/afshar87/ontologies/2024/3/Laser-Plasma_ontology#Owner"/>
        <rdfs:range rdf:resource="http://www.w3.org/2001/XMLSchema#string"/>
        <rdfs:comment>The creator of this laser_plasma ontology. 

Currently: Masoud Afshari</rdfs:comment>
    </owl:DatatypeProperty>
    


    <!-- http://www.semanticweb.org/afshar87/ontologies/2024/3/Laser-Plasma_ontology#Facility_properties -->

    <owl:DatatypeProperty rdf:about="http://www.semanticweb.org/afshar87/ontologies/2024/3/Laser-Plasma_ontology#Facility_properties"/>
    


    <!-- http://www.semanticweb.org/afshar87/ontologies/2024/3/Laser-Plasma_ontology#Ionization -->

    <owl:DatatypeProperty rdf:about="http://www.semanticweb.org/afshar87/ontologies/2024/3/Laser-Plasma_ontology#Ionization">
        <rdfs:subPropertyOf rdf:resource="http://www.semanticweb.org/afshar87/ontologies/2024/3/Laser-Plasma_ontology#plasma_properties"/>
        <rdfs:domain rdf:resource="http://www.semanticweb.org/afshar87/ontologies/2024/3/Laser-Plasma_ontology#Plasma"/>
    </owl:DatatypeProperty>
    


    <!-- http://www.semanticweb.org/afshar87/ontologies/2024/3/Laser-Plasma_ontology#Ionization_ADKCircPol -->

    <owl:DatatypeProperty rdf:about="http://www.semanticweb.org/afshar87/ontologies/2024/3/Laser-Plasma_ontology#Ionization_ADKCircPol">
        <rdfs:subPropertyOf rdf:resource="http://www.semanticweb.org/afshar87/ontologies/2024/3/Laser-Plasma_ontology#Ionization"/>
        <rdfs:domain rdf:resource="http://www.semanticweb.org/afshar87/ontologies/2024/3/Laser-Plasma_ontology#Plasma"/>
        <rdfs:range rdf:resource="http://www.w3.org/2001/XMLSchema#boolean"/>
    </owl:DatatypeProperty>
    


    <!-- http://www.semanticweb.org/afshar87/ontologies/2024/3/Laser-Plasma_ontology#Ionization_BSI -->

    <owl:DatatypeProperty rdf:about="http://www.semanticweb.org/afshar87/ontologies/2024/3/Laser-Plasma_ontology#Ionization_BSI">
        <rdfs:subPropertyOf rdf:resource="http://www.semanticweb.org/afshar87/ontologies/2024/3/Laser-Plasma_ontology#Ionization"/>
        <rdfs:domain rdf:resource="http://www.semanticweb.org/afshar87/ontologies/2024/3/Laser-Plasma_ontology#Plasma"/>
        <rdfs:range rdf:resource="http://www.w3.org/2001/XMLSchema#boolean"/>
    </owl:DatatypeProperty>
    


    <!-- http://www.semanticweb.org/afshar87/ontologies/2024/3/Laser-Plasma_ontology#Ionization_BSIStarkShifted -->

    <owl:DatatypeProperty rdf:about="http://www.semanticweb.org/afshar87/ontologies/2024/3/Laser-Plasma_ontology#Ionization_BSIStarkShifted">
        <rdfs:subPropertyOf rdf:resource="http://www.semanticweb.org/afshar87/ontologies/2024/3/Laser-Plasma_ontology#Ionization"/>
        <rdfs:domain rdf:resource="http://www.semanticweb.org/afshar87/ontologies/2024/3/Laser-Plasma_ontology#Plasma"/>
        <rdfs:range rdf:resource="http://www.w3.org/2001/XMLSchema#boolean"/>
    </owl:DatatypeProperty>
    


    <!-- http://www.semanticweb.org/afshar87/ontologies/2024/3/Laser-Plasma_ontology#Ionization_BSI_Effective_Z -->

    <owl:DatatypeProperty rdf:about="http://www.semanticweb.org/afshar87/ontologies/2024/3/Laser-Plasma_ontology#Ionization_BSI_Effective_Z">
        <rdfs:subPropertyOf rdf:resource="http://www.semanticweb.org/afshar87/ontologies/2024/3/Laser-Plasma_ontology#Ionization"/>
        <rdfs:domain rdf:resource="http://www.semanticweb.org/afshar87/ontologies/2024/3/Laser-Plasma_ontology#Plasma"/>
        <rdfs:range rdf:resource="http://www.w3.org/2001/XMLSchema#boolean"/>
    </owl:DatatypeProperty>
    


    <!-- http://www.semanticweb.org/afshar87/ontologies/2024/3/Laser-Plasma_ontology#Ionization_Keldysh -->

    <owl:DatatypeProperty rdf:about="http://www.semanticweb.org/afshar87/ontologies/2024/3/Laser-Plasma_ontology#Ionization_Keldysh">
        <rdfs:subPropertyOf rdf:resource="http://www.semanticweb.org/afshar87/ontologies/2024/3/Laser-Plasma_ontology#Ionization"/>
        <rdfs:domain rdf:resource="http://www.semanticweb.org/afshar87/ontologies/2024/3/Laser-Plasma_ontology#Plasma"/>
        <rdfs:range rdf:resource="http://www.w3.org/2001/XMLSchema#boolean"/>
    </owl:DatatypeProperty>
    


    <!-- http://www.semanticweb.org/afshar87/ontologies/2024/3/Laser-Plasma_ontology#Ionization_ThomasFermi -->

    <owl:DatatypeProperty rdf:about="http://www.semanticweb.org/afshar87/ontologies/2024/3/Laser-Plasma_ontology#Ionization_ThomasFermi">
        <rdfs:subPropertyOf rdf:resource="http://www.semanticweb.org/afshar87/ontologies/2024/3/Laser-Plasma_ontology#Ionization"/>
        <rdfs:domain rdf:resource="http://www.semanticweb.org/afshar87/ontologies/2024/3/Laser-Plasma_ontology#Plasma"/>
        <rdfs:range rdf:resource="http://www.w3.org/2001/XMLSchema#boolean"/>
    </owl:DatatypeProperty>
    


    <!-- http://www.semanticweb.org/afshar87/ontologies/2024/3/Laser-Plasma_ontology#LG_mode_number -->

    <owl:DatatypeProperty rdf:about="http://www.semanticweb.org/afshar87/ontologies/2024/3/Laser-Plasma_ontology#LG_mode_number">
        <rdfs:subPropertyOf rdf:resource="http://www.semanticweb.org/afshar87/ontologies/2024/3/Laser-Plasma_ontology#laser_Laguerre-Gaussian_mode_(LG)"/>
        <rdfs:domain rdf:resource="http://www.semanticweb.org/afshar87/ontologies/2024/3/Laser-Plasma_ontology#Laser"/>
        <rdfs:range rdf:resource="http://www.w3.org/2001/XMLSchema#integer"/>
    </owl:DatatypeProperty>
    


    <!-- http://www.semanticweb.org/afshar87/ontologies/2024/3/Laser-Plasma_ontology#PI_collaborators -->

    <owl:DatatypeProperty rdf:about="http://www.semanticweb.org/afshar87/ontologies/2024/3/Laser-Plasma_ontology#PI_collaborators">
        <rdfs:subPropertyOf rdf:resource="http://www.semanticweb.org/afshar87/ontologies/2024/3/Laser-Plasma_ontology#project_Principal_Investigator_(PI)"/>
        <rdfs:domain rdf:resource="http://www.semanticweb.org/afshar87/ontologies/2024/3/Laser-Plasma_ontology#Project"/>
        <rdfs:range rdf:resource="http://www.w3.org/2001/XMLSchema#string"/>
        <rdfs:comment>collaborators who support PI.</rdfs:comment>
    </owl:DatatypeProperty>
    


    <!-- http://www.semanticweb.org/afshar87/ontologies/2024/3/Laser-Plasma_ontology#PI_contact_number -->

    <owl:DatatypeProperty rdf:about="http://www.semanticweb.org/afshar87/ontologies/2024/3/Laser-Plasma_ontology#PI_contact_number">
        <rdfs:subPropertyOf rdf:resource="http://www.semanticweb.org/afshar87/ontologies/2024/3/Laser-Plasma_ontology#project_Principal_Investigator_(PI)"/>
        <rdfs:domain rdf:resource="http://www.semanticweb.org/afshar87/ontologies/2024/3/Laser-Plasma_ontology#Project"/>
        <rdfs:range rdf:resource="http://www.w3.org/2001/XMLSchema#integer"/>
        <rdfs:comment>PI contact (phone) number</rdfs:comment>
    </owl:DatatypeProperty>
    


    <!-- http://www.semanticweb.org/afshar87/ontologies/2024/3/Laser-Plasma_ontology#PI_email_address -->

    <owl:DatatypeProperty rdf:about="http://www.semanticweb.org/afshar87/ontologies/2024/3/Laser-Plasma_ontology#PI_email_address">
        <rdfs:subPropertyOf rdf:resource="http://www.semanticweb.org/afshar87/ontologies/2024/3/Laser-Plasma_ontology#project_Principal_Investigator_(PI)"/>
        <rdfs:domain rdf:resource="http://www.semanticweb.org/afshar87/ontologies/2024/3/Laser-Plasma_ontology#Project"/>
        <rdfs:range rdf:resource="http://www.w3.org/2001/XMLSchema#string"/>
        <rdfs:comment>PI Email Address</rdfs:comment>
    </owl:DatatypeProperty>
    


    <!-- http://www.semanticweb.org/afshar87/ontologies/2024/3/Laser-Plasma_ontology#PI_institute -->

    <owl:DatatypeProperty rdf:about="http://www.semanticweb.org/afshar87/ontologies/2024/3/Laser-Plasma_ontology#PI_institute">
        <rdfs:subPropertyOf rdf:resource="http://www.semanticweb.org/afshar87/ontologies/2024/3/Laser-Plasma_ontology#project_Principal_Investigator_(PI)"/>
        <rdfs:domain rdf:resource="http://www.semanticweb.org/afshar87/ontologies/2024/3/Laser-Plasma_ontology#Project"/>
        <rdfs:range rdf:resource="http://www.w3.org/2001/XMLSchema#string"/>
        <rdfs:comment>The institute (group or department) where the PI is working there</rdfs:comment>
    </owl:DatatypeProperty>
    


    <!-- http://www.semanticweb.org/afshar87/ontologies/2024/3/Laser-Plasma_ontology#PI_name -->

    <owl:DatatypeProperty rdf:about="http://www.semanticweb.org/afshar87/ontologies/2024/3/Laser-Plasma_ontology#PI_name">
        <rdfs:subPropertyOf rdf:resource="http://www.semanticweb.org/afshar87/ontologies/2024/3/Laser-Plasma_ontology#project_Principal_Investigator_(PI)"/>
        <rdfs:domain rdf:resource="http://www.semanticweb.org/afshar87/ontologies/2024/3/Laser-Plasma_ontology#Project"/>
        <rdfs:range rdf:resource="http://www.w3.org/2001/XMLSchema#string"/>
        <rdfs:comment>the name or family name of the PI of a project.</rdfs:comment>
    </owl:DatatypeProperty>
    


    <!-- http://www.semanticweb.org/afshar87/ontologies/2024/3/Laser-Plasma_ontology#PI_website -->

    <owl:DatatypeProperty rdf:about="http://www.semanticweb.org/afshar87/ontologies/2024/3/Laser-Plasma_ontology#PI_website">
        <rdfs:subPropertyOf rdf:resource="http://www.semanticweb.org/afshar87/ontologies/2024/3/Laser-Plasma_ontology#project_Principal_Investigator_(PI)"/>
        <rdfs:domain rdf:resource="http://www.semanticweb.org/afshar87/ontologies/2024/3/Laser-Plasma_ontology#Project"/>
        <rdfs:range rdf:resource="http://www.w3.org/2001/XMLSchema#string"/>
        <rdfs:comment>the website of PI: Orcid, Google Scholar, ResearchGate, etc.</rdfs:comment>
    </owl:DatatypeProperty>
    


    <!-- http://www.semanticweb.org/afshar87/ontologies/2024/3/Laser-Plasma_ontology#Recombination -->

    <owl:DatatypeProperty rdf:about="http://www.semanticweb.org/afshar87/ontologies/2024/3/Laser-Plasma_ontology#Recombination">
        <rdfs:subPropertyOf rdf:resource="http://www.semanticweb.org/afshar87/ontologies/2024/3/Laser-Plasma_ontology#plasma_properties"/>
        <rdfs:domain rdf:resource="http://www.semanticweb.org/afshar87/ontologies/2024/3/Laser-Plasma_ontology#Plasma"/>
    </owl:DatatypeProperty>
    


    <!-- http://www.semanticweb.org/afshar87/ontologies/2024/3/Laser-Plasma_ontology#Simulation_code_DOI -->

    <owl:DatatypeProperty rdf:about="http://www.semanticweb.org/afshar87/ontologies/2024/3/Laser-Plasma_ontology#Simulation_code_DOI">
        <rdfs:subPropertyOf rdf:resource="http://www.semanticweb.org/afshar87/ontologies/2024/3/Laser-Plasma_ontology#simulation_property"/>
        <rdfs:domain rdf:resource="http://www.semanticweb.org/afshar87/ontologies/2024/3/Laser-Plasma_ontology#Simulation"/>
        <rdfs:range rdf:resource="http://www.w3.org/2001/XMLSchema#string"/>
        <rdfs:comment>The DOI of a peer-reviewed paper that address the details of the code.</rdfs:comment>
    </owl:DatatypeProperty>
    


    <!-- http://www.semanticweb.org/afshar87/ontologies/2024/3/Laser-Plasma_ontology#Simulation_code_Git -->

    <owl:DatatypeProperty rdf:about="http://www.semanticweb.org/afshar87/ontologies/2024/3/Laser-Plasma_ontology#Simulation_code_Git">
        <rdfs:subPropertyOf rdf:resource="http://www.semanticweb.org/afshar87/ontologies/2024/3/Laser-Plasma_ontology#simulation_property"/>
        <rdfs:domain rdf:resource="http://www.semanticweb.org/afshar87/ontologies/2024/3/Laser-Plasma_ontology#Simulation"/>
        <rdfs:range rdf:resource="http://www.w3.org/2001/XMLSchema#string"/>
        <rdfs:comment>The git address of the code where it is maintained and updated.</rdfs:comment>
    </owl:DatatypeProperty>
    


    <!-- http://www.semanticweb.org/afshar87/ontologies/2024/3/Laser-Plasma_ontology#Simulation_code_name -->

    <owl:DatatypeProperty rdf:about="http://www.semanticweb.org/afshar87/ontologies/2024/3/Laser-Plasma_ontology#Simulation_code_name">
        <rdfs:subPropertyOf rdf:resource="http://www.semanticweb.org/afshar87/ontologies/2024/3/Laser-Plasma_ontology#simulation_property"/>
        <rdfs:domain rdf:resource="http://www.semanticweb.org/afshar87/ontologies/2024/3/Laser-Plasma_ontology#Simulation"/>
        <rdfs:range rdf:resource="http://www.w3.org/2001/XMLSchema#string"/>
        <rdfs:comment>The name of simulation code</rdfs:comment>
    </owl:DatatypeProperty>
    


    <!-- http://www.semanticweb.org/afshar87/ontologies/2024/3/Laser-Plasma_ontology#bunch_divergence -->

    <owl:DatatypeProperty rdf:about="http://www.semanticweb.org/afshar87/ontologies/2024/3/Laser-Plasma_ontology#bunch_divergence">
        <rdfs:subPropertyOf rdf:resource="http://www.semanticweb.org/afshar87/ontologies/2024/3/Laser-Plasma_ontology#particle_bunch_properties"/>
        <rdfs:domain rdf:resource="http://www.semanticweb.org/afshar87/ontologies/2024/3/Laser-Plasma_ontology#Laser_Plasma_Application"/>
        <rdfs:range rdf:resource="http://www.w3.org/2001/XMLSchema#float"/>
        <rdfs:comment>the angular spread of the particle beam  from the central axis of the beam. It  describes how a beam widens as it travels. 

 The unit of divergence for a particle beam is radians per unit length. A divergence of 1 radian per meter (1 rad/m) signifies that for every meter the beam travels, it widens by an angle of 1 radian.</rdfs:comment>
    </owl:DatatypeProperty>
    


    <!-- http://www.semanticweb.org/afshar87/ontologies/2024/3/Laser-Plasma_ontology#bunch_emittance -->

    <owl:DatatypeProperty rdf:about="http://www.semanticweb.org/afshar87/ontologies/2024/3/Laser-Plasma_ontology#bunch_emittance">
        <rdfs:subPropertyOf rdf:resource="http://www.semanticweb.org/afshar87/ontologies/2024/3/Laser-Plasma_ontology#particle_bunch_properties"/>
        <rdfs:domain rdf:resource="http://www.semanticweb.org/afshar87/ontologies/2024/3/Laser-Plasma_ontology#Laser_Plasma_Application"/>
        <rdfs:range rdf:resource="http://www.w3.org/2001/XMLSchema#float"/>
        <rdfs:comment>the beam&apos;s phase space characteristics, indicating its divergence and focusability.</rdfs:comment>
    </owl:DatatypeProperty>
    


    <!-- http://www.semanticweb.org/afshar87/ontologies/2024/3/Laser-Plasma_ontology#bunch_emittance_X -->

    <owl:DatatypeProperty rdf:about="http://www.semanticweb.org/afshar87/ontologies/2024/3/Laser-Plasma_ontology#bunch_emittance_X">
        <rdfs:subPropertyOf rdf:resource="http://www.semanticweb.org/afshar87/ontologies/2024/3/Laser-Plasma_ontology#particle_bunch_properties"/>
        <rdfs:domain rdf:resource="http://www.semanticweb.org/afshar87/ontologies/2024/3/Laser-Plasma_ontology#Laser_Plasma_Application"/>
        <rdfs:range rdf:resource="http://www.w3.org/2001/XMLSchema#float"/>
        <rdfs:comment>the beam&apos;s phase space characteristics, indicating its divergence and focusability in the  X direction</rdfs:comment>
    </owl:DatatypeProperty>
    


    <!-- http://www.semanticweb.org/afshar87/ontologies/2024/3/Laser-Plasma_ontology#bunch_emittance_Y -->

    <owl:DatatypeProperty rdf:about="http://www.semanticweb.org/afshar87/ontologies/2024/3/Laser-Plasma_ontology#bunch_emittance_Y">
        <rdfs:subPropertyOf rdf:resource="http://www.semanticweb.org/afshar87/ontologies/2024/3/Laser-Plasma_ontology#particle_bunch_properties"/>
        <rdfs:comment>the beam&apos;s phase space characteristics, indicating its divergence and focusability in the  Y direction</rdfs:comment>
    </owl:DatatypeProperty>
    


    <!-- http://www.semanticweb.org/afshar87/ontologies/2024/3/Laser-Plasma_ontology#bunch_emittance_Z -->

    <owl:DatatypeProperty rdf:about="http://www.semanticweb.org/afshar87/ontologies/2024/3/Laser-Plasma_ontology#bunch_emittance_Z">
        <rdfs:subPropertyOf rdf:resource="http://www.semanticweb.org/afshar87/ontologies/2024/3/Laser-Plasma_ontology#particle_bunch_properties"/>
        <rdfs:comment>the beam&apos;s phase space characteristics, indicating its divergence and focusability in the  Z direction</rdfs:comment>
    </owl:DatatypeProperty>
    


    <!-- http://www.semanticweb.org/afshar87/ontologies/2024/3/Laser-Plasma_ontology#bunch_energy_spectrum_type -->

    <owl:DatatypeProperty rdf:about="http://www.semanticweb.org/afshar87/ontologies/2024/3/Laser-Plasma_ontology#bunch_energy_spectrum_type">
        <rdfs:subPropertyOf rdf:resource="http://www.semanticweb.org/afshar87/ontologies/2024/3/Laser-Plasma_ontology#particle_bunch_properties"/>
        <rdfs:domain rdf:resource="http://www.semanticweb.org/afshar87/ontologies/2024/3/Laser-Plasma_ontology#Laser_Plasma_Application"/>
        <rdfs:range rdf:resource="http://www.w3.org/2001/XMLSchema#string"/>
        <rdfs:comment>spectrumType&quot; (e.g., &quot;GaussianSpectrum,&quot; &quot;MonoenergeticSpectrum&quot;) and parameters specific to that type. For example, a &quot;GaussianSpectrum&quot; class might have properties for &quot;meanEnergy&quot; and &quot;standardDeviation&quot; to represent a Gaussian energy distribution.</rdfs:comment>
    </owl:DatatypeProperty>
    


    <!-- http://www.semanticweb.org/afshar87/ontologies/2024/3/Laser-Plasma_ontology#bunch_mean_energy -->

    <owl:DatatypeProperty rdf:about="http://www.semanticweb.org/afshar87/ontologies/2024/3/Laser-Plasma_ontology#bunch_mean_energy">
        <rdfs:subPropertyOf rdf:resource="http://www.semanticweb.org/afshar87/ontologies/2024/3/Laser-Plasma_ontology#particle_bunch_properties"/>
        <rdfs:domain rdf:resource="http://www.semanticweb.org/afshar87/ontologies/2024/3/Laser-Plasma_ontology#Laser_Plasma_Application"/>
        <rdfs:range rdf:resource="http://www.w3.org/2001/XMLSchema#float"/>
        <rdfs:comment>the mean energy of particle bunch</rdfs:comment>
    </owl:DatatypeProperty>
    


    <!-- http://www.semanticweb.org/afshar87/ontologies/2024/3/Laser-Plasma_ontology#bunch_peak_energy -->

    <owl:DatatypeProperty rdf:about="http://www.semanticweb.org/afshar87/ontologies/2024/3/Laser-Plasma_ontology#bunch_peak_energy">
        <rdfs:subPropertyOf rdf:resource="http://www.semanticweb.org/afshar87/ontologies/2024/3/Laser-Plasma_ontology#particle_bunch_properties"/>
        <rdfs:domain rdf:resource="http://www.semanticweb.org/afshar87/ontologies/2024/3/Laser-Plasma_ontology#Laser_Plasma_Application"/>
        <rdfs:range rdf:resource="http://www.w3.org/2001/XMLSchema#float"/>
        <rdfs:comment>the peak energy of the particle bunch</rdfs:comment>
    </owl:DatatypeProperty>
    


    <!-- http://www.semanticweb.org/afshar87/ontologies/2024/3/Laser-Plasma_ontology#bunch_pulse_duration -->

    <owl:DatatypeProperty rdf:about="http://www.semanticweb.org/afshar87/ontologies/2024/3/Laser-Plasma_ontology#bunch_pulse_duration">
        <rdfs:subPropertyOf rdf:resource="http://www.semanticweb.org/afshar87/ontologies/2024/3/Laser-Plasma_ontology#particle_bunch_properties"/>
        <rdfs:domain rdf:resource="http://www.semanticweb.org/afshar87/ontologies/2024/3/Laser-Plasma_ontology#Laser_Plasma_Application"/>
        <rdfs:range rdf:resource="http://www.w3.org/2001/XMLSchema#float"/>
        <rdfs:comment>the Pulse Duration of particle bunch</rdfs:comment>
    </owl:DatatypeProperty>
    


    <!-- http://www.semanticweb.org/afshar87/ontologies/2024/3/Laser-Plasma_ontology#bunch_repetition_rate -->

    <owl:DatatypeProperty rdf:about="http://www.semanticweb.org/afshar87/ontologies/2024/3/Laser-Plasma_ontology#bunch_repetition_rate">
        <rdfs:subPropertyOf rdf:resource="http://www.semanticweb.org/afshar87/ontologies/2024/3/Laser-Plasma_ontology#particle_bunch_properties"/>
        <rdfs:domain rdf:resource="http://www.semanticweb.org/afshar87/ontologies/2024/3/Laser-Plasma_ontology#Laser_Plasma_Application"/>
        <rdfs:range rdf:resource="http://www.w3.org/2001/XMLSchema#float"/>
        <rdfs:comment>for pulsed beams, such as those created with pulsed lasers, indicates the number of pulses emitted per unit time (Hz).</rdfs:comment>
    </owl:DatatypeProperty>
    


    <!-- http://www.semanticweb.org/afshar87/ontologies/2024/3/Laser-Plasma_ontology#bunch_spatial_profile_type -->

    <owl:DatatypeProperty rdf:about="http://www.semanticweb.org/afshar87/ontologies/2024/3/Laser-Plasma_ontology#bunch_spatial_profile_type">
        <rdfs:subPropertyOf rdf:resource="http://www.semanticweb.org/afshar87/ontologies/2024/3/Laser-Plasma_ontology#particle_bunch_properties"/>
        <rdfs:domain rdf:resource="http://www.semanticweb.org/afshar87/ontologies/2024/3/Laser-Plasma_ontology#Laser_Plasma_Application"/>
        <rdfs:range rdf:resource="http://www.w3.org/2001/XMLSchema#string"/>
        <rdfs:comment>the spatial distribution of particle density within the beam  (e.g., &quot;GaussianProfile,&quot; &quot;UniformProfile&quot;) similar to the energy spectrum</rdfs:comment>
    </owl:DatatypeProperty>
    


    <!-- http://www.semanticweb.org/afshar87/ontologies/2024/3/Laser-Plasma_ontology#bunch_species -->

    <owl:DatatypeProperty rdf:about="http://www.semanticweb.org/afshar87/ontologies/2024/3/Laser-Plasma_ontology#bunch_species">
        <rdfs:subPropertyOf rdf:resource="http://www.semanticweb.org/afshar87/ontologies/2024/3/Laser-Plasma_ontology#particle_bunch_properties"/>
        <rdfs:domain rdf:resource="http://www.semanticweb.org/afshar87/ontologies/2024/3/Laser-Plasma_ontology#Laser_Plasma_Application"/>
        <rdfs:range rdf:resource="http://www.w3.org/2001/XMLSchema#string"/>
        <rdfs:seeAlso>the type of particle in the beam (e.g., &quot;proton,&quot; &quot;electron,&quot; &quot;carbonIon&quot;). it determines the distribution of individual energies and how many particles in the bunch have a specific energy or energy range.</rdfs:seeAlso>
    </owl:DatatypeProperty>
    


    <!-- http://www.semanticweb.org/afshar87/ontologies/2024/3/Laser-Plasma_ontology#bunch_standard_deviation -->

    <owl:DatatypeProperty rdf:about="http://www.semanticweb.org/afshar87/ontologies/2024/3/Laser-Plasma_ontology#bunch_standard_deviation">
        <rdfs:subPropertyOf rdf:resource="http://www.semanticweb.org/afshar87/ontologies/2024/3/Laser-Plasma_ontology#particle_bunch_properties"/>
        <rdfs:domain rdf:resource="http://www.semanticweb.org/afshar87/ontologies/2024/3/Laser-Plasma_ontology#Laser_Plasma_Application"/>
        <rdfs:range rdf:resource="http://www.w3.org/2001/XMLSchema#float"/>
        <rdfs:comment>the standard deviation of particle bunch energy</rdfs:comment>
    </owl:DatatypeProperty>
    


    <!-- http://www.semanticweb.org/afshar87/ontologies/2024/3/Laser-Plasma_ontology#bunch_total_charge -->

    <owl:DatatypeProperty rdf:about="http://www.semanticweb.org/afshar87/ontologies/2024/3/Laser-Plasma_ontology#bunch_total_charge">
        <rdfs:subPropertyOf rdf:resource="http://www.semanticweb.org/afshar87/ontologies/2024/3/Laser-Plasma_ontology#particle_bunch_properties"/>
        <rdfs:domain rdf:resource="http://www.semanticweb.org/afshar87/ontologies/2024/3/Laser-Plasma_ontology#Laser_Plasma_Application"/>
        <rdfs:range rdf:resource="http://www.w3.org/2001/XMLSchema#float"/>
        <rdfs:comment>total charge of a particle bunch</rdfs:comment>
    </owl:DatatypeProperty>
    


    <!-- http://www.semanticweb.org/afshar87/ontologies/2024/3/Laser-Plasma_ontology#bunch_transmittance -->

    <owl:DatatypeProperty rdf:about="http://www.semanticweb.org/afshar87/ontologies/2024/3/Laser-Plasma_ontology#bunch_transmittance">
        <rdfs:subPropertyOf rdf:resource="http://www.semanticweb.org/afshar87/ontologies/2024/3/Laser-Plasma_ontology#particle_bunch_properties"/>
        <rdfs:domain rdf:resource="http://www.semanticweb.org/afshar87/ontologies/2024/3/Laser-Plasma_ontology#Laser_Plasma_Application"/>
        <rdfs:range rdf:resource="http://www.w3.org/2001/XMLSchema#float"/>
        <rdfs:comment>if beam interacts with materials, specifies the fraction of particles that pass through a material without being absorbed or scattered.</rdfs:comment>
    </owl:DatatypeProperty>
    


    <!-- http://www.semanticweb.org/afshar87/ontologies/2024/3/Laser-Plasma_ontology#creator_identifier -->

    <owl:DatatypeProperty rdf:about="http://www.semanticweb.org/afshar87/ontologies/2024/3/Laser-Plasma_ontology#creator_identifier">
        <rdfs:subPropertyOf rdf:resource="http://www.semanticweb.org/afshar87/ontologies/2024/3/Laser-Plasma_ontology#Creator"/>
        <rdfs:domain rdf:resource="http://www.semanticweb.org/afshar87/ontologies/2024/3/Laser-Plasma_ontology#Owner"/>
        <rdfs:range rdf:resource="http://www.w3.org/2001/XMLSchema#string"/>
        <rdfs:comment>creator identifier : https://orcid.org/0000-0003-4486-9683</rdfs:comment>
    </owl:DatatypeProperty>
    


    <!-- http://www.semanticweb.org/afshar87/ontologies/2024/3/Laser-Plasma_ontology#data_acquisition_method -->

    <owl:DatatypeProperty rdf:about="http://www.semanticweb.org/afshar87/ontologies/2024/3/Laser-Plasma_ontology#data_acquisition_method">
        <rdfs:subPropertyOf rdf:resource="http://www.semanticweb.org/afshar87/ontologies/2024/3/Laser-Plasma_ontology#data_property"/>
        <rdfs:domain rdf:resource="http://www.semanticweb.org/afshar87/ontologies/2024/3/Laser-Plasma_ontology#Data"/>
        <rdfs:domain rdf:resource="http://www.semanticweb.org/afshar87/ontologies/2024/3/Laser-Plasma_ontology#Diagnostics"/>
        <rdfs:domain rdf:resource="http://www.semanticweb.org/afshar87/ontologies/2024/3/Laser-Plasma_ontology#Experiment"/>
        <rdfs:domain rdf:resource="http://www.semanticweb.org/afshar87/ontologies/2024/3/Laser-Plasma_ontology#Simulation"/>
        <rdfs:range rdf:resource="http://www.w3.org/2001/XMLSchema#string"/>
        <rdfs:comment>data acquisition methods used in an experiment. e.g.,  &quot;Time-resolved spectroscopy,&quot; &quot;X-ray imaging&quot;.</rdfs:comment>
    </owl:DatatypeProperty>
    


    <!-- http://www.semanticweb.org/afshar87/ontologies/2024/3/Laser-Plasma_ontology#data_calibration_method -->

    <owl:DatatypeProperty rdf:about="http://www.semanticweb.org/afshar87/ontologies/2024/3/Laser-Plasma_ontology#data_calibration_method">
        <rdfs:subPropertyOf rdf:resource="http://www.semanticweb.org/afshar87/ontologies/2024/3/Laser-Plasma_ontology#data_property"/>
        <rdfs:domain rdf:resource="http://www.semanticweb.org/afshar87/ontologies/2024/3/Laser-Plasma_ontology#Data"/>
        <rdfs:domain rdf:resource="http://www.semanticweb.org/afshar87/ontologies/2024/3/Laser-Plasma_ontology#Diagnostics"/>
        <rdfs:domain rdf:resource="http://www.semanticweb.org/afshar87/ontologies/2024/3/Laser-Plasma_ontology#Experiment"/>
        <rdfs:domain rdf:resource="http://www.semanticweb.org/afshar87/ontologies/2024/3/Laser-Plasma_ontology#Simulation"/>
        <rdfs:range rdf:resource="http://www.w3.org/2001/XMLSchema#string"/>
        <rdfs:comment>It describes the specific techniques or procedures used to ensure the accuracy and reliability of the data collected by a diagnostic tool during the experimental campaign.for instance: General Calibration Methods:

Dark Current Correction: This method accounts for background signal in detectors used for measuring light or particle flux.

Flat-Field Correction: This method corrects for spatial non-uniformities in detector response, ensuring consistent sensitivity across the entire detection area.

Energy Calibration: This method establishes the relationship between the detector signal and the actual energy of particles (e.g., electrons, ions) being measured.

Wavelength Calibration: This method defines the relationship between the detector signal and the actual wavelength of light for spectroscopic techniques.

LaserPlasma Specific Calibration Methods:

Thomson Scattering Calibration: This method utilizes reference materials with well-defined electron density and temperature to calibrate the measurement of these parameters in the plasma using Thomson Scattering diagnostics.

Interferometry Calibration: This method employs reference paths with known optical path lengths to calibrate the measurement of electron density in the plasma using interferometry diagnostics.

Particle Spectrometer Calibration: This method utilizes well-characterized radioactive sources emitting particles with known energies to calibrate the energy scale and resolution of particle spectrometers used to diagnose particle acceleration in the plasma.</rdfs:comment>
    </owl:DatatypeProperty>
    


    <!-- http://www.semanticweb.org/afshar87/ontologies/2024/3/Laser-Plasma_ontology#data_encoding_scheme -->

    <owl:DatatypeProperty rdf:about="http://www.semanticweb.org/afshar87/ontologies/2024/3/Laser-Plasma_ontology#data_encoding_scheme">
        <rdfs:subPropertyOf rdf:resource="http://www.semanticweb.org/afshar87/ontologies/2024/3/Laser-Plasma_ontology#data_property"/>
        <rdfs:domain rdf:resource="http://www.semanticweb.org/afshar87/ontologies/2024/3/Laser-Plasma_ontology#Data"/>
        <rdfs:range rdf:resource="http://www.w3.org/2001/XMLSchema#string"/>
        <rdfs:comment>This refers to the specific method used to represent characters, numbers, and other data elements within a data format.
Different encoding schemes define how these elements are translated into a series of bits (0s and 1s) that computers can understand.

Common encoding schemes:

ASCII (American Standard Code for Information Interchange): A widely used character encoding for text formats, representing characters with 7-bit or 8-bit codes.

Unicode: A more comprehensive character encoding that can represent a wider range of characters, including those from various languages and symbols.

Binary encoding schemes: Specific to binary formats, defining how data types like integers, floating-point numbers, or images are represented in binary form.</rdfs:comment>
    </owl:DatatypeProperty>
    


    <!-- http://www.semanticweb.org/afshar87/ontologies/2024/3/Laser-Plasma_ontology#data_filename_extension -->

    <owl:DatatypeProperty rdf:about="http://www.semanticweb.org/afshar87/ontologies/2024/3/Laser-Plasma_ontology#data_filename_extension">
        <rdfs:subPropertyOf rdf:resource="http://www.semanticweb.org/afshar87/ontologies/2024/3/Laser-Plasma_ontology#data_property"/>
        <rdfs:domain rdf:resource="http://www.semanticweb.org/afshar87/ontologies/2024/3/Laser-Plasma_ontology#Data"/>
        <rdfs:range rdf:resource="http://www.w3.org/2001/XMLSchema#string"/>
        <rdfs:comment>This is a short suffix added to the filename that indicates the data format of the file.
Operating systems and software applications use file extensions to identify the appropriate program to open or process the data.
Common examples:
&quot;.txt&quot; for plain text files
&quot;.csv&quot; for comma-separated values
&quot;.jpg&quot; for JPEG image files
&quot;.doc&quot; for Microsoft Word documents</rdfs:comment>
    </owl:DatatypeProperty>
    


    <!-- http://www.semanticweb.org/afshar87/ontologies/2024/3/Laser-Plasma_ontology#data_format -->

    <owl:DatatypeProperty rdf:about="http://www.semanticweb.org/afshar87/ontologies/2024/3/Laser-Plasma_ontology#data_format">
        <rdfs:subPropertyOf rdf:resource="http://www.semanticweb.org/afshar87/ontologies/2024/3/Laser-Plasma_ontology#data_property"/>
        <rdfs:domain rdf:resource="http://www.semanticweb.org/afshar87/ontologies/2024/3/Laser-Plasma_ontology#Data"/>
        <rdfs:range rdf:resource="http://www.w3.org/2001/XMLSchema#string"/>
        <rdfs:comment>This refers to the specific way data is structured and represented for storage or transmission. It defines how the data elements are arranged and interpreted by a computer program.

There are various data formats, each with its strengths and weaknesses:

Text formats: Human-readable formats like CSV (comma-separated values), plain text, or JSON (JavaScript Object Notation) use simple text characters to represent data.

Binary formats: These formats store data directly in machine code, making them more compact and efficient for computer processing but not human-readable. Examples include image formats (JPEG, PNG) or executable programs.

Database formats: Structured formats designed for efficient storage and retrieval of data in databases. Examples include SQL (Structured Query Language) or NoSQL databases.</rdfs:comment>
    </owl:DatatypeProperty>
    


    <!-- http://www.semanticweb.org/afshar87/ontologies/2024/3/Laser-Plasma_ontology#data_metadata -->

    <owl:DatatypeProperty rdf:about="http://www.semanticweb.org/afshar87/ontologies/2024/3/Laser-Plasma_ontology#data_metadata">
        <rdfs:subPropertyOf rdf:resource="http://www.semanticweb.org/afshar87/ontologies/2024/3/Laser-Plasma_ontology#data_type"/>
        <rdfs:domain rdf:resource="http://www.semanticweb.org/afshar87/ontologies/2024/3/Laser-Plasma_ontology#Data"/>
        <rdfs:range rdf:resource="http://www.w3.org/2001/XMLSchema#string"/>
        <rdfs:comment>Metadata: Provides information about the data and can be:

Descriptive Metadata: Provides information about the data itself (e.g., title, author, creation date, format).

Structural Metadata: Describes the organization and structure of the data (e.g., data types, units, relationships).

Administrative Metadata: Includes information about data access, ownership, and permissions.

Provenance Metadata: Tracks the origin and history of the data (e.g., processing steps, software used).</rdfs:comment>
    </owl:DatatypeProperty>
    


    <!-- http://www.semanticweb.org/afshar87/ontologies/2024/3/Laser-Plasma_ontology#data_processed -->

    <owl:DatatypeProperty rdf:about="http://www.semanticweb.org/afshar87/ontologies/2024/3/Laser-Plasma_ontology#data_processed">
        <rdfs:subPropertyOf rdf:resource="http://www.semanticweb.org/afshar87/ontologies/2024/3/Laser-Plasma_ontology#data_type"/>
        <rdfs:domain rdf:resource="http://www.semanticweb.org/afshar87/ontologies/2024/3/Laser-Plasma_ontology#Data"/>
        <rdfs:range rdf:resource="http://www.w3.org/2001/XMLSchema#string"/>
        <rdfs:comment>processed raw data achieved in simulation or experiment.</rdfs:comment>
    </owl:DatatypeProperty>
    


    <!-- http://www.semanticweb.org/afshar87/ontologies/2024/3/Laser-Plasma_ontology#data_property -->

    <owl:DatatypeProperty rdf:about="http://www.semanticweb.org/afshar87/ontologies/2024/3/Laser-Plasma_ontology#data_property"/>
    


    <!-- http://www.semanticweb.org/afshar87/ontologies/2024/3/Laser-Plasma_ontology#data_raw -->

    <owl:DatatypeProperty rdf:about="http://www.semanticweb.org/afshar87/ontologies/2024/3/Laser-Plasma_ontology#data_raw">
        <rdfs:subPropertyOf rdf:resource="http://www.semanticweb.org/afshar87/ontologies/2024/3/Laser-Plasma_ontology#data_type"/>
        <rdfs:domain rdf:resource="http://www.semanticweb.org/afshar87/ontologies/2024/3/Laser-Plasma_ontology#Data"/>
        <rdfs:range rdf:resource="http://www.w3.org/2001/XMLSchema#string"/>
        <rdfs:comment>raw data achieved in simulation or experiment.</rdfs:comment>
    </owl:DatatypeProperty>
    


    <!-- http://www.semanticweb.org/afshar87/ontologies/2024/3/Laser-Plasma_ontology#data_type -->

    <owl:DatatypeProperty rdf:about="http://www.semanticweb.org/afshar87/ontologies/2024/3/Laser-Plasma_ontology#data_type">
        <rdfs:subPropertyOf rdf:resource="http://www.semanticweb.org/afshar87/ontologies/2024/3/Laser-Plasma_ontology#data_property"/>
        <rdfs:domain rdf:resource="http://www.semanticweb.org/afshar87/ontologies/2024/3/Laser-Plasma_ontology#Data"/>
        <rdfs:range rdf:resource="http://www.w3.org/2001/XMLSchema#string"/>
        <rdfs:comment>the type of data achieved in experiments or simulations</rdfs:comment>
    </owl:DatatypeProperty>
    


    <!-- http://www.semanticweb.org/afshar87/ontologies/2024/3/Laser-Plasma_ontology#diagnostic_name -->

    <owl:DatatypeProperty rdf:about="http://www.semanticweb.org/afshar87/ontologies/2024/3/Laser-Plasma_ontology#diagnostic_name">
        <rdfs:subPropertyOf rdf:resource="http://www.semanticweb.org/afshar87/ontologies/2024/3/Laser-Plasma_ontology#diagnostic_property"/>
        <rdfs:domain rdf:resource="http://www.semanticweb.org/afshar87/ontologies/2024/3/Laser-Plasma_ontology#Diagnostics"/>
        <rdfs:range rdf:resource="http://www.w3.org/2001/XMLSchema#string"/>
        <rdfs:comment>The diagnostic   used in an experiment: &quot;X-ray Spectroscopy&quot;, &quot;Thomson Scattering,&quot; &quot;Optical Interferometry,&quot; &quot;Particle Spectrometer.&quot; etc.</rdfs:comment>
    </owl:DatatypeProperty>
    


    <!-- http://www.semanticweb.org/afshar87/ontologies/2024/3/Laser-Plasma_ontology#diagnostic_property -->

    <owl:DatatypeProperty rdf:about="http://www.semanticweb.org/afshar87/ontologies/2024/3/Laser-Plasma_ontology#diagnostic_property">
        <rdfs:domain rdf:resource="http://www.semanticweb.org/afshar87/ontologies/2024/3/Laser-Plasma_ontology#Diagnostics"/>
    </owl:DatatypeProperty>
    


    <!-- http://www.semanticweb.org/afshar87/ontologies/2024/3/Laser-Plasma_ontology#electromagnetic_fields -->

    <owl:DatatypeProperty rdf:about="http://www.semanticweb.org/afshar87/ontologies/2024/3/Laser-Plasma_ontology#electromagnetic_fields">
        <rdfs:subPropertyOf rdf:resource="http://www.semanticweb.org/afshar87/ontologies/2024/3/Laser-Plasma_ontology#plasma_properties"/>
        <rdfs:domain rdf:resource="http://www.semanticweb.org/afshar87/ontologies/2024/3/Laser-Plasma_ontology#Plasma"/>
        <rdfs:range rdf:resource="http://www.w3.org/2001/XMLSchema#double"/>
        <rdfs:range rdf:resource="http://www.w3.org/2001/XMLSchema#string"/>
    </owl:DatatypeProperty>
    


    <!-- http://www.semanticweb.org/afshar87/ontologies/2024/3/Laser-Plasma_ontology#facility_address -->

    <owl:DatatypeProperty rdf:about="http://www.semanticweb.org/afshar87/ontologies/2024/3/Laser-Plasma_ontology#facility_address">
        <rdfs:subPropertyOf rdf:resource="http://www.semanticweb.org/afshar87/ontologies/2024/3/Laser-Plasma_ontology#Facility_properties"/>
        <rdfs:domain rdf:resource="http://www.semanticweb.org/afshar87/ontologies/2024/3/Laser-Plasma_ontology#Facility"/>
        <rdfs:range rdf:resource="http://www.w3.org/2001/XMLSchema#string"/>
        <rdfs:comment>The Address of facility (either eperimental facility or Sumpercomputer)</rdfs:comment>
    </owl:DatatypeProperty>
    


    <!-- http://www.semanticweb.org/afshar87/ontologies/2024/3/Laser-Plasma_ontology#facility_fund -->

    <owl:DatatypeProperty rdf:about="http://www.semanticweb.org/afshar87/ontologies/2024/3/Laser-Plasma_ontology#facility_fund">
        <rdfs:subPropertyOf rdf:resource="http://www.semanticweb.org/afshar87/ontologies/2024/3/Laser-Plasma_ontology#Facility_properties"/>
        <rdfs:domain rdf:resource="http://www.semanticweb.org/afshar87/ontologies/2024/3/Laser-Plasma_ontology#Facility"/>
        <rdfs:range rdf:resource="http://www.w3.org/2001/XMLSchema#string"/>
        <rdfs:comment>The fund that is dedicated to that facility to perform a specific experiment.</rdfs:comment>
    </owl:DatatypeProperty>
    


    <!-- http://www.semanticweb.org/afshar87/ontologies/2024/3/Laser-Plasma_ontology#facility_name -->

    <owl:DatatypeProperty rdf:about="http://www.semanticweb.org/afshar87/ontologies/2024/3/Laser-Plasma_ontology#facility_name">
        <rdfs:subPropertyOf rdf:resource="http://www.semanticweb.org/afshar87/ontologies/2024/3/Laser-Plasma_ontology#Facility_properties"/>
        <rdfs:domain rdf:resource="http://www.semanticweb.org/afshar87/ontologies/2024/3/Laser-Plasma_ontology#Facility"/>
        <rdfs:range rdf:resource="http://www.w3.org/2001/XMLSchema#string"/>
        <rdfs:comment>The name of facility (either eperimental facility or Sumpercomputer)</rdfs:comment>
    </owl:DatatypeProperty>
    


    <!-- http://www.semanticweb.org/afshar87/ontologies/2024/3/Laser-Plasma_ontology#huygens_surface_positions_xmax -->

    <owl:DatatypeProperty rdf:about="http://www.semanticweb.org/afshar87/ontologies/2024/3/Laser-Plasma_ontology#huygens_surface_positions_xmax">
        <rdfs:subPropertyOf rdf:resource="http://www.semanticweb.org/afshar87/ontologies/2024/3/Laser-Plasma_ontology#laser_huygens_surface_positions"/>
        <rdfs:domain rdf:resource="http://www.semanticweb.org/afshar87/ontologies/2024/3/Laser-Plasma_ontology#Laser"/>
        <rdfs:range rdf:resource="http://www.w3.org/2001/XMLSchema#integer"/>
    </owl:DatatypeProperty>
    


    <!-- http://www.semanticweb.org/afshar87/ontologies/2024/3/Laser-Plasma_ontology#huygens_surface_positions_xmin -->

    <owl:DatatypeProperty rdf:about="http://www.semanticweb.org/afshar87/ontologies/2024/3/Laser-Plasma_ontology#huygens_surface_positions_xmin">
        <rdfs:subPropertyOf rdf:resource="http://www.semanticweb.org/afshar87/ontologies/2024/3/Laser-Plasma_ontology#laser_huygens_surface_positions"/>
        <rdfs:domain rdf:resource="http://www.semanticweb.org/afshar87/ontologies/2024/3/Laser-Plasma_ontology#Laser"/>
        <rdfs:range rdf:resource="http://www.w3.org/2001/XMLSchema#integer"/>
    </owl:DatatypeProperty>
    


    <!-- http://www.semanticweb.org/afshar87/ontologies/2024/3/Laser-Plasma_ontology#huygens_surface_positions_ymax -->

    <owl:DatatypeProperty rdf:about="http://www.semanticweb.org/afshar87/ontologies/2024/3/Laser-Plasma_ontology#huygens_surface_positions_ymax">
        <rdfs:subPropertyOf rdf:resource="http://www.semanticweb.org/afshar87/ontologies/2024/3/Laser-Plasma_ontology#laser_huygens_surface_positions"/>
        <rdfs:domain rdf:resource="http://www.semanticweb.org/afshar87/ontologies/2024/3/Laser-Plasma_ontology#Laser"/>
        <rdfs:range rdf:resource="http://www.w3.org/2001/XMLSchema#integer"/>
    </owl:DatatypeProperty>
    


    <!-- http://www.semanticweb.org/afshar87/ontologies/2024/3/Laser-Plasma_ontology#huygens_surface_positions_ymin -->

    <owl:DatatypeProperty rdf:about="http://www.semanticweb.org/afshar87/ontologies/2024/3/Laser-Plasma_ontology#huygens_surface_positions_ymin">
        <rdfs:subPropertyOf rdf:resource="http://www.semanticweb.org/afshar87/ontologies/2024/3/Laser-Plasma_ontology#laser_huygens_surface_positions"/>
        <rdfs:domain rdf:resource="http://www.semanticweb.org/afshar87/ontologies/2024/3/Laser-Plasma_ontology#Laser"/>
        <rdfs:range rdf:resource="http://www.w3.org/2001/XMLSchema#integer"/>
    </owl:DatatypeProperty>
    


    <!-- http://www.semanticweb.org/afshar87/ontologies/2024/3/Laser-Plasma_ontology#huygens_surface_positions_zmax -->

    <owl:DatatypeProperty rdf:about="http://www.semanticweb.org/afshar87/ontologies/2024/3/Laser-Plasma_ontology#huygens_surface_positions_zmax">
        <rdfs:subPropertyOf rdf:resource="http://www.semanticweb.org/afshar87/ontologies/2024/3/Laser-Plasma_ontology#laser_huygens_surface_positions"/>
        <rdfs:domain rdf:resource="http://www.semanticweb.org/afshar87/ontologies/2024/3/Laser-Plasma_ontology#Laser"/>
        <rdfs:range rdf:resource="http://www.w3.org/2001/XMLSchema#integer"/>
    </owl:DatatypeProperty>
    


    <!-- http://www.semanticweb.org/afshar87/ontologies/2024/3/Laser-Plasma_ontology#huygens_surface_positions_zmin -->

    <owl:DatatypeProperty rdf:about="http://www.semanticweb.org/afshar87/ontologies/2024/3/Laser-Plasma_ontology#huygens_surface_positions_zmin">
        <rdfs:subPropertyOf rdf:resource="http://www.semanticweb.org/afshar87/ontologies/2024/3/Laser-Plasma_ontology#laser_huygens_surface_positions"/>
        <rdfs:domain rdf:resource="http://www.semanticweb.org/afshar87/ontologies/2024/3/Laser-Plasma_ontology#Laser"/>
        <rdfs:range rdf:resource="http://www.w3.org/2001/XMLSchema#integer"/>
    </owl:DatatypeProperty>
    


    <!-- http://www.semanticweb.org/afshar87/ontologies/2024/3/Laser-Plasma_ontology#ionization_degree -->

    <owl:DatatypeProperty rdf:about="http://www.semanticweb.org/afshar87/ontologies/2024/3/Laser-Plasma_ontology#ionization_degree">
        <rdfs:subPropertyOf rdf:resource="http://www.semanticweb.org/afshar87/ontologies/2024/3/Laser-Plasma_ontology#Ionization"/>
        <rdfs:domain rdf:resource="http://www.semanticweb.org/afshar87/ontologies/2024/3/Laser-Plasma_ontology#Ionization"/>
        <rdfs:range rdf:resource="http://www.w3.org/2001/XMLSchema#float"/>
        <rdfs:comment>the (average) number of electrons removed per ion (atom) which  is :

  Z - bound_electrons, (look at data property : ionization_number_of_bound_electrons) where Z is  atomic number (number of protonsin the nucleus of a atom of a element).</rdfs:comment>
    </owl:DatatypeProperty>
    


    <!-- http://www.semanticweb.org/afshar87/ontologies/2024/3/Laser-Plasma_ontology#ionization_models -->

    <owl:DatatypeProperty rdf:about="http://www.semanticweb.org/afshar87/ontologies/2024/3/Laser-Plasma_ontology#ionization_models">
        <rdfs:subPropertyOf rdf:resource="http://www.semanticweb.org/afshar87/ontologies/2024/3/Laser-Plasma_ontology#Ionization"/>
        <rdfs:domain rdf:resource="http://www.semanticweb.org/afshar87/ontologies/2024/3/Laser-Plasma_ontology#Plasma"/>
        <rdfs:range rdf:resource="http://www.w3.org/2001/XMLSchema#string"/>
        <rdfs:comment>ionization mechanisms applied to the species or element in the simulation.</rdfs:comment>
    </owl:DatatypeProperty>
    


    <!-- http://www.semanticweb.org/afshar87/ontologies/2024/3/Laser-Plasma_ontology#ionization_number_of_bound_electrons -->

    <owl:DatatypeProperty rdf:about="http://www.semanticweb.org/afshar87/ontologies/2024/3/Laser-Plasma_ontology#ionization_number_of_bound_electrons">
        <rdfs:subPropertyOf rdf:resource="http://www.semanticweb.org/afshar87/ontologies/2024/3/Laser-Plasma_ontology#Ionization"/>
        <rdfs:domain rdf:resource="http://www.semanticweb.org/afshar87/ontologies/2024/3/Laser-Plasma_ontology#Simulation"/>
        <rdfs:range rdf:resource="http://www.w3.org/2001/XMLSchema#integer"/>
        <rdfs:comment>the initial number of bound electrons, the charge state is Z - bound_electrons, e.g. bound_electrons for carbon could be 6 to 0.</rdfs:comment>
    </owl:DatatypeProperty>
    


    <!-- http://www.semanticweb.org/afshar87/ontologies/2024/3/Laser-Plasma_ontology#ionization_species -->

    <owl:DatatypeProperty rdf:about="http://www.semanticweb.org/afshar87/ontologies/2024/3/Laser-Plasma_ontology#ionization_species">
        <rdfs:subPropertyOf rdf:resource="http://www.semanticweb.org/afshar87/ontologies/2024/3/Laser-Plasma_ontology#Ionization"/>
        <rdfs:domain rdf:resource="http://www.semanticweb.org/afshar87/ontologies/2024/3/Laser-Plasma_ontology#Plasma"/>
        <rdfs:range rdf:resource="http://www.w3.org/2001/XMLSchema#string"/>
        <rdfs:comment>which species does the ionization</rdfs:comment>
    </owl:DatatypeProperty>
    


    <!-- http://www.semanticweb.org/afshar87/ontologies/2024/3/Laser-Plasma_ontology#laser_amplitude -->

    <owl:DatatypeProperty rdf:about="http://www.semanticweb.org/afshar87/ontologies/2024/3/Laser-Plasma_ontology#laser_amplitude">
        <rdfs:subPropertyOf rdf:resource="http://www.semanticweb.org/afshar87/ontologies/2024/3/Laser-Plasma_ontology#laser_pulse"/>
        <rdfs:domain rdf:resource="http://www.semanticweb.org/afshar87/ontologies/2024/3/Laser-Plasma_ontology#Laser"/>
        <rdfs:range rdf:resource="http://www.w3.org/2001/XMLSchema#double"/>
        <rdfs:comment>The maximum value (amplitude), E_max, of the electric field (E) of the laser pulse.</rdfs:comment>
    </owl:DatatypeProperty>
    


    <!-- http://www.semanticweb.org/afshar87/ontologies/2024/3/Laser-Plasma_ontology#laser_beam -->

    <owl:DatatypeProperty rdf:about="http://www.semanticweb.org/afshar87/ontologies/2024/3/Laser-Plasma_ontology#laser_beam">
        <rdfs:subPropertyOf rdf:resource="http://www.semanticweb.org/afshar87/ontologies/2024/3/Laser-Plasma_ontology#laser_properties"/>
        <rdfs:domain rdf:resource="http://www.semanticweb.org/afshar87/ontologies/2024/3/Laser-Plasma_ontology#Laser"/>
    </owl:DatatypeProperty>
    


    <!-- http://www.semanticweb.org/afshar87/ontologies/2024/3/Laser-Plasma_ontology#laser_beam_shape -->

    <owl:DatatypeProperty rdf:about="http://www.semanticweb.org/afshar87/ontologies/2024/3/Laser-Plasma_ontology#laser_beam_shape">
        <rdfs:subPropertyOf rdf:resource="http://www.semanticweb.org/afshar87/ontologies/2024/3/Laser-Plasma_ontology#laser_beam"/>
        <rdfs:domain rdf:resource="http://www.semanticweb.org/afshar87/ontologies/2024/3/Laser-Plasma_ontology#Laser"/>
        <rdfs:range rdf:resource="http://www.w3.org/2001/XMLSchema#string"/>
        <rdfs:comment>The mode of a laser beam such as Gaussian beam or a Laguerre-Gaussian mode.</rdfs:comment>
    </owl:DatatypeProperty>
    


    <!-- http://www.semanticweb.org/afshar87/ontologies/2024/3/Laser-Plasma_ontology#laser_beam_waist -->

    <owl:DatatypeProperty rdf:about="http://www.semanticweb.org/afshar87/ontologies/2024/3/Laser-Plasma_ontology#laser_beam_waist">
        <rdfs:subPropertyOf rdf:resource="http://www.semanticweb.org/afshar87/ontologies/2024/3/Laser-Plasma_ontology#laser_beam"/>
        <rdfs:domain rdf:resource="http://www.semanticweb.org/afshar87/ontologies/2024/3/Laser-Plasma_ontology#Laser"/>
        <rdfs:range rdf:resource="http://www.w3.org/2001/XMLSchema#double"/>
        <rdfs:comment>The beam waist w0 is a fundamental parameter of a Gaussian beam and is defined as the radius at which:

-  the electric field amplitude drops to  ( 1/e ) of its maximum value  on-axis
- and the beam width w(z) is the smallest (the intensity on-axis (r = 0) is the largest).  

Key Characteristics of the Beam Waist:

1. Beam Waist Radius w0:
   - It represents the minimum spot size of the beam.
   - At this point, the beam is most tightly focused.</rdfs:comment>
    </owl:DatatypeProperty>
    


    <!-- http://www.semanticweb.org/afshar87/ontologies/2024/3/Laser-Plasma_ontology#laser_energy -->

    <owl:DatatypeProperty rdf:about="http://www.semanticweb.org/afshar87/ontologies/2024/3/Laser-Plasma_ontology#laser_energy">
        <rdfs:subPropertyOf rdf:resource="http://www.semanticweb.org/afshar87/ontologies/2024/3/Laser-Plasma_ontology#laser_pulse"/>
        <rdfs:domain rdf:resource="http://www.semanticweb.org/afshar87/ontologies/2024/3/Laser-Plasma_ontology#Laser"/>
        <rdfs:range rdf:resource="http://www.w3.org/2001/XMLSchema#double"/>
        <rdfs:comment>the total amount of energy delivered by a single laser pulse.  

 
EXPERIMENTALLY:
In experiments, measuring laser energy often involves using a laser power meter which measures the average power output of the laser beam. However, since pulsed lasers deliver energy in bursts, we need to account for the pulse repetition rate (Hz) to calculate the energy per pulse. Formula:

laser_energyPulse (J) = Average Power (W) / Repetition Rate (Hz)


THEORITICALLY:
 the energy can be calculated by integrating:

- the squared electric field (E) of the pulse over a specific volume (V) and time interval (t):

LaserEnergyPulse = âˆ« (Îµâ‚€ * E(t, x, y, z)Â²)dV dt

Here, Îµâ‚€ represents the permittivity of free space, a constant value. E(t, x, y, z) represents the electric field as a function of time (t) and position (x, y, z) within the volume (V). The integration calculates the total energy content within the defined volume and time window.

- Poynting vector (S), which describes the energy flux (energy flow per unit area per unit time) of an electromagnetic field. The time integral of the Poynting vector over a specific area (A) through which the pulse propagates gives the total energy:

LaserEnergyPulse = âˆ« S(t, A) dt

 Here, S(t, A) represents the Poynting vector as a function of time (t) across the area (A). The integration calculates the total energy that flows through the defined area over the pulse duration.</rdfs:comment>
    </owl:DatatypeProperty>
    


    <!-- http://www.semanticweb.org/afshar87/ontologies/2024/3/Laser-Plasma_ontology#laser_focus_position -->

    <owl:DatatypeProperty rdf:about="http://www.semanticweb.org/afshar87/ontologies/2024/3/Laser-Plasma_ontology#laser_focus_position">
        <rdfs:subPropertyOf rdf:resource="http://www.semanticweb.org/afshar87/ontologies/2024/3/Laser-Plasma_ontology#laser_beam"/>
        <rdfs:domain rdf:resource="http://www.semanticweb.org/afshar87/ontologies/2024/3/Laser-Plasma_ontology#Laser"/>
        <rdfs:range rdf:resource="http://www.w3.org/2001/XMLSchema#double"/>
        <rdfs:comment>laser focus position coordinates</rdfs:comment>
    </owl:DatatypeProperty>
    


    <!-- http://www.semanticweb.org/afshar87/ontologies/2024/3/Laser-Plasma_ontology#laser_focus_position_x -->

    <owl:DatatypeProperty rdf:about="http://www.semanticweb.org/afshar87/ontologies/2024/3/Laser-Plasma_ontology#laser_focus_position_x">
        <rdfs:subPropertyOf rdf:resource="http://www.semanticweb.org/afshar87/ontologies/2024/3/Laser-Plasma_ontology#laser_focus_position"/>
        <rdfs:domain rdf:resource="http://www.semanticweb.org/afshar87/ontologies/2024/3/Laser-Plasma_ontology#Laser"/>
        <rdfs:range rdf:resource="http://www.w3.org/2001/XMLSchema#double"/>
        <rdfs:comment>laser focus position in x direction</rdfs:comment>
    </owl:DatatypeProperty>
    


    <!-- http://www.semanticweb.org/afshar87/ontologies/2024/3/Laser-Plasma_ontology#laser_focus_position_y -->

    <owl:DatatypeProperty rdf:about="http://www.semanticweb.org/afshar87/ontologies/2024/3/Laser-Plasma_ontology#laser_focus_position_y">
        <rdfs:subPropertyOf rdf:resource="http://www.semanticweb.org/afshar87/ontologies/2024/3/Laser-Plasma_ontology#laser_focus_position"/>
        <rdfs:domain rdf:resource="http://www.semanticweb.org/afshar87/ontologies/2024/3/Laser-Plasma_ontology#Laser"/>
        <rdfs:range rdf:resource="http://www.w3.org/2001/XMLSchema#double"/>
        <rdfs:comment>laser focus position in y direction</rdfs:comment>
    </owl:DatatypeProperty>
    


    <!-- http://www.semanticweb.org/afshar87/ontologies/2024/3/Laser-Plasma_ontology#laser_focus_position_z -->

    <owl:DatatypeProperty rdf:about="http://www.semanticweb.org/afshar87/ontologies/2024/3/Laser-Plasma_ontology#laser_focus_position_z">
        <rdfs:subPropertyOf rdf:resource="http://www.semanticweb.org/afshar87/ontologies/2024/3/Laser-Plasma_ontology#laser_focus_position"/>
        <rdfs:domain rdf:resource="http://www.semanticweb.org/afshar87/ontologies/2024/3/Laser-Plasma_ontology#Laser"/>
        <rdfs:range rdf:resource="http://www.w3.org/2001/XMLSchema#double"/>
        <rdfs:comment></rdfs:comment>
        <rdfs:comment>laser focus position in z direction</rdfs:comment>
    </owl:DatatypeProperty>
    


    <!-- http://www.semanticweb.org/afshar87/ontologies/2024/3/Laser-Plasma_ontology#laser_frequency -->

    <owl:DatatypeProperty rdf:about="http://www.semanticweb.org/afshar87/ontologies/2024/3/Laser-Plasma_ontology#laser_frequency">
        <rdfs:subPropertyOf rdf:resource="http://www.semanticweb.org/afshar87/ontologies/2024/3/Laser-Plasma_ontology#laser_beam"/>
        <rdfs:domain rdf:resource="http://www.semanticweb.org/afshar87/ontologies/2024/3/Laser-Plasma_ontology#Laser"/>
        <rdfs:range rdf:resource="http://www.w3.org/2001/XMLSchema#double"/>
        <rdfs:comment>the frequency of a laser pulse. It related to the laser wavelength (Î») through the speed of light (c) by the following equation:

laser_frequency (Hz) = c / Î» (meters)</rdfs:comment>
    </owl:DatatypeProperty>
    


    <!-- http://www.semanticweb.org/afshar87/ontologies/2024/3/Laser-Plasma_ontology#laser_huygens_surface_positions -->

    <owl:DatatypeProperty rdf:about="http://www.semanticweb.org/afshar87/ontologies/2024/3/Laser-Plasma_ontology#laser_huygens_surface_positions">
        <rdfs:subPropertyOf rdf:resource="http://www.semanticweb.org/afshar87/ontologies/2024/3/Laser-Plasma_ontology#laser_beam"/>
    </owl:DatatypeProperty>
    


    <!-- http://www.semanticweb.org/afshar87/ontologies/2024/3/Laser-Plasma_ontology#laser_meanPower -->

    <owl:DatatypeProperty rdf:about="http://www.semanticweb.org/afshar87/ontologies/2024/3/Laser-Plasma_ontology#laser_meanPower">
        <rdfs:subPropertyOf rdf:resource="http://www.semanticweb.org/afshar87/ontologies/2024/3/Laser-Plasma_ontology#laser_beam"/>
        <rdfs:domain rdf:resource="http://www.semanticweb.org/afshar87/ontologies/2024/3/Laser-Plasma_ontology#Laser"/>
        <rdfs:range rdf:resource="http://www.w3.org/2001/XMLSchema#double"/>
        <rdfs:comment>The total energy output of a laser per unit time, averaged over a longer period that includes many pulses where 

Average Power = Peak Power  *   pulse duration *  pulse repetition rate (Hertz)</rdfs:comment>
    </owl:DatatypeProperty>
    


    <!-- http://www.semanticweb.org/afshar87/ontologies/2024/3/Laser-Plasma_ontology#laser_omega -->

    <owl:DatatypeProperty rdf:about="http://www.semanticweb.org/afshar87/ontologies/2024/3/Laser-Plasma_ontology#laser_omega">
        <rdfs:subPropertyOf rdf:resource="http://www.semanticweb.org/afshar87/ontologies/2024/3/Laser-Plasma_ontology#laser_beam"/>
        <rdfs:domain rdf:resource="http://www.semanticweb.org/afshar87/ontologies/2024/3/Laser-Plasma_ontology#Laser"/>
        <rdfs:range rdf:resource="http://www.w3.org/2001/XMLSchema#double"/>
        <rdfs:comment>Angular frequency (Ï‰) of a laser pulse. it represents the frequency of a periodic motion expressed in radians per second (rad/s).

In the context of a laser pulse, the angular frequency relates to the laser&apos;s frequency (f) through the following relationship:

Ï‰ (rad/s) = 2 * Ï€ * f (Hz)

Here, Ï€ (pi) is a mathematical constant approximately equal to 3.14159.</rdfs:comment>
    </owl:DatatypeProperty>
    


    <!-- http://www.semanticweb.org/afshar87/ontologies/2024/3/Laser-Plasma_ontology#laser_peakPower -->

    <owl:DatatypeProperty rdf:about="http://www.semanticweb.org/afshar87/ontologies/2024/3/Laser-Plasma_ontology#laser_peakPower">
        <rdfs:subPropertyOf rdf:resource="http://www.semanticweb.org/afshar87/ontologies/2024/3/Laser-Plasma_ontology#laser_pulse"/>
        <rdfs:domain rdf:resource="http://www.semanticweb.org/afshar87/ontologies/2024/3/Laser-Plasma_ontology#Laser"/>
        <rdfs:range rdf:resource="http://www.w3.org/2001/XMLSchema#double"/>
        <rdfs:comment>The highest instantaneous power delivered by a single laser puls. it is often related to other laser pulse properties like pulse duration (Ï„) through the following equation:

Peak Power (W) = Energy per Pulse (J) / Pulse Duration (s)</rdfs:comment>
    </owl:DatatypeProperty>
    


    <!-- http://www.semanticweb.org/afshar87/ontologies/2024/3/Laser-Plasma_ontology#laser_peak_intensity -->

    <owl:DatatypeProperty rdf:about="http://www.semanticweb.org/afshar87/ontologies/2024/3/Laser-Plasma_ontology#laser_peak_intensity">
        <rdfs:subPropertyOf rdf:resource="http://www.semanticweb.org/afshar87/ontologies/2024/3/Laser-Plasma_ontology#laser_pulse"/>
        <rdfs:domain rdf:resource="http://www.semanticweb.org/afshar87/ontologies/2024/3/Laser-Plasma_ontology#Laser"/>
        <rdfs:range rdf:resource="http://www.w3.org/2001/XMLSchema#double"/>
        <rdfs:comment>Peak Intensity (I_peak) refers to the maximum intensity (power per unit area) of the laser pulse. It&apos;s calculated based on the electric field amplitude (E_max) and the wave impedance of free space:

I_peak = (1/2) * Îµâ‚€ * c * E_max^2

Here, Îµâ‚€ is the permittivity of free space, and c is the speed of light in vacuum.</rdfs:comment>
    </owl:DatatypeProperty>
    


    <!-- http://www.semanticweb.org/afshar87/ontologies/2024/3/Laser-Plasma_ontology#laser_polarization -->

    <owl:DatatypeProperty rdf:about="http://www.semanticweb.org/afshar87/ontologies/2024/3/Laser-Plasma_ontology#laser_polarization">
        <rdfs:subPropertyOf rdf:resource="http://www.semanticweb.org/afshar87/ontologies/2024/3/Laser-Plasma_ontology#laser_beam"/>
    </owl:DatatypeProperty>
    


    <!-- http://www.semanticweb.org/afshar87/ontologies/2024/3/Laser-Plasma_ontology#laser_polarization_circular -->

    <owl:DatatypeProperty rdf:about="http://www.semanticweb.org/afshar87/ontologies/2024/3/Laser-Plasma_ontology#laser_polarization_circular">
        <rdfs:subPropertyOf rdf:resource="http://www.semanticweb.org/afshar87/ontologies/2024/3/Laser-Plasma_ontology#laser_polarization_type"/>
        <rdfs:domain rdf:resource="http://www.semanticweb.org/afshar87/ontologies/2024/3/Laser-Plasma_ontology#Laser"/>
        <rdfs:range rdf:resource="http://www.w3.org/2001/XMLSchema#string"/>
    </owl:DatatypeProperty>
    


    <!-- http://www.semanticweb.org/afshar87/ontologies/2024/3/Laser-Plasma_ontology#laser_polarization_direction -->

    <owl:DatatypeProperty rdf:about="http://www.semanticweb.org/afshar87/ontologies/2024/3/Laser-Plasma_ontology#laser_polarization_direction">
        <rdfs:subPropertyOf rdf:resource="http://www.semanticweb.org/afshar87/ontologies/2024/3/Laser-Plasma_ontology#laser_polarization"/>
    </owl:DatatypeProperty>
    


    <!-- http://www.semanticweb.org/afshar87/ontologies/2024/3/Laser-Plasma_ontology#laser_polarization_direction_x -->

    <owl:DatatypeProperty rdf:about="http://www.semanticweb.org/afshar87/ontologies/2024/3/Laser-Plasma_ontology#laser_polarization_direction_x">
        <rdfs:subPropertyOf rdf:resource="http://www.semanticweb.org/afshar87/ontologies/2024/3/Laser-Plasma_ontology#laser_polarization_direction"/>
        <rdfs:domain rdf:resource="http://www.semanticweb.org/afshar87/ontologies/2024/3/Laser-Plasma_ontology#Laser"/>
        <rdfs:range rdf:resource="http://www.w3.org/2001/XMLSchema#boolean"/>
    </owl:DatatypeProperty>
    


    <!-- http://www.semanticweb.org/afshar87/ontologies/2024/3/Laser-Plasma_ontology#laser_polarization_direction_y -->

    <owl:DatatypeProperty rdf:about="http://www.semanticweb.org/afshar87/ontologies/2024/3/Laser-Plasma_ontology#laser_polarization_direction_y">
        <rdfs:subPropertyOf rdf:resource="http://www.semanticweb.org/afshar87/ontologies/2024/3/Laser-Plasma_ontology#laser_polarization_direction"/>
        <rdfs:domain rdf:resource="http://www.semanticweb.org/afshar87/ontologies/2024/3/Laser-Plasma_ontology#Laser"/>
        <rdfs:range rdf:resource="http://www.w3.org/2001/XMLSchema#boolean"/>
    </owl:DatatypeProperty>
    


    <!-- http://www.semanticweb.org/afshar87/ontologies/2024/3/Laser-Plasma_ontology#laser_polarization_direction_z -->

    <owl:DatatypeProperty rdf:about="http://www.semanticweb.org/afshar87/ontologies/2024/3/Laser-Plasma_ontology#laser_polarization_direction_z">
        <rdfs:subPropertyOf rdf:resource="http://www.semanticweb.org/afshar87/ontologies/2024/3/Laser-Plasma_ontology#laser_polarization_direction"/>
        <rdfs:domain rdf:resource="http://www.semanticweb.org/afshar87/ontologies/2024/3/Laser-Plasma_ontology#Laser"/>
        <rdfs:range rdf:resource="http://www.w3.org/2001/XMLSchema#boolean"/>
    </owl:DatatypeProperty>
    


    <!-- http://www.semanticweb.org/afshar87/ontologies/2024/3/Laser-Plasma_ontology#laser_polarization_elliptical -->

    <owl:DatatypeProperty rdf:about="http://www.semanticweb.org/afshar87/ontologies/2024/3/Laser-Plasma_ontology#laser_polarization_elliptical">
        <rdfs:subPropertyOf rdf:resource="http://www.semanticweb.org/afshar87/ontologies/2024/3/Laser-Plasma_ontology#laser_polarization_type"/>
        <rdfs:domain rdf:resource="http://www.semanticweb.org/afshar87/ontologies/2024/3/Laser-Plasma_ontology#Laser"/>
        <rdfs:range rdf:resource="http://www.w3.org/2001/XMLSchema#string"/>
    </owl:DatatypeProperty>
    


    <!-- http://www.semanticweb.org/afshar87/ontologies/2024/3/Laser-Plasma_ontology#laser_polarization_linear -->

    <owl:DatatypeProperty rdf:about="http://www.semanticweb.org/afshar87/ontologies/2024/3/Laser-Plasma_ontology#laser_polarization_linear">
        <rdfs:subPropertyOf rdf:resource="http://www.semanticweb.org/afshar87/ontologies/2024/3/Laser-Plasma_ontology#laser_polarization_type"/>
        <rdfs:domain rdf:resource="http://www.semanticweb.org/afshar87/ontologies/2024/3/Laser-Plasma_ontology#Laser"/>
        <rdfs:range rdf:resource="http://www.w3.org/2001/XMLSchema#string"/>
    </owl:DatatypeProperty>
    


    <!-- http://www.semanticweb.org/afshar87/ontologies/2024/3/Laser-Plasma_ontology#laser_polarization_type -->

    <owl:DatatypeProperty rdf:about="http://www.semanticweb.org/afshar87/ontologies/2024/3/Laser-Plasma_ontology#laser_polarization_type">
        <rdfs:subPropertyOf rdf:resource="http://www.semanticweb.org/afshar87/ontologies/2024/3/Laser-Plasma_ontology#laser_polarization"/>
        <rdfs:domain rdf:resource="http://www.semanticweb.org/afshar87/ontologies/2024/3/Laser-Plasma_ontology#Laser"/>
        <rdfs:range rdf:resource="http://www.w3.org/2001/XMLSchema#string"/>
        <rdfs:comment>Polarization state of the laser pulse (e.g., linear, circular, elliptical)</rdfs:comment>
    </owl:DatatypeProperty>
    


    <!-- http://www.semanticweb.org/afshar87/ontologies/2024/3/Laser-Plasma_ontology#laser_propagation_direction -->

    <owl:DatatypeProperty rdf:about="http://www.semanticweb.org/afshar87/ontologies/2024/3/Laser-Plasma_ontology#laser_propagation_direction">
        <rdfs:subPropertyOf rdf:resource="http://www.semanticweb.org/afshar87/ontologies/2024/3/Laser-Plasma_ontology#laser_beam"/>
        <rdfs:domain rdf:resource="http://www.semanticweb.org/afshar87/ontologies/2024/3/Laser-Plasma_ontology#Laser"/>
    </owl:DatatypeProperty>
    


    <!-- http://www.semanticweb.org/afshar87/ontologies/2024/3/Laser-Plasma_ontology#laser_propagation_direction_x -->

    <owl:DatatypeProperty rdf:about="http://www.semanticweb.org/afshar87/ontologies/2024/3/Laser-Plasma_ontology#laser_propagation_direction_x">
        <rdfs:subPropertyOf rdf:resource="http://www.semanticweb.org/afshar87/ontologies/2024/3/Laser-Plasma_ontology#laser_propagation_direction"/>
        <rdfs:domain rdf:resource="http://www.semanticweb.org/afshar87/ontologies/2024/3/Laser-Plasma_ontology#Laser"/>
        <rdfs:range rdf:resource="http://www.w3.org/2001/XMLSchema#boolean"/>
    </owl:DatatypeProperty>
    


    <!-- http://www.semanticweb.org/afshar87/ontologies/2024/3/Laser-Plasma_ontology#laser_propagation_direction_y -->

    <owl:DatatypeProperty rdf:about="http://www.semanticweb.org/afshar87/ontologies/2024/3/Laser-Plasma_ontology#laser_propagation_direction_y">
        <rdfs:subPropertyOf rdf:resource="http://www.semanticweb.org/afshar87/ontologies/2024/3/Laser-Plasma_ontology#laser_propagation_direction"/>
        <rdfs:domain rdf:resource="http://www.semanticweb.org/afshar87/ontologies/2024/3/Laser-Plasma_ontology#Laser"/>
        <rdfs:range rdf:resource="http://www.w3.org/2001/XMLSchema#boolean"/>
    </owl:DatatypeProperty>
    


    <!-- http://www.semanticweb.org/afshar87/ontologies/2024/3/Laser-Plasma_ontology#laser_propagation_direction_z -->

    <owl:DatatypeProperty rdf:about="http://www.semanticweb.org/afshar87/ontologies/2024/3/Laser-Plasma_ontology#laser_propagation_direction_z">
        <rdfs:subPropertyOf rdf:resource="http://www.semanticweb.org/afshar87/ontologies/2024/3/Laser-Plasma_ontology#laser_propagation_direction"/>
        <rdfs:domain rdf:resource="http://www.semanticweb.org/afshar87/ontologies/2024/3/Laser-Plasma_ontology#Laser"/>
        <rdfs:range rdf:resource="http://www.w3.org/2001/XMLSchema#boolean"/>
    </owl:DatatypeProperty>
    


    <!-- http://www.semanticweb.org/afshar87/ontologies/2024/3/Laser-Plasma_ontology#laser_properties -->

    <owl:DatatypeProperty rdf:about="http://www.semanticweb.org/afshar87/ontologies/2024/3/Laser-Plasma_ontology#laser_properties"/>
    


    <!-- http://www.semanticweb.org/afshar87/ontologies/2024/3/Laser-Plasma_ontology#laser_pulse -->

    <owl:DatatypeProperty rdf:about="http://www.semanticweb.org/afshar87/ontologies/2024/3/Laser-Plasma_ontology#laser_pulse">
        <rdfs:subPropertyOf rdf:resource="http://www.semanticweb.org/afshar87/ontologies/2024/3/Laser-Plasma_ontology#laser_properties"/>
    </owl:DatatypeProperty>
    


    <!-- http://www.semanticweb.org/afshar87/ontologies/2024/3/Laser-Plasma_ontology#laser_pulse_duration_FWHM -->

    <owl:DatatypeProperty rdf:about="http://www.semanticweb.org/afshar87/ontologies/2024/3/Laser-Plasma_ontology#laser_pulse_duration_FWHM">
        <rdfs:subPropertyOf rdf:resource="http://www.semanticweb.org/afshar87/ontologies/2024/3/Laser-Plasma_ontology#laser_pulse"/>
        <rdfs:domain rdf:resource="http://www.semanticweb.org/afshar87/ontologies/2024/3/Laser-Plasma_ontology#Laser"/>
        <rdfs:range rdf:resource="http://www.w3.org/2001/XMLSchema#double"/>
        <rdfs:comment>Pulse duration, commonly referred to as the Full Width at Half Maximum (FWHM), is a measure of the temporal length of a laser pulse. Specifically, the FWHM is defined as the duration over which the pulse&apos;s intensity is at least half of its maximum value.</rdfs:comment>
    </owl:DatatypeProperty>
    


    <!-- http://www.semanticweb.org/afshar87/ontologies/2024/3/Laser-Plasma_ontology#laser_pulse_multiplicator -->

    <owl:DatatypeProperty rdf:about="http://www.semanticweb.org/afshar87/ontologies/2024/3/Laser-Plasma_ontology#laser_pulse_multiplicator">
        <rdfs:subPropertyOf rdf:resource="http://www.semanticweb.org/afshar87/ontologies/2024/3/Laser-Plasma_ontology#laser_pulse"/>
        <rdfs:domain rdf:resource="http://www.semanticweb.org/afshar87/ontologies/2024/3/Laser-Plasma_ontology#Laser"/>
        <rdfs:range rdf:resource="http://www.w3.org/2001/XMLSchema#integer"/>
        <rdfs:comment>The laser pulse will be initialized laser_pulse_multiplicator times of the pulse_duration.</rdfs:comment>
    </owl:DatatypeProperty>
    


    <!-- http://www.semanticweb.org/afshar87/ontologies/2024/3/Laser-Plasma_ontology#laser_repetition_rate -->

    <owl:DatatypeProperty rdf:about="http://www.semanticweb.org/afshar87/ontologies/2024/3/Laser-Plasma_ontology#laser_repetition_rate">
        <rdfs:subPropertyOf rdf:resource="http://www.semanticweb.org/afshar87/ontologies/2024/3/Laser-Plasma_ontology#laser_pulse"/>
        <rdfs:domain rdf:resource="http://www.semanticweb.org/afshar87/ontologies/2024/3/Laser-Plasma_ontology#Laser"/>
        <rdfs:range rdf:resource="http://www.w3.org/2001/XMLSchema#float"/>
        <rdfs:comment>The laser repetition rate refers to the number of pulses per second a laser pulse is emitted  which  is typically measured in Hertz (Hz).</rdfs:comment>
    </owl:DatatypeProperty>
    


    <!-- http://www.semanticweb.org/afshar87/ontologies/2024/3/Laser-Plasma_ontology#laser_temporal_phase -->

    <owl:DatatypeProperty rdf:about="http://www.semanticweb.org/afshar87/ontologies/2024/3/Laser-Plasma_ontology#laser_temporal_phase">
        <rdfs:subPropertyOf rdf:resource="http://www.semanticweb.org/afshar87/ontologies/2024/3/Laser-Plasma_ontology#laser_pulse"/>
        <rdfs:domain rdf:resource="http://www.semanticweb.org/afshar87/ontologies/2024/3/Laser-Plasma_ontology#Laser"/>
        <rdfs:range rdf:resource="http://www.w3.org/2001/XMLSchema#float"/>
        <rdfs:comment>The Carrier-Envelope Phase (CEP) is a crucial parameter in ultrafast optics, especially in the context of femtosecond laser pulses. Here is a detailed explanation:

Definition:
The Carrier-Envelope Phase (CEP) is the phase difference between the peak of the carrier wave and the peak of the pulse envelope. In other words, it describes the offset between the oscillations of the electric field (the carrier wave) and the maximum of the pulse envelope in a laser pulse.

 Mathematical Representation:
The electric field E(t) of a laser pulse can be represented as:
 E(t) = E0(t) cos(Ï‰0t +Ï•)
where:
-  E0(t)  is the pulse envelope.
- Ï‰0 is the carrier frequency.
- Ï• is the carrier-envelope phase.
In this equation, ðœ™ determines the phase shift between the peak of the envelope E0(ð‘¡)
and the carrier waveâ€™s oscillations.</rdfs:comment>
    </owl:DatatypeProperty>
    


    <!-- http://www.semanticweb.org/afshar87/ontologies/2024/3/Laser-Plasma_ontology#laser_wavelength -->

    <owl:DatatypeProperty rdf:about="http://www.semanticweb.org/afshar87/ontologies/2024/3/Laser-Plasma_ontology#laser_wavelength">
        <rdfs:subPropertyOf rdf:resource="http://www.semanticweb.org/afshar87/ontologies/2024/3/Laser-Plasma_ontology#laser_beam"/>
        <rdfs:domain rdf:resource="http://www.semanticweb.org/afshar87/ontologies/2024/3/Laser-Plasma_ontology#Laser"/>
        <rdfs:range rdf:resource="http://www.w3.org/2001/XMLSchema#double"/>
        <rdfs:comment>The central  wavelength of a laser pulse in a vacuum. It related to the laser laser_frequency through the speed of light (c) by the following equation:

 Î» (meters) = c /  laser_frequency (Hz)</rdfs:comment>
    </owl:DatatypeProperty>
    


    <!-- http://www.semanticweb.org/afshar87/ontologies/2024/3/Laser-Plasma_ontology#macroparticle -->

    <owl:DatatypeProperty rdf:about="http://www.semanticweb.org/afshar87/ontologies/2024/3/Laser-Plasma_ontology#macroparticle">
        <rdfs:subPropertyOf rdf:resource="http://www.semanticweb.org/afshar87/ontologies/2024/3/Laser-Plasma_ontology#simulation_property"/>
        <rdfs:comment>Represents a macroparticle in a simulation.</rdfs:comment>
    </owl:DatatypeProperty>
    


    <!-- http://www.semanticweb.org/afshar87/ontologies/2024/3/Laser-Plasma_ontology#macroparticle_attributes -->

    <owl:DatatypeProperty rdf:about="http://www.semanticweb.org/afshar87/ontologies/2024/3/Laser-Plasma_ontology#macroparticle_attributes">
        <rdfs:subPropertyOf rdf:resource="http://www.semanticweb.org/afshar87/ontologies/2024/3/Laser-Plasma_ontology#macroparticle"/>
        <rdfs:domain rdf:resource="http://www.semanticweb.org/afshar87/ontologies/2024/3/Laser-Plasma_ontology#Macroparticle"/>
        <rdfs:range rdf:resource="http://www.w3.org/2001/XMLSchema#string"/>
        <owl:backwardCompatibleWith>the attribute NAME (reference) of a macroparticle</owl:backwardCompatibleWith>
    </owl:DatatypeProperty>
    


    <!-- http://www.semanticweb.org/afshar87/ontologies/2024/3/Laser-Plasma_ontology#macroparticle_attributes_momentum -->

    <owl:DatatypeProperty rdf:about="http://www.semanticweb.org/afshar87/ontologies/2024/3/Laser-Plasma_ontology#macroparticle_attributes_momentum">
        <rdfs:subPropertyOf rdf:resource="http://www.semanticweb.org/afshar87/ontologies/2024/3/Laser-Plasma_ontology#macroparticle_attributes"/>
        <rdfs:domain rdf:resource="http://www.semanticweb.org/afshar87/ontologies/2024/3/Laser-Plasma_ontology#Macroparticle"/>
        <rdfs:range rdf:resource="http://www.w3.org/2001/XMLSchema#string"/>
        <rdfs:comment>the attribute NAME that refer to the momentum of a macroparticle. It represents the name or reference to the PIC code for the attribute. However, the actual data type that represents can be a numerical value like a float or an integer in the code.</rdfs:comment>
    </owl:DatatypeProperty>
    


    <!-- http://www.semanticweb.org/afshar87/ontologies/2024/3/Laser-Plasma_ontology#macroparticle_attributes_position -->

    <owl:DatatypeProperty rdf:about="http://www.semanticweb.org/afshar87/ontologies/2024/3/Laser-Plasma_ontology#macroparticle_attributes_position">
        <rdfs:subPropertyOf rdf:resource="http://www.semanticweb.org/afshar87/ontologies/2024/3/Laser-Plasma_ontology#macroparticle_attributes"/>
        <rdfs:domain rdf:resource="http://www.semanticweb.org/afshar87/ontologies/2024/3/Laser-Plasma_ontology#Macroparticle"/>
        <rdfs:range rdf:resource="http://www.w3.org/2001/XMLSchema#string"/>
        <rdfs:comment>the attribute NAME that refer to the position of a macroparticle in the simulation space. It refers to a template (specific class in PIC code) to represent position.</rdfs:comment>
    </owl:DatatypeProperty>
    


    <!-- http://www.semanticweb.org/afshar87/ontologies/2024/3/Laser-Plasma_ontology#macroparticle_attributes_weighting -->

    <owl:DatatypeProperty rdf:about="http://www.semanticweb.org/afshar87/ontologies/2024/3/Laser-Plasma_ontology#macroparticle_attributes_weighting">
        <rdfs:subPropertyOf rdf:resource="http://www.semanticweb.org/afshar87/ontologies/2024/3/Laser-Plasma_ontology#macroparticle_attributes"/>
        <rdfs:domain rdf:resource="http://www.semanticweb.org/afshar87/ontologies/2024/3/Laser-Plasma_ontology#Macroparticle"/>
        <rdfs:range rdf:resource="http://www.w3.org/2001/XMLSchema#string"/>
        <rdfs:comment>the attribute NAME that refer to the weighting factor of a macroparticle which represents the relative importance or scaling of the macroparticle. It represents the name or reference to the PIC code for the attribute. However, the actual data type that represents can be a numerical value like a float or an integer in the code.</rdfs:comment>
    </owl:DatatypeProperty>
    


    <!-- http://www.semanticweb.org/afshar87/ontologies/2024/3/Laser-Plasma_ontology#moving_window_velocity -->

    <owl:DatatypeProperty rdf:about="http://www.semanticweb.org/afshar87/ontologies/2024/3/Laser-Plasma_ontology#moving_window_velocity">
        <rdfs:subPropertyOf rdf:resource="http://www.semanticweb.org/afshar87/ontologies/2024/3/Laser-Plasma_ontology#simulation_property"/>
        <rdfs:domain rdf:resource="http://www.semanticweb.org/afshar87/ontologies/2024/3/Laser-Plasma_ontology#Simulation"/>
        <rdfs:comment>If we have moving Window in the simulation</rdfs:comment>
    </owl:DatatypeProperty>
    


    <!-- http://www.semanticweb.org/afshar87/ontologies/2024/3/Laser-Plasma_ontology#moving_window_velocity_enabled -->

    <owl:DatatypeProperty rdf:about="http://www.semanticweb.org/afshar87/ontologies/2024/3/Laser-Plasma_ontology#moving_window_velocity_enabled">
        <rdfs:subPropertyOf rdf:resource="http://www.semanticweb.org/afshar87/ontologies/2024/3/Laser-Plasma_ontology#moving_window_velocity"/>
        <rdfs:domain rdf:resource="http://www.semanticweb.org/afshar87/ontologies/2024/3/Laser-Plasma_ontology#Simulation"/>
        <rdfs:range rdf:resource="http://www.w3.org/2001/XMLSchema#boolean"/>
    </owl:DatatypeProperty>
    


    <!-- http://www.semanticweb.org/afshar87/ontologies/2024/3/Laser-Plasma_ontology#moving_window_velocity_x -->

    <owl:DatatypeProperty rdf:about="http://www.semanticweb.org/afshar87/ontologies/2024/3/Laser-Plasma_ontology#moving_window_velocity_x">
        <rdfs:subPropertyOf rdf:resource="http://www.semanticweb.org/afshar87/ontologies/2024/3/Laser-Plasma_ontology#moving_window_velocity"/>
        <rdfs:domain rdf:resource="http://www.semanticweb.org/afshar87/ontologies/2024/3/Laser-Plasma_ontology#Simulation"/>
        <rdfs:range rdf:resource="http://www.w3.org/2001/XMLSchema#float"/>
    </owl:DatatypeProperty>
    


    <!-- http://www.semanticweb.org/afshar87/ontologies/2024/3/Laser-Plasma_ontology#moving_window_velocity_y -->

    <owl:DatatypeProperty rdf:about="http://www.semanticweb.org/afshar87/ontologies/2024/3/Laser-Plasma_ontology#moving_window_velocity_y">
        <rdfs:subPropertyOf rdf:resource="http://www.semanticweb.org/afshar87/ontologies/2024/3/Laser-Plasma_ontology#moving_window_velocity"/>
        <rdfs:domain rdf:resource="http://www.semanticweb.org/afshar87/ontologies/2024/3/Laser-Plasma_ontology#Simulation"/>
        <rdfs:range rdf:resource="http://www.w3.org/2001/XMLSchema#float"/>
    </owl:DatatypeProperty>
    


    <!-- http://www.semanticweb.org/afshar87/ontologies/2024/3/Laser-Plasma_ontology#moving_window_velocity_z -->

    <owl:DatatypeProperty rdf:about="http://www.semanticweb.org/afshar87/ontologies/2024/3/Laser-Plasma_ontology#moving_window_velocity_z">
        <rdfs:subPropertyOf rdf:resource="http://www.semanticweb.org/afshar87/ontologies/2024/3/Laser-Plasma_ontology#moving_window_velocity"/>
        <rdfs:domain rdf:resource="http://www.semanticweb.org/afshar87/ontologies/2024/3/Laser-Plasma_ontology#Simulation"/>
        <rdfs:range rdf:resource="http://www.w3.org/2001/XMLSchema#float"/>
    </owl:DatatypeProperty>
    


    <!-- http://www.semanticweb.org/afshar87/ontologies/2024/3/Laser-Plasma_ontology#opacity -->

    <owl:DatatypeProperty rdf:about="http://www.semanticweb.org/afshar87/ontologies/2024/3/Laser-Plasma_ontology#opacity">
        <rdfs:subPropertyOf rdf:resource="http://www.semanticweb.org/afshar87/ontologies/2024/3/Laser-Plasma_ontology#plasma_properties"/>
        <rdfs:domain rdf:resource="http://www.semanticweb.org/afshar87/ontologies/2024/3/Laser-Plasma_ontology#Plasma"/>
        <rdfs:range rdf:resource="http://www.w3.org/2001/XMLSchema#double"/>
        <rdfs:comment>Opacity of the plasma, representing its ability to absorb radiation (often expressed in cm^-1).</rdfs:comment>
    </owl:DatatypeProperty>
    


    <!-- http://www.semanticweb.org/afshar87/ontologies/2024/3/Laser-Plasma_ontology#particle_bunch_properties -->

    <owl:DatatypeProperty rdf:about="http://www.semanticweb.org/afshar87/ontologies/2024/3/Laser-Plasma_ontology#particle_bunch_properties">
        <rdfs:domain rdf:resource="http://www.semanticweb.org/afshar87/ontologies/2024/3/Laser-Plasma_ontology#Laser_Plasma_Application"/>
        <rdfs:range rdf:resource="http://www.w3.org/2001/XMLSchema#float"/>
        <rdfs:comment>laser-produced lasma generates particle beam with following characteristics</rdfs:comment>
    </owl:DatatypeProperty>
    


    <!-- http://www.semanticweb.org/afshar87/ontologies/2024/3/Laser-Plasma_ontology#particle_shape_gaussian_amplitude -->

    <owl:DatatypeProperty rdf:about="http://www.semanticweb.org/afshar87/ontologies/2024/3/Laser-Plasma_ontology#particle_shape_gaussian_amplitude">
        <rdfs:subPropertyOf rdf:resource="http://www.semanticweb.org/afshar87/ontologies/2024/3/Laser-Plasma_ontology#species_particle_shape"/>
        <rdfs:domain rdf:resource="http://www.semanticweb.org/afshar87/ontologies/2024/3/Laser-Plasma_ontology#Species"/>
        <rdfs:range rdf:resource="http://www.w3.org/2001/XMLSchema#double"/>
        <rdfs:comment>The amplitude (A) represents the maximum value of the Gaussian curve, which scales the height of the distribution. 

f(x) = A*exp F*0.5* [  (xâˆ’Î¼) / (Ïƒ) ]^n</rdfs:comment>
    </owl:DatatypeProperty>
    


    <!-- http://www.semanticweb.org/afshar87/ontologies/2024/3/Laser-Plasma_ontology#particle_shape_gaussian_center -->

    <owl:DatatypeProperty rdf:about="http://www.semanticweb.org/afshar87/ontologies/2024/3/Laser-Plasma_ontology#particle_shape_gaussian_center">
        <rdfs:subPropertyOf rdf:resource="http://www.semanticweb.org/afshar87/ontologies/2024/3/Laser-Plasma_ontology#species_particle_shape"/>
        <rdfs:domain rdf:resource="http://www.semanticweb.org/afshar87/ontologies/2024/3/Laser-Plasma_ontology#Species"/>
        <rdfs:range rdf:resource="http://www.w3.org/2001/XMLSchema#float"/>
        <rdfs:comment>center (Î¼) is the point around which the Gaussian curve is symmetrically distributed.


f(x) = A*exp F*0.5* [  (xâˆ’Î¼) / (Ïƒ) ]^n</rdfs:comment>
    </owl:DatatypeProperty>
    


    <!-- http://www.semanticweb.org/afshar87/ontologies/2024/3/Laser-Plasma_ontology#particle_shape_gaussian_factor -->

    <owl:DatatypeProperty rdf:about="http://www.semanticweb.org/afshar87/ontologies/2024/3/Laser-Plasma_ontology#particle_shape_gaussian_factor">
        <rdfs:subPropertyOf rdf:resource="http://www.semanticweb.org/afshar87/ontologies/2024/3/Laser-Plasma_ontology#species_particle_shape"/>
        <rdfs:domain rdf:resource="http://www.semanticweb.org/afshar87/ontologies/2024/3/Laser-Plasma_ontology#Species"/>
        <rdfs:range rdf:resource="http://www.w3.org/2001/XMLSchema#float"/>
        <rdfs:comment>the factor (F) adjusts the shape and scaling of the Gaussian distribution.

f(x) = A*exp F*0.5* [  (xâˆ’Î¼) / (Ïƒ) ]^n

Effect of F:

If  F&gt;0, the decay of the Gaussian function is slower, resulting in a broader distribution.
If  F&lt;0, like  F=âˆ’1, the exponential decay is steeper, making the distribution narrower and more peaked around  Î¼.

Significance:

Setting  F=âˆ’1 often means the function is normalized such that the area under the Gaussian curve equals A, which is the amplitude of the peak.</rdfs:comment>
    </owl:DatatypeProperty>
    


    <!-- http://www.semanticweb.org/afshar87/ontologies/2024/3/Laser-Plasma_ontology#particle_shape_gaussian_power -->

    <owl:DatatypeProperty rdf:about="http://www.semanticweb.org/afshar87/ontologies/2024/3/Laser-Plasma_ontology#particle_shape_gaussian_power">
        <rdfs:subPropertyOf rdf:resource="http://www.semanticweb.org/afshar87/ontologies/2024/3/Laser-Plasma_ontology#species_particle_shape"/>
        <rdfs:domain rdf:resource="http://www.semanticweb.org/afshar87/ontologies/2024/3/Laser-Plasma_ontology#Species"/>
        <rdfs:range rdf:resource="http://www.w3.org/2001/XMLSchema#float"/>
        <rdfs:comment>the power (n) is to raise the exponential argument of a Gaussian function with the following form

f(x) = A*exp F*0.5* [  (xâˆ’Î¼) / (Ïƒ) ]^n</rdfs:comment>
    </owl:DatatypeProperty>
    


    <!-- http://www.semanticweb.org/afshar87/ontologies/2024/3/Laser-Plasma_ontology#particle_shape_gaussian_sigma -->

    <owl:DatatypeProperty rdf:about="http://www.semanticweb.org/afshar87/ontologies/2024/3/Laser-Plasma_ontology#particle_shape_gaussian_sigma">
        <rdfs:subPropertyOf rdf:resource="http://www.semanticweb.org/afshar87/ontologies/2024/3/Laser-Plasma_ontology#species_particle_shape"/>
        <rdfs:domain rdf:resource="http://www.semanticweb.org/afshar87/ontologies/2024/3/Laser-Plasma_ontology#Species"/>
        <rdfs:range rdf:resource="http://www.w3.org/2001/XMLSchema#double"/>
        <rdfs:comment>the standard deviation (Ïƒ) of the Gaussian distribution which determines the spread or width of the Gaussian distribution.


f(x) = A*exp F*0.5* [  (xâˆ’Î¼) / (Ïƒ) ]^n</rdfs:comment>
    </owl:DatatypeProperty>
    


    <!-- http://www.semanticweb.org/afshar87/ontologies/2024/3/Laser-Plasma_ontology#plasma_properties -->

    <owl:DatatypeProperty rdf:about="http://www.semanticweb.org/afshar87/ontologies/2024/3/Laser-Plasma_ontology#plasma_properties"/>
    


    <!-- http://www.semanticweb.org/afshar87/ontologies/2024/3/Laser-Plasma_ontology#project_data_end -->

    <owl:DatatypeProperty rdf:about="http://www.semanticweb.org/afshar87/ontologies/2024/3/Laser-Plasma_ontology#project_data_end">
        <rdfs:subPropertyOf rdf:resource="http://www.semanticweb.org/afshar87/ontologies/2024/3/Laser-Plasma_ontology#project_date"/>
        <rdfs:domain rdf:resource="http://www.semanticweb.org/afshar87/ontologies/2024/3/Laser-Plasma_ontology#Project"/>
        <rdfs:range rdf:resource="http://www.w3.org/2001/XMLSchema#dateTime"/>
        <rdfs:comment>the date a project has been ended</rdfs:comment>
    </owl:DatatypeProperty>
    


    <!-- http://www.semanticweb.org/afshar87/ontologies/2024/3/Laser-Plasma_ontology#project_data_start -->

    <owl:DatatypeProperty rdf:about="http://www.semanticweb.org/afshar87/ontologies/2024/3/Laser-Plasma_ontology#project_data_start">
        <rdfs:subPropertyOf rdf:resource="http://www.semanticweb.org/afshar87/ontologies/2024/3/Laser-Plasma_ontology#project_date"/>
        <rdfs:domain rdf:resource="http://www.semanticweb.org/afshar87/ontologies/2024/3/Laser-Plasma_ontology#Project"/>
        <rdfs:range rdf:resource="http://www.w3.org/2001/XMLSchema#dateTime"/>
        <rdfs:comment>the date a project has been started</rdfs:comment>
    </owl:DatatypeProperty>
    


    <!-- http://www.semanticweb.org/afshar87/ontologies/2024/3/Laser-Plasma_ontology#project_date -->

    <owl:DatatypeProperty rdf:about="http://www.semanticweb.org/afshar87/ontologies/2024/3/Laser-Plasma_ontology#project_date">
        <rdfs:subPropertyOf rdf:resource="http://www.semanticweb.org/afshar87/ontologies/2024/3/Laser-Plasma_ontology#project_property"/>
        <rdfs:domain rdf:resource="http://www.semanticweb.org/afshar87/ontologies/2024/3/Laser-Plasma_ontology#Project"/>
        <rdfs:range rdf:resource="http://www.w3.org/2001/XMLSchema#dateTime"/>
        <rdfs:comment>the date a project has been performed</rdfs:comment>
    </owl:DatatypeProperty>
    


    <!-- http://www.semanticweb.org/afshar87/ontologies/2024/3/Laser-Plasma_ontology#project_fund -->

    <owl:DatatypeProperty rdf:about="http://www.semanticweb.org/afshar87/ontologies/2024/3/Laser-Plasma_ontology#project_fund">
        <rdfs:subPropertyOf rdf:resource="http://www.semanticweb.org/afshar87/ontologies/2024/3/Laser-Plasma_ontology#project_property"/>
        <rdfs:domain rdf:resource="http://www.semanticweb.org/afshar87/ontologies/2024/3/Laser-Plasma_ontology#Project"/>
        <rdfs:range rdf:resource="http://www.w3.org/2001/XMLSchema#string"/>
        <rdfs:comment>The fund that is dedicated to the specific project.</rdfs:comment>
    </owl:DatatypeProperty>
    


    <!-- http://www.semanticweb.org/afshar87/ontologies/2024/3/Laser-Plasma_ontology#project_goal -->

    <owl:DatatypeProperty rdf:about="http://www.semanticweb.org/afshar87/ontologies/2024/3/Laser-Plasma_ontology#project_goal">
        <rdfs:subPropertyOf rdf:resource="http://www.semanticweb.org/afshar87/ontologies/2024/3/Laser-Plasma_ontology#project_property"/>
        <rdfs:domain rdf:resource="http://www.semanticweb.org/afshar87/ontologies/2024/3/Laser-Plasma_ontology#Project"/>
        <rdfs:range rdf:resource="http://www.w3.org/2001/XMLSchema#string"/>
        <rdfs:comment>the goals or open questions that will be addressed in the project.</rdfs:comment>
    </owl:DatatypeProperty>
    


    <!-- http://www.semanticweb.org/afshar87/ontologies/2024/3/Laser-Plasma_ontology#project_property -->

    <owl:DatatypeProperty rdf:about="http://www.semanticweb.org/afshar87/ontologies/2024/3/Laser-Plasma_ontology#project_property">
        <rdfs:domain rdf:resource="http://www.semanticweb.org/afshar87/ontologies/2024/3/Laser-Plasma_ontology#Project"/>
        <rdfs:comment>the properties of a project (either simulation or experiment)</rdfs:comment>
    </owl:DatatypeProperty>
    


    <!-- http://www.semanticweb.org/afshar87/ontologies/2024/3/Laser-Plasma_ontology#project_title -->

    <owl:DatatypeProperty rdf:about="http://www.semanticweb.org/afshar87/ontologies/2024/3/Laser-Plasma_ontology#project_title">
        <rdfs:subPropertyOf rdf:resource="http://www.semanticweb.org/afshar87/ontologies/2024/3/Laser-Plasma_ontology#project_property"/>
        <rdfs:domain rdf:resource="http://www.semanticweb.org/afshar87/ontologies/2024/3/Laser-Plasma_ontology#Project"/>
        <rdfs:range rdf:resource="http://www.w3.org/2001/XMLSchema#string"/>
        <rdfs:comment>the title of project that can be an experimental or simulation work</rdfs:comment>
    </owl:DatatypeProperty>
    


    <!-- http://www.semanticweb.org/afshar87/ontologies/2024/3/Laser-Plasma_ontology#radiation_emission -->

    <owl:DatatypeProperty rdf:about="http://www.semanticweb.org/afshar87/ontologies/2024/3/Laser-Plasma_ontology#radiation_emission">
        <rdfs:subPropertyOf rdf:resource="http://www.semanticweb.org/afshar87/ontologies/2024/3/Laser-Plasma_ontology#plasma_properties"/>
        <rdfs:domain rdf:resource="http://www.semanticweb.org/afshar87/ontologies/2024/3/Laser-Plasma_ontology#Plasma"/>
        <rdfs:range rdf:resource="http://www.w3.org/2001/XMLSchema#string"/>
        <rdfs:comment>The radiation emission from (laser) plasma that can be x-ray, gamma ray, etc.</rdfs:comment>
    </owl:DatatypeProperty>
    


    <!-- http://www.semanticweb.org/afshar87/ontologies/2024/3/Laser-Plasma_ontology#recombination_bound_electron -->

    <owl:DatatypeProperty rdf:about="http://www.semanticweb.org/afshar87/ontologies/2024/3/Laser-Plasma_ontology#recombination_bound_electron">
        <rdfs:subPropertyOf rdf:resource="http://www.semanticweb.org/afshar87/ontologies/2024/3/Laser-Plasma_ontology#Recombination"/>
        <rdfs:domain rdf:resource="http://www.semanticweb.org/afshar87/ontologies/2024/3/Laser-Plasma_ontology#Laser_Plasma_Physics"/>
        <rdfs:range rdf:resource="http://www.w3.org/2001/XMLSchema#string"/>
        <rdfs:comment>recombination via bound electrons known as charge exchange</rdfs:comment>
    </owl:DatatypeProperty>
    


    <!-- http://www.semanticweb.org/afshar87/ontologies/2024/3/Laser-Plasma_ontology#recombination_dielectronic -->

    <owl:DatatypeProperty rdf:about="http://www.semanticweb.org/afshar87/ontologies/2024/3/Laser-Plasma_ontology#recombination_dielectronic">
        <rdfs:subPropertyOf rdf:resource="http://www.semanticweb.org/afshar87/ontologies/2024/3/Laser-Plasma_ontology#recombination_free_electron"/>
        <rdfs:domain rdf:resource="http://www.semanticweb.org/afshar87/ontologies/2024/3/Laser-Plasma_ontology#Laser_Plasma_Physics"/>
        <rdfs:range rdf:resource="http://www.w3.org/2001/XMLSchema#string"/>
    </owl:DatatypeProperty>
    


    <!-- http://www.semanticweb.org/afshar87/ontologies/2024/3/Laser-Plasma_ontology#recombination_free_electron -->

    <owl:DatatypeProperty rdf:about="http://www.semanticweb.org/afshar87/ontologies/2024/3/Laser-Plasma_ontology#recombination_free_electron">
        <rdfs:subPropertyOf rdf:resource="http://www.semanticweb.org/afshar87/ontologies/2024/3/Laser-Plasma_ontology#Recombination"/>
        <rdfs:domain rdf:resource="http://www.semanticweb.org/afshar87/ontologies/2024/3/Laser-Plasma_ontology#Laser_Plasma_Physics"/>
        <rdfs:range rdf:resource="http://www.w3.org/2001/XMLSchema#string"/>
        <rdfs:comment>recombination via free electron</rdfs:comment>
    </owl:DatatypeProperty>
    


    <!-- http://www.semanticweb.org/afshar87/ontologies/2024/3/Laser-Plasma_ontology#recombination_radiative -->

    <owl:DatatypeProperty rdf:about="http://www.semanticweb.org/afshar87/ontologies/2024/3/Laser-Plasma_ontology#recombination_radiative">
        <rdfs:subPropertyOf rdf:resource="http://www.semanticweb.org/afshar87/ontologies/2024/3/Laser-Plasma_ontology#recombination_free_electron"/>
        <rdfs:domain rdf:resource="http://www.semanticweb.org/afshar87/ontologies/2024/3/Laser-Plasma_ontology#Laser_Plasma_Physics"/>
        <rdfs:range rdf:resource="http://www.w3.org/2001/XMLSchema#string"/>
        <rdfs:comment>radiative recombination</rdfs:comment>
    </owl:DatatypeProperty>
    


    <!-- http://www.semanticweb.org/afshar87/ontologies/2024/3/Laser-Plasma_ontology#recombination_threebody -->

    <owl:DatatypeProperty rdf:about="http://www.semanticweb.org/afshar87/ontologies/2024/3/Laser-Plasma_ontology#recombination_threebody">
        <rdfs:subPropertyOf rdf:resource="http://www.semanticweb.org/afshar87/ontologies/2024/3/Laser-Plasma_ontology#recombination_free_electron"/>
        <rdfs:domain rdf:resource="http://www.semanticweb.org/afshar87/ontologies/2024/3/Laser-Plasma_ontology#Laser_Plasma_Physics"/>
        <rdfs:range rdf:resource="http://www.w3.org/2001/XMLSchema#string"/>
        <rdfs:comment>threebody recombination</rdfs:comment>
    </owl:DatatypeProperty>
    


    <!-- http://www.semanticweb.org/afshar87/ontologies/2024/3/Laser-Plasma_ontology#simulation_approach -->

    <owl:DatatypeProperty rdf:about="http://www.semanticweb.org/afshar87/ontologies/2024/3/Laser-Plasma_ontology#simulation_approach">
        <rdfs:subPropertyOf rdf:resource="http://www.semanticweb.org/afshar87/ontologies/2024/3/Laser-Plasma_ontology#simulation_property"/>
        <rdfs:domain rdf:resource="http://www.semanticweb.org/afshar87/ontologies/2024/3/Laser-Plasma_ontology#Simulation"/>
        <rdfs:range rdf:resource="http://www.w3.org/2001/XMLSchema#string"/>
        <rdfs:comment>, several approaches are used to model the complex interactions between the intense laser pulse and the plasma. Here&apos;s a breakdown of the most common methods:

1. Particle-in-Cell (PIC) Simulation:

Method: PIC is a powerful technique that treats the plasma as a collection of charged particles (electrons and ions) and the laser pulse as an electromagnetic field. The particles&apos; motion and interactions are tracked by solving the equations of motion for each particle under the influence of the electromagnetic field and collisions.
Strengths:
Captures the kinetic behavior of particles in the plasma.
Can model a wide range of phenomena, including laser-driven wakefield generation, electron acceleration, and nonlinear laser-plasma interactions.
Weaknesses:
Computationally expensive, especially for large-scale simulations.
Requires careful choice of parameters like particle number, simulation size, and collision model.

2. Fluid Simulations:

Method: This approach treats the plasma as a continuous fluid described by macroscopic quantities like density, velocity, and pressure. The dynamics of the fluid are governed by fluid equations like the hydrodynamic equations or magnetohydrodynamic (MHD) equations.
Strengths:
Less computationally expensive compared to PIC for large-scale simulations.
Useful for studying large-scale phenomena in plasma, like shock waves and instabilities.
Weaknesses:
Loses information about the kinetic behavior of individual particles.
May not be accurate for situations where kinetic effects are important, such as very short time scales or strong laser-plasma interactions.

3. Hybrid Simulations:

Method: This combines PIC and fluid approaches. A specific region of the simulation domain might be treated with PIC for high-fidelity modeling of particle dynamics, while other regions can be modeled using less computationally expensive fluid equations.
Strengths:
Offers a balance between computational efficiency and accuracy.
Can be tailored to capture the most important physics in different regions of the simulation domain.
Weaknesses:
Requires careful consideration of the interface between PIC and fluid regions.
Might still be computationally expensive depending on the complexity of the problem.

Radiation-Hydrodynamics Simulation:

4. Simulations that combine the principles of radiation transport and hydrodynamics to model high-energy-density physics scenarios.

5. Molecular Dynamics Simulation:

Simulations that use molecular dynamics to study the interactions and dynamics of particles on a molecular level.


Magnetohydrodynamics (MHD) Simulation:

Simulations that combine magnetic and fluid dynamic equations to model the behavior of magnetized plasmas.</rdfs:comment>
    </owl:DatatypeProperty>
    


    <!-- http://www.semanticweb.org/afshar87/ontologies/2024/3/Laser-Plasma_ontology#simulation_bc_r -->

    <owl:DatatypeProperty rdf:about="http://www.semanticweb.org/afshar87/ontologies/2024/3/Laser-Plasma_ontology#simulation_bc_r">
        <rdfs:subPropertyOf rdf:resource="http://www.semanticweb.org/afshar87/ontologies/2024/3/Laser-Plasma_ontology#simulation_boundary_condition"/>
        <rdfs:domain rdf:resource="http://www.semanticweb.org/afshar87/ontologies/2024/3/Laser-Plasma_ontology#BoundaryConditionType"/>
        <rdfs:range rdf:resource="http://www.w3.org/2001/XMLSchema#string"/>
        <rdfs:comment>in Cylindrical geometry:

 Boundary condition at either side of R  (both min and max) : e.g. periodic, open, dirichlet.</rdfs:comment>
    </owl:DatatypeProperty>
    


    <!-- http://www.semanticweb.org/afshar87/ontologies/2024/3/Laser-Plasma_ontology#simulation_bc_rmax -->

    <owl:DatatypeProperty rdf:about="http://www.semanticweb.org/afshar87/ontologies/2024/3/Laser-Plasma_ontology#simulation_bc_rmax">
        <rdfs:subPropertyOf rdf:resource="http://www.semanticweb.org/afshar87/ontologies/2024/3/Laser-Plasma_ontology#simulation_boundary_condition"/>
        <rdfs:domain rdf:resource="http://www.semanticweb.org/afshar87/ontologies/2024/3/Laser-Plasma_ontology#BoundaryConditionType"/>
        <rdfs:range rdf:resource="http://www.w3.org/2001/XMLSchema#string"/>
        <rdfs:comment>in Cylindrical geometry:

 Boundary condition at max R: e.g. periodic, open, dirichlet.</rdfs:comment>
    </owl:DatatypeProperty>
    


    <!-- http://www.semanticweb.org/afshar87/ontologies/2024/3/Laser-Plasma_ontology#simulation_bc_rmin -->

    <owl:DatatypeProperty rdf:about="http://www.semanticweb.org/afshar87/ontologies/2024/3/Laser-Plasma_ontology#simulation_bc_rmin">
        <rdfs:subPropertyOf rdf:resource="http://www.semanticweb.org/afshar87/ontologies/2024/3/Laser-Plasma_ontology#simulation_boundary_condition"/>
        <rdfs:domain rdf:resource="http://www.semanticweb.org/afshar87/ontologies/2024/3/Laser-Plasma_ontology#BoundaryConditionType"/>
        <rdfs:range rdf:resource="http://www.w3.org/2001/XMLSchema#string"/>
        <rdfs:comment>in Cylindrical geometry:

 Boundary condition at min R: e.g. periodic, open, dirichlet.</rdfs:comment>
    </owl:DatatypeProperty>
    


    <!-- http://www.semanticweb.org/afshar87/ontologies/2024/3/Laser-Plasma_ontology#simulation_bc_x -->

    <owl:DatatypeProperty rdf:about="http://www.semanticweb.org/afshar87/ontologies/2024/3/Laser-Plasma_ontology#simulation_bc_x">
        <rdfs:subPropertyOf rdf:resource="http://www.semanticweb.org/afshar87/ontologies/2024/3/Laser-Plasma_ontology#simulation_boundary_condition"/>
        <rdfs:domain rdf:resource="http://www.semanticweb.org/afshar87/ontologies/2024/3/Laser-Plasma_ontology#BoundaryConditionType"/>
        <rdfs:range rdf:resource="http://www.w3.org/2001/XMLSchema#string"/>
        <rdfs:comment>Boundary condition at either side of x  direction (both min and max) : e.g. periodic, open, dirichlet.</rdfs:comment>
    </owl:DatatypeProperty>
    


    <!-- http://www.semanticweb.org/afshar87/ontologies/2024/3/Laser-Plasma_ontology#simulation_bc_xmax -->

    <owl:DatatypeProperty rdf:about="http://www.semanticweb.org/afshar87/ontologies/2024/3/Laser-Plasma_ontology#simulation_bc_xmax">
        <rdfs:subPropertyOf rdf:resource="http://www.semanticweb.org/afshar87/ontologies/2024/3/Laser-Plasma_ontology#simulation_boundary_condition"/>
        <rdfs:domain rdf:resource="http://www.semanticweb.org/afshar87/ontologies/2024/3/Laser-Plasma_ontology#BoundaryConditionType"/>
        <rdfs:range rdf:resource="http://www.w3.org/2001/XMLSchema#string"/>
        <rdfs:comment>Boundary condition at max X: e.g. periodic, open, dirichlet.</rdfs:comment>
    </owl:DatatypeProperty>
    


    <!-- http://www.semanticweb.org/afshar87/ontologies/2024/3/Laser-Plasma_ontology#simulation_bc_xmin -->

    <owl:DatatypeProperty rdf:about="http://www.semanticweb.org/afshar87/ontologies/2024/3/Laser-Plasma_ontology#simulation_bc_xmin">
        <rdfs:subPropertyOf rdf:resource="http://www.semanticweb.org/afshar87/ontologies/2024/3/Laser-Plasma_ontology#simulation_boundary_condition"/>
        <rdfs:domain rdf:resource="http://www.semanticweb.org/afshar87/ontologies/2024/3/Laser-Plasma_ontology#BoundaryConditionType"/>
        <rdfs:range rdf:resource="http://www.w3.org/2001/XMLSchema#string"/>
        <rdfs:comment>Boundary condition at min X: e.g. periodic, open, dirichlet.</rdfs:comment>
    </owl:DatatypeProperty>
    


    <!-- http://www.semanticweb.org/afshar87/ontologies/2024/3/Laser-Plasma_ontology#simulation_bc_y -->

    <owl:DatatypeProperty rdf:about="http://www.semanticweb.org/afshar87/ontologies/2024/3/Laser-Plasma_ontology#simulation_bc_y">
        <rdfs:subPropertyOf rdf:resource="http://www.semanticweb.org/afshar87/ontologies/2024/3/Laser-Plasma_ontology#simulation_boundary_condition"/>
        <rdfs:domain rdf:resource="http://www.semanticweb.org/afshar87/ontologies/2024/3/Laser-Plasma_ontology#BoundaryConditionType"/>
        <rdfs:range rdf:resource="http://www.w3.org/2001/XMLSchema#string"/>
        <rdfs:comment>Boundary condition at either side of y direction (both min and max) : e.g. periodic, open, dirichlet.</rdfs:comment>
    </owl:DatatypeProperty>
    


    <!-- http://www.semanticweb.org/afshar87/ontologies/2024/3/Laser-Plasma_ontology#simulation_bc_ymax -->

    <owl:DatatypeProperty rdf:about="http://www.semanticweb.org/afshar87/ontologies/2024/3/Laser-Plasma_ontology#simulation_bc_ymax">
        <rdfs:subPropertyOf rdf:resource="http://www.semanticweb.org/afshar87/ontologies/2024/3/Laser-Plasma_ontology#simulation_boundary_condition"/>
        <rdfs:domain rdf:resource="http://www.semanticweb.org/afshar87/ontologies/2024/3/Laser-Plasma_ontology#BoundaryConditionType"/>
        <rdfs:range rdf:resource="http://www.w3.org/2001/XMLSchema#string"/>
        <rdfs:comment>Boundary condition at max Y: e.g. periodic, open, dirichlet.</rdfs:comment>
    </owl:DatatypeProperty>
    


    <!-- http://www.semanticweb.org/afshar87/ontologies/2024/3/Laser-Plasma_ontology#simulation_bc_ymin -->

    <owl:DatatypeProperty rdf:about="http://www.semanticweb.org/afshar87/ontologies/2024/3/Laser-Plasma_ontology#simulation_bc_ymin">
        <rdfs:subPropertyOf rdf:resource="http://www.semanticweb.org/afshar87/ontologies/2024/3/Laser-Plasma_ontology#simulation_boundary_condition"/>
        <rdfs:domain rdf:resource="http://www.semanticweb.org/afshar87/ontologies/2024/3/Laser-Plasma_ontology#BoundaryConditionType"/>
        <rdfs:range rdf:resource="http://www.w3.org/2001/XMLSchema#string"/>
        <rdfs:comment>Boundary condition at min Y: e.g. periodic, open, dirichlet.</rdfs:comment>
    </owl:DatatypeProperty>
    


    <!-- http://www.semanticweb.org/afshar87/ontologies/2024/3/Laser-Plasma_ontology#simulation_bc_z -->

    <owl:DatatypeProperty rdf:about="http://www.semanticweb.org/afshar87/ontologies/2024/3/Laser-Plasma_ontology#simulation_bc_z">
        <rdfs:subPropertyOf rdf:resource="http://www.semanticweb.org/afshar87/ontologies/2024/3/Laser-Plasma_ontology#simulation_boundary_condition"/>
        <rdfs:domain rdf:resource="http://www.semanticweb.org/afshar87/ontologies/2024/3/Laser-Plasma_ontology#BoundaryConditionType"/>
        <rdfs:range rdf:resource="http://www.w3.org/2001/XMLSchema#string"/>
        <rdfs:comment>Boundary condition at either side of z direction (both min and max) : e.g. periodic, open, dirichlet.</rdfs:comment>
    </owl:DatatypeProperty>
    


    <!-- http://www.semanticweb.org/afshar87/ontologies/2024/3/Laser-Plasma_ontology#simulation_bc_zmax -->

    <owl:DatatypeProperty rdf:about="http://www.semanticweb.org/afshar87/ontologies/2024/3/Laser-Plasma_ontology#simulation_bc_zmax">
        <rdfs:subPropertyOf rdf:resource="http://www.semanticweb.org/afshar87/ontologies/2024/3/Laser-Plasma_ontology#simulation_boundary_condition"/>
        <rdfs:domain rdf:resource="http://www.semanticweb.org/afshar87/ontologies/2024/3/Laser-Plasma_ontology#BoundaryConditionType"/>
        <rdfs:range rdf:resource="http://www.w3.org/2001/XMLSchema#string"/>
        <rdfs:comment>in Cartesian  or Cylindrical geometry:

Boundary condition at max Z: e.g. periodic, open, dirichlet.</rdfs:comment>
    </owl:DatatypeProperty>
    


    <!-- http://www.semanticweb.org/afshar87/ontologies/2024/3/Laser-Plasma_ontology#simulation_bc_zmin -->

    <owl:DatatypeProperty rdf:about="http://www.semanticweb.org/afshar87/ontologies/2024/3/Laser-Plasma_ontology#simulation_bc_zmin">
        <rdfs:subPropertyOf rdf:resource="http://www.semanticweb.org/afshar87/ontologies/2024/3/Laser-Plasma_ontology#simulation_boundary_condition"/>
        <rdfs:domain rdf:resource="http://www.semanticweb.org/afshar87/ontologies/2024/3/Laser-Plasma_ontology#BoundaryConditionType"/>
        <rdfs:range rdf:resource="http://www.w3.org/2001/XMLSchema#string"/>
        <rdfs:comment>in Cartesian  or Cylindrical geometry:

Boundary condition at min Z: e.g. periodic, open, dirichlet.</rdfs:comment>
    </owl:DatatypeProperty>
    


    <!-- http://www.semanticweb.org/afshar87/ontologies/2024/3/Laser-Plasma_ontology#simulation_boundary_condition -->

    <owl:DatatypeProperty rdf:about="http://www.semanticweb.org/afshar87/ontologies/2024/3/Laser-Plasma_ontology#simulation_boundary_condition">
        <rdfs:subPropertyOf rdf:resource="http://www.semanticweb.org/afshar87/ontologies/2024/3/Laser-Plasma_ontology#simulation_property"/>
        <rdfs:domain rdf:resource="http://www.semanticweb.org/afshar87/ontologies/2024/3/Laser-Plasma_ontology#Simulation"/>
        <rdfs:range rdf:resource="http://www.w3.org/2001/XMLSchema#string"/>
        <rdfs:comment>The boundary conditions that are used in the simulation e.g. periodic, open, dirichlet.</rdfs:comment>
    </owl:DatatypeProperty>
    


    <!-- http://www.semanticweb.org/afshar87/ontologies/2024/3/Laser-Plasma_ontology#simulation_box -->

    <owl:DatatypeProperty rdf:about="http://www.semanticweb.org/afshar87/ontologies/2024/3/Laser-Plasma_ontology#simulation_box">
        <rdfs:subPropertyOf rdf:resource="http://www.semanticweb.org/afshar87/ontologies/2024/3/Laser-Plasma_ontology#simulation_property"/>
        <rdfs:domain rdf:resource="http://www.semanticweb.org/afshar87/ontologies/2024/3/Laser-Plasma_ontology#Simulation"/>
        <rdfs:range rdf:resource="http://www.w3.org/2001/XMLSchema#float"/>
        <rdfs:comment>simulation box which defines the min, and max values in X, Y, and Z directions.</rdfs:comment>
    </owl:DatatypeProperty>
    


    <!-- http://www.semanticweb.org/afshar87/ontologies/2024/3/Laser-Plasma_ontology#simulation_box_xmax -->

    <owl:DatatypeProperty rdf:about="http://www.semanticweb.org/afshar87/ontologies/2024/3/Laser-Plasma_ontology#simulation_box_xmax">
        <rdfs:subPropertyOf rdf:resource="http://www.semanticweb.org/afshar87/ontologies/2024/3/Laser-Plasma_ontology#simulation_box"/>
        <rdfs:domain rdf:resource="http://www.semanticweb.org/afshar87/ontologies/2024/3/Laser-Plasma_ontology#Simulation"/>
        <rdfs:range rdf:resource="http://www.w3.org/2001/XMLSchema#float"/>
        <rdfs:comment>simulation box which defines the max value in X direction.</rdfs:comment>
    </owl:DatatypeProperty>
    


    <!-- http://www.semanticweb.org/afshar87/ontologies/2024/3/Laser-Plasma_ontology#simulation_box_xmin -->

    <owl:DatatypeProperty rdf:about="http://www.semanticweb.org/afshar87/ontologies/2024/3/Laser-Plasma_ontology#simulation_box_xmin">
        <rdfs:subPropertyOf rdf:resource="http://www.semanticweb.org/afshar87/ontologies/2024/3/Laser-Plasma_ontology#simulation_box"/>
        <rdfs:domain rdf:resource="http://www.semanticweb.org/afshar87/ontologies/2024/3/Laser-Plasma_ontology#Simulation"/>
        <rdfs:range rdf:resource="http://www.w3.org/2001/XMLSchema#float"/>
        <rdfs:comment>simulation box which defines the min value in X direction.</rdfs:comment>
    </owl:DatatypeProperty>
    


    <!-- http://www.semanticweb.org/afshar87/ontologies/2024/3/Laser-Plasma_ontology#simulation_box_ymax -->

    <owl:DatatypeProperty rdf:about="http://www.semanticweb.org/afshar87/ontologies/2024/3/Laser-Plasma_ontology#simulation_box_ymax">
        <rdfs:subPropertyOf rdf:resource="http://www.semanticweb.org/afshar87/ontologies/2024/3/Laser-Plasma_ontology#simulation_box"/>
        <rdfs:domain rdf:resource="http://www.semanticweb.org/afshar87/ontologies/2024/3/Laser-Plasma_ontology#Simulation"/>
        <rdfs:range rdf:resource="http://www.w3.org/2001/XMLSchema#float"/>
        <rdfs:comment>simulation box which defines the max value in Y direction.</rdfs:comment>
    </owl:DatatypeProperty>
    


    <!-- http://www.semanticweb.org/afshar87/ontologies/2024/3/Laser-Plasma_ontology#simulation_box_ymin -->

    <owl:DatatypeProperty rdf:about="http://www.semanticweb.org/afshar87/ontologies/2024/3/Laser-Plasma_ontology#simulation_box_ymin">
        <rdfs:subPropertyOf rdf:resource="http://www.semanticweb.org/afshar87/ontologies/2024/3/Laser-Plasma_ontology#simulation_box"/>
        <rdfs:domain rdf:resource="http://www.semanticweb.org/afshar87/ontologies/2024/3/Laser-Plasma_ontology#Simulation"/>
        <rdfs:range rdf:resource="http://www.w3.org/2001/XMLSchema#float"/>
        <rdfs:comment>simulation box which defines the min value in Y direction.</rdfs:comment>
    </owl:DatatypeProperty>
    


    <!-- http://www.semanticweb.org/afshar87/ontologies/2024/3/Laser-Plasma_ontology#simulation_box_zmax -->

    <owl:DatatypeProperty rdf:about="http://www.semanticweb.org/afshar87/ontologies/2024/3/Laser-Plasma_ontology#simulation_box_zmax">
        <rdfs:subPropertyOf rdf:resource="http://www.semanticweb.org/afshar87/ontologies/2024/3/Laser-Plasma_ontology#simulation_box"/>
        <rdfs:domain rdf:resource="http://www.semanticweb.org/afshar87/ontologies/2024/3/Laser-Plasma_ontology#Simulation"/>
        <rdfs:range rdf:resource="http://www.w3.org/2001/XMLSchema#float"/>
        <rdfs:comment>in Cartesian  or Cylindrical geometry:

simulation box which defines the max value in Z direction.</rdfs:comment>
    </owl:DatatypeProperty>
    


    <!-- http://www.semanticweb.org/afshar87/ontologies/2024/3/Laser-Plasma_ontology#simulation_box_zmin -->

    <owl:DatatypeProperty rdf:about="http://www.semanticweb.org/afshar87/ontologies/2024/3/Laser-Plasma_ontology#simulation_box_zmin">
        <rdfs:subPropertyOf rdf:resource="http://www.semanticweb.org/afshar87/ontologies/2024/3/Laser-Plasma_ontology#simulation_box"/>
        <rdfs:domain rdf:resource="http://www.semanticweb.org/afshar87/ontologies/2024/3/Laser-Plasma_ontology#Simulation"/>
        <rdfs:range rdf:resource="http://www.w3.org/2001/XMLSchema#float"/>
        <rdfs:comment>in Cartesian  or Cylindrical geometry:

simulation box which defines the min value in Z direction.</rdfs:comment>
    </owl:DatatypeProperty>
    


    <!-- http://www.semanticweb.org/afshar87/ontologies/2024/3/Laser-Plasma_ontology#simulation_cell_size -->

    <owl:DatatypeProperty rdf:about="http://www.semanticweb.org/afshar87/ontologies/2024/3/Laser-Plasma_ontology#simulation_cell_size">
        <rdfs:subPropertyOf rdf:resource="http://www.semanticweb.org/afshar87/ontologies/2024/3/Laser-Plasma_ontology#simulation_property"/>
        <rdfs:domain rdf:resource="http://www.semanticweb.org/afshar87/ontologies/2024/3/Laser-Plasma_ontology#Simulation"/>
        <rdfs:range rdf:resource="http://www.w3.org/2001/XMLSchema#long"/>
        <rdfs:comment>The resolution that is used in simulation codes.</rdfs:comment>
    </owl:DatatypeProperty>
    


    <!-- http://www.semanticweb.org/afshar87/ontologies/2024/3/Laser-Plasma_ontology#simulation_cell_size_x -->

    <owl:DatatypeProperty rdf:about="http://www.semanticweb.org/afshar87/ontologies/2024/3/Laser-Plasma_ontology#simulation_cell_size_x">
        <rdfs:subPropertyOf rdf:resource="http://www.semanticweb.org/afshar87/ontologies/2024/3/Laser-Plasma_ontology#simulation_cell_size"/>
        <rdfs:domain rdf:resource="http://www.semanticweb.org/afshar87/ontologies/2024/3/Laser-Plasma_ontology#Simulation"/>
        <rdfs:range rdf:resource="http://www.w3.org/2001/XMLSchema#double"/>
        <rdfs:comment>simulation_cellSize in x direction</rdfs:comment>
    </owl:DatatypeProperty>
    


    <!-- http://www.semanticweb.org/afshar87/ontologies/2024/3/Laser-Plasma_ontology#simulation_cell_size_y -->

    <owl:DatatypeProperty rdf:about="http://www.semanticweb.org/afshar87/ontologies/2024/3/Laser-Plasma_ontology#simulation_cell_size_y">
        <rdfs:subPropertyOf rdf:resource="http://www.semanticweb.org/afshar87/ontologies/2024/3/Laser-Plasma_ontology#simulation_cell_size"/>
        <rdfs:domain rdf:resource="http://www.semanticweb.org/afshar87/ontologies/2024/3/Laser-Plasma_ontology#Simulation"/>
        <rdfs:range rdf:resource="http://www.w3.org/2001/XMLSchema#double"/>
        <rdfs:comment>simulation_cellSize in y direction</rdfs:comment>
    </owl:DatatypeProperty>
    


    <!-- http://www.semanticweb.org/afshar87/ontologies/2024/3/Laser-Plasma_ontology#simulation_cell_size_z -->

    <owl:DatatypeProperty rdf:about="http://www.semanticweb.org/afshar87/ontologies/2024/3/Laser-Plasma_ontology#simulation_cell_size_z">
        <rdfs:subPropertyOf rdf:resource="http://www.semanticweb.org/afshar87/ontologies/2024/3/Laser-Plasma_ontology#simulation_cell_size"/>
        <rdfs:domain rdf:resource="http://www.semanticweb.org/afshar87/ontologies/2024/3/Laser-Plasma_ontology#Simulation"/>
        <rdfs:range rdf:resource="http://www.w3.org/2001/XMLSchema#double"/>
        <rdfs:comment>simulation_cellSize in z direction</rdfs:comment>
    </owl:DatatypeProperty>
    


    <!-- http://www.semanticweb.org/afshar87/ontologies/2024/3/Laser-Plasma_ontology#simulation_code_version -->

    <owl:DatatypeProperty rdf:about="http://www.semanticweb.org/afshar87/ontologies/2024/3/Laser-Plasma_ontology#simulation_code_version">
        <rdfs:subPropertyOf rdf:resource="http://www.semanticweb.org/afshar87/ontologies/2024/3/Laser-Plasma_ontology#simulation_property"/>
        <rdfs:domain rdf:resource="http://www.semanticweb.org/afshar87/ontologies/2024/3/Laser-Plasma_ontology#Simulation"/>
        <rdfs:range rdf:resource="http://www.w3.org/2001/XMLSchema#float"/>
        <rdfs:range rdf:resource="http://www.w3.org/2001/XMLSchema#string"/>
        <rdfs:comment>The version of the simulation code that is used.</rdfs:comment>
    </owl:DatatypeProperty>
    


    <!-- http://www.semanticweb.org/afshar87/ontologies/2024/3/Laser-Plasma_ontology#simulation_field_solver -->

    <owl:DatatypeProperty rdf:about="http://www.semanticweb.org/afshar87/ontologies/2024/3/Laser-Plasma_ontology#simulation_field_solver">
        <rdfs:subPropertyOf rdf:resource="http://www.semanticweb.org/afshar87/ontologies/2024/3/Laser-Plasma_ontology#simulation_property"/>
        <rdfs:domain rdf:resource="http://www.semanticweb.org/afshar87/ontologies/2024/3/Laser-Plasma_ontology#Simulation"/>
        <rdfs:range rdf:resource="http://www.w3.org/2001/XMLSchema#string"/>
        <rdfs:comment>Which  field solver is used in the simulation e.g. &apos;Yee&apos;, &apos;CKC&apos;, &apos;Lehe&apos;.</rdfs:comment>
    </owl:DatatypeProperty>
    


    <!-- http://www.semanticweb.org/afshar87/ontologies/2024/3/Laser-Plasma_ontology#simulation_max_time_step -->

    <owl:DatatypeProperty rdf:about="http://www.semanticweb.org/afshar87/ontologies/2024/3/Laser-Plasma_ontology#simulation_max_time_step">
        <rdfs:subPropertyOf rdf:resource="http://www.semanticweb.org/afshar87/ontologies/2024/3/Laser-Plasma_ontology#simulation_property"/>
        <rdfs:domain rdf:resource="http://www.semanticweb.org/afshar87/ontologies/2024/3/Laser-Plasma_ontology#Simulation"/>
        <rdfs:range rdf:resource="http://www.w3.org/2001/XMLSchema#integer"/>
        <rdfs:comment>Maximum number of time steps in the simulation</rdfs:comment>
    </owl:DatatypeProperty>
    


    <!-- http://www.semanticweb.org/afshar87/ontologies/2024/3/Laser-Plasma_ontology#simulation_minimum_weight -->

    <owl:DatatypeProperty rdf:about="http://www.semanticweb.org/afshar87/ontologies/2024/3/Laser-Plasma_ontology#simulation_minimum_weight">
        <rdfs:subPropertyOf rdf:resource="http://www.semanticweb.org/afshar87/ontologies/2024/3/Laser-Plasma_ontology#simulation_property"/>
        <rdfs:domain rdf:resource="http://www.semanticweb.org/afshar87/ontologies/2024/3/Laser-Plasma_ontology#Simulation"/>
        <rdfs:range rdf:resource="http://www.w3.org/2001/XMLSchema#float"/>
    </owl:DatatypeProperty>
    


    <!-- http://www.semanticweb.org/afshar87/ontologies/2024/3/Laser-Plasma_ontology#simulation_nr -->

    <owl:DatatypeProperty rdf:about="http://www.semanticweb.org/afshar87/ontologies/2024/3/Laser-Plasma_ontology#simulation_nr">
        <rdfs:subPropertyOf rdf:resource="http://www.semanticweb.org/afshar87/ontologies/2024/3/Laser-Plasma_ontology#simulation_number_of_cells"/>
        <rdfs:domain rdf:resource="http://www.semanticweb.org/afshar87/ontologies/2024/3/Laser-Plasma_ontology#Simulation"/>
        <rdfs:range rdf:resource="http://www.w3.org/2001/XMLSchema#integer"/>
        <rdfs:comment>in Cylindrical geometry:

Number of cells along R (number of nodes = nr+1)</rdfs:comment>
    </owl:DatatypeProperty>
    


    <!-- http://www.semanticweb.org/afshar87/ontologies/2024/3/Laser-Plasma_ontology#simulation_number_of_cells -->

    <owl:DatatypeProperty rdf:about="http://www.semanticweb.org/afshar87/ontologies/2024/3/Laser-Plasma_ontology#simulation_number_of_cells">
        <rdfs:subPropertyOf rdf:resource="http://www.semanticweb.org/afshar87/ontologies/2024/3/Laser-Plasma_ontology#simulation_property"/>
        <rdfs:domain rdf:resource="http://www.semanticweb.org/afshar87/ontologies/2024/3/Laser-Plasma_ontology#Simulation"/>
        <rdfs:range rdf:resource="http://www.w3.org/2001/XMLSchema#integer"/>
    </owl:DatatypeProperty>
    


    <!-- http://www.semanticweb.org/afshar87/ontologies/2024/3/Laser-Plasma_ontology#simulation_number_of_gpu -->

    <owl:DatatypeProperty rdf:about="http://www.semanticweb.org/afshar87/ontologies/2024/3/Laser-Plasma_ontology#simulation_number_of_gpu">
        <rdfs:subPropertyOf rdf:resource="http://www.semanticweb.org/afshar87/ontologies/2024/3/Laser-Plasma_ontology#simulation_property"/>
        <rdfs:range rdf:resource="http://www.w3.org/2001/XMLSchema#integer"/>
    </owl:DatatypeProperty>
    


    <!-- http://www.semanticweb.org/afshar87/ontologies/2024/3/Laser-Plasma_ontology#simulation_number_of_gpu_x -->

    <owl:DatatypeProperty rdf:about="http://www.semanticweb.org/afshar87/ontologies/2024/3/Laser-Plasma_ontology#simulation_number_of_gpu_x">
        <rdfs:subPropertyOf rdf:resource="http://www.semanticweb.org/afshar87/ontologies/2024/3/Laser-Plasma_ontology#simulation_number_of_gpu"/>
        <rdfs:domain rdf:resource="http://www.semanticweb.org/afshar87/ontologies/2024/3/Laser-Plasma_ontology#Simulation"/>
        <rdfs:range rdf:resource="http://www.w3.org/2001/XMLSchema#integer"/>
        <rdfs:comment>number of gpu in x direction</rdfs:comment>
    </owl:DatatypeProperty>
    


    <!-- http://www.semanticweb.org/afshar87/ontologies/2024/3/Laser-Plasma_ontology#simulation_number_of_gpu_y -->

    <owl:DatatypeProperty rdf:about="http://www.semanticweb.org/afshar87/ontologies/2024/3/Laser-Plasma_ontology#simulation_number_of_gpu_y">
        <rdfs:subPropertyOf rdf:resource="http://www.semanticweb.org/afshar87/ontologies/2024/3/Laser-Plasma_ontology#simulation_number_of_gpu"/>
        <rdfs:domain rdf:resource="http://www.semanticweb.org/afshar87/ontologies/2024/3/Laser-Plasma_ontology#Simulation"/>
        <rdfs:range rdf:resource="http://www.w3.org/2001/XMLSchema#integer"/>
        <rdfs:comment>number of gpu in y direction</rdfs:comment>
    </owl:DatatypeProperty>
    


    <!-- http://www.semanticweb.org/afshar87/ontologies/2024/3/Laser-Plasma_ontology#simulation_number_of_gpu_z -->

    <owl:DatatypeProperty rdf:about="http://www.semanticweb.org/afshar87/ontologies/2024/3/Laser-Plasma_ontology#simulation_number_of_gpu_z">
        <rdfs:subPropertyOf rdf:resource="http://www.semanticweb.org/afshar87/ontologies/2024/3/Laser-Plasma_ontology#simulation_number_of_gpu"/>
        <rdfs:domain rdf:resource="http://www.semanticweb.org/afshar87/ontologies/2024/3/Laser-Plasma_ontology#Simulation"/>
        <rdfs:range rdf:resource="http://www.w3.org/2001/XMLSchema#integer"/>
        <rdfs:comment>number of gpu in z direction</rdfs:comment>
    </owl:DatatypeProperty>
    


    <!-- http://www.semanticweb.org/afshar87/ontologies/2024/3/Laser-Plasma_ontology#simulation_nx -->

    <owl:DatatypeProperty rdf:about="http://www.semanticweb.org/afshar87/ontologies/2024/3/Laser-Plasma_ontology#simulation_nx">
        <rdfs:subPropertyOf rdf:resource="http://www.semanticweb.org/afshar87/ontologies/2024/3/Laser-Plasma_ontology#simulation_number_of_cells"/>
        <rdfs:domain rdf:resource="http://www.semanticweb.org/afshar87/ontologies/2024/3/Laser-Plasma_ontology#Simulation"/>
        <rdfs:range rdf:resource="http://www.w3.org/2001/XMLSchema#integer"/>
        <rdfs:comment>Number of cells along X (number of grid nodes = nx+1)</rdfs:comment>
    </owl:DatatypeProperty>
    


    <!-- http://www.semanticweb.org/afshar87/ontologies/2024/3/Laser-Plasma_ontology#simulation_ny -->

    <owl:DatatypeProperty rdf:about="http://www.semanticweb.org/afshar87/ontologies/2024/3/Laser-Plasma_ontology#simulation_ny">
        <rdfs:subPropertyOf rdf:resource="http://www.semanticweb.org/afshar87/ontologies/2024/3/Laser-Plasma_ontology#simulation_number_of_cells"/>
        <rdfs:domain rdf:resource="http://www.semanticweb.org/afshar87/ontologies/2024/3/Laser-Plasma_ontology#Simulation"/>
        <rdfs:range rdf:resource="http://www.w3.org/2001/XMLSchema#integer"/>
        <rdfs:comment>Number of cells along Y (number of grid nodes = ny+1)</rdfs:comment>
    </owl:DatatypeProperty>
    


    <!-- http://www.semanticweb.org/afshar87/ontologies/2024/3/Laser-Plasma_ontology#simulation_nz -->

    <owl:DatatypeProperty rdf:about="http://www.semanticweb.org/afshar87/ontologies/2024/3/Laser-Plasma_ontology#simulation_nz">
        <rdfs:subPropertyOf rdf:resource="http://www.semanticweb.org/afshar87/ontologies/2024/3/Laser-Plasma_ontology#simulation_number_of_cells"/>
        <rdfs:domain rdf:resource="http://www.semanticweb.org/afshar87/ontologies/2024/3/Laser-Plasma_ontology#Simulation"/>
        <rdfs:range rdf:resource="http://www.w3.org/2001/XMLSchema#integer"/>
        <rdfs:comment>in Cartesian  or Cylindrical geometry:

Number of cells along Z (number of grid nodes = nz+1)</rdfs:comment>
    </owl:DatatypeProperty>
    


    <!-- http://www.semanticweb.org/afshar87/ontologies/2024/3/Laser-Plasma_ontology#simulation_output -->

    <owl:DatatypeProperty rdf:about="http://www.semanticweb.org/afshar87/ontologies/2024/3/Laser-Plasma_ontology#simulation_output">
        <rdfs:subPropertyOf rdf:resource="http://www.semanticweb.org/afshar87/ontologies/2024/3/Laser-Plasma_ontology#simulation_property"/>
    </owl:DatatypeProperty>
    


    <!-- http://www.semanticweb.org/afshar87/ontologies/2024/3/Laser-Plasma_ontology#simulation_output_png -->

    <owl:DatatypeProperty rdf:about="http://www.semanticweb.org/afshar87/ontologies/2024/3/Laser-Plasma_ontology#simulation_output_png">
        <rdfs:subPropertyOf rdf:resource="http://www.semanticweb.org/afshar87/ontologies/2024/3/Laser-Plasma_ontology#simulation_output"/>
        <rdfs:domain rdf:resource="http://www.semanticweb.org/afshar87/ontologies/2024/3/Laser-Plasma_ontology#Output"/>
        <rdfs:comment>output as png images of a parameter such as  magnetic field or electric field</rdfs:comment>
    </owl:DatatypeProperty>
    


    <!-- http://www.semanticweb.org/afshar87/ontologies/2024/3/Laser-Plasma_ontology#simulation_output_png_axis_2D -->

    <owl:DatatypeProperty rdf:about="http://www.semanticweb.org/afshar87/ontologies/2024/3/Laser-Plasma_ontology#simulation_output_png_axis_2D">
        <rdfs:subPropertyOf rdf:resource="http://www.semanticweb.org/afshar87/ontologies/2024/3/Laser-Plasma_ontology#simulation_output_png"/>
        <rdfs:domain rdf:resource="http://www.semanticweb.org/afshar87/ontologies/2024/3/Laser-Plasma_ontology#Output"/>
        <rdfs:range rdf:resource="http://www.w3.org/2001/XMLSchema#string"/>
        <rdfs:comment>the output of a parameter (e.g. magnetic field or electric field) in 2D such as xy, yz, yz, etc as png images.</rdfs:comment>
    </owl:DatatypeProperty>
    


    <!-- http://www.semanticweb.org/afshar87/ontologies/2024/3/Laser-Plasma_ontology#simulation_output_png_period -->

    <owl:DatatypeProperty rdf:about="http://www.semanticweb.org/afshar87/ontologies/2024/3/Laser-Plasma_ontology#simulation_output_png_period">
        <rdfs:subPropertyOf rdf:resource="http://www.semanticweb.org/afshar87/ontologies/2024/3/Laser-Plasma_ontology#simulation_output_png"/>
        <rdfs:domain rdf:resource="http://www.semanticweb.org/afshar87/ontologies/2024/3/Laser-Plasma_ontology#Output"/>
        <rdfs:range rdf:resource="http://www.w3.org/2001/XMLSchema#integer"/>
        <rdfs:comment>the period of the output as png images of a parameter such as  magnetic field or electric field</rdfs:comment>
    </owl:DatatypeProperty>
    


    <!-- http://www.semanticweb.org/afshar87/ontologies/2024/3/Laser-Plasma_ontology#simulation_particle_per_cell -->

    <owl:DatatypeProperty rdf:about="http://www.semanticweb.org/afshar87/ontologies/2024/3/Laser-Plasma_ontology#simulation_particle_per_cell">
        <rdfs:subPropertyOf rdf:resource="http://www.semanticweb.org/afshar87/ontologies/2024/3/Laser-Plasma_ontology#simulation_property"/>
        <rdfs:domain rdf:resource="http://www.semanticweb.org/afshar87/ontologies/2024/3/Laser-Plasma_ontology#Simulation"/>
        <rdfs:range rdf:resource="http://www.w3.org/2001/XMLSchema#integer"/>
        <rdfs:comment>number of particles per cell</rdfs:comment>
    </owl:DatatypeProperty>
    


    <!-- http://www.semanticweb.org/afshar87/ontologies/2024/3/Laser-Plasma_ontology#simulation_particle_pusher -->

    <owl:DatatypeProperty rdf:about="http://www.semanticweb.org/afshar87/ontologies/2024/3/Laser-Plasma_ontology#simulation_particle_pusher">
        <rdfs:subPropertyOf rdf:resource="http://www.semanticweb.org/afshar87/ontologies/2024/3/Laser-Plasma_ontology#simulation_property"/>
        <rdfs:domain rdf:resource="http://www.semanticweb.org/afshar87/ontologies/2024/3/Laser-Plasma_ontology#Simulation"/>
        <rdfs:range rdf:resource="http://www.w3.org/2001/XMLSchema#string"/>
        <rdfs:comment>Which particle pusher is used in the simulation.</rdfs:comment>
    </owl:DatatypeProperty>
    


    <!-- http://www.semanticweb.org/afshar87/ontologies/2024/3/Laser-Plasma_ontology#simulation_property -->

    <owl:DatatypeProperty rdf:about="http://www.semanticweb.org/afshar87/ontologies/2024/3/Laser-Plasma_ontology#simulation_property">
        <rdfs:domain rdf:resource="http://www.semanticweb.org/afshar87/ontologies/2024/3/Laser-Plasma_ontology#Simulation"/>
    </owl:DatatypeProperty>
    


    <!-- http://www.semanticweb.org/afshar87/ontologies/2024/3/Laser-Plasma_ontology#simulation_time_step -->

    <owl:DatatypeProperty rdf:about="http://www.semanticweb.org/afshar87/ontologies/2024/3/Laser-Plasma_ontology#simulation_time_step">
        <rdfs:subPropertyOf rdf:resource="http://www.semanticweb.org/afshar87/ontologies/2024/3/Laser-Plasma_ontology#simulation_property"/>
        <rdfs:domain rdf:resource="http://www.semanticweb.org/afshar87/ontologies/2024/3/Laser-Plasma_ontology#Simulation"/>
        <rdfs:range rdf:resource="http://www.w3.org/2001/XMLSchema#double"/>
        <rdfs:comment>time step used in the simulation.</rdfs:comment>
    </owl:DatatypeProperty>
    


    <!-- http://www.semanticweb.org/afshar87/ontologies/2024/3/Laser-Plasma_ontology#simulation_vacuum_cells -->

    <owl:DatatypeProperty rdf:about="http://www.semanticweb.org/afshar87/ontologies/2024/3/Laser-Plasma_ontology#simulation_vacuum_cells">
        <rdfs:subPropertyOf rdf:resource="http://www.semanticweb.org/afshar87/ontologies/2024/3/Laser-Plasma_ontology#simulation_property"/>
        <rdfs:domain rdf:resource="http://www.semanticweb.org/afshar87/ontologies/2024/3/Laser-Plasma_ontology#Simulation"/>
        <rdfs:range rdf:resource="http://www.w3.org/2001/XMLSchema#integer"/>
        <rdfs:comment>The number of vacuum cells assumes a charge-free volume  in front of a target  which is important for laser initialization and propagation.</rdfs:comment>
    </owl:DatatypeProperty>
    


    <!-- http://www.semanticweb.org/afshar87/ontologies/2024/3/Laser-Plasma_ontology#species_atomicMass -->

    <owl:DatatypeProperty rdf:about="http://www.semanticweb.org/afshar87/ontologies/2024/3/Laser-Plasma_ontology#species_atomicMass">
        <rdfs:subPropertyOf rdf:resource="http://www.semanticweb.org/afshar87/ontologies/2024/3/Laser-Plasma_ontology#species_properties"/>
        <rdfs:domain rdf:resource="http://www.semanticweb.org/afshar87/ontologies/2024/3/Laser-Plasma_ontology#Species"/>
        <rdfs:range rdf:resource="http://www.w3.org/2001/XMLSchema#double"/>
        <rdfs:comment>The sum of the number of protons and neutrons  in the nucleus of a species</rdfs:comment>
    </owl:DatatypeProperty>
    


    <!-- http://www.semanticweb.org/afshar87/ontologies/2024/3/Laser-Plasma_ontology#species_atomicNumber -->

    <owl:DatatypeProperty rdf:about="http://www.semanticweb.org/afshar87/ontologies/2024/3/Laser-Plasma_ontology#species_atomicNumber">
        <rdfs:subPropertyOf rdf:resource="http://www.semanticweb.org/afshar87/ontologies/2024/3/Laser-Plasma_ontology#species_properties"/>
        <rdfs:domain rdf:resource="http://www.semanticweb.org/afshar87/ontologies/2024/3/Laser-Plasma_ontology#Species"/>
        <rdfs:range rdf:resource="http://www.w3.org/2001/XMLSchema#nonNegativeInteger"/>
        <rdfs:comment>the number of protons in the nucleus of a species</rdfs:comment>
    </owl:DatatypeProperty>
    


    <!-- http://www.semanticweb.org/afshar87/ontologies/2024/3/Laser-Plasma_ontology#species_charge -->

    <owl:DatatypeProperty rdf:about="http://www.semanticweb.org/afshar87/ontologies/2024/3/Laser-Plasma_ontology#species_charge">
        <rdfs:subPropertyOf rdf:resource="http://www.semanticweb.org/afshar87/ontologies/2024/3/Laser-Plasma_ontology#species_properties"/>
        <rdfs:domain rdf:resource="http://www.semanticweb.org/afshar87/ontologies/2024/3/Laser-Plasma_ontology#Species"/>
        <rdfs:range rdf:resource="http://www.w3.org/2001/XMLSchema#double"/>
        <rdfs:comment>the charge of a species. Positive (negative) numbers can be used for positively (negatively) charged particles. (e.g., 1*e_charge, -4*e_charge) where e_charge = -1.60217663E-19.</rdfs:comment>
    </owl:DatatypeProperty>
    


    <!-- http://www.semanticweb.org/afshar87/ontologies/2024/3/Laser-Plasma_ontology#species_charge_e -->

    <owl:DatatypeProperty rdf:about="http://www.semanticweb.org/afshar87/ontologies/2024/3/Laser-Plasma_ontology#species_charge_e">
        <rdfs:subPropertyOf rdf:resource="http://www.semanticweb.org/afshar87/ontologies/2024/3/Laser-Plasma_ontology#species_properties"/>
        <rdfs:domain rdf:resource="http://www.semanticweb.org/afshar87/ontologies/2024/3/Laser-Plasma_ontology#Species"/>
        <rdfs:range rdf:resource="http://www.w3.org/2001/XMLSchema#float"/>
        <rdfs:comment>the charge of a species in multiples of the electron charge. Positive (negative) numbers can be used for positively (negatively) charged particles (e.g., +1.,+2, -4).</rdfs:comment>
    </owl:DatatypeProperty>
    


    <!-- http://www.semanticweb.org/afshar87/ontologies/2024/3/Laser-Plasma_ontology#species_chemical_symbol -->

    <owl:DatatypeProperty rdf:about="http://www.semanticweb.org/afshar87/ontologies/2024/3/Laser-Plasma_ontology#species_chemical_symbol">
        <rdfs:subPropertyOf rdf:resource="http://www.semanticweb.org/afshar87/ontologies/2024/3/Laser-Plasma_ontology#species_properties"/>
        <rdfs:domain rdf:resource="http://www.semanticweb.org/afshar87/ontologies/2024/3/Laser-Plasma_ontology#Species"/>
        <rdfs:range rdf:resource="http://www.w3.org/2001/XMLSchema#string"/>
        <rdfs:comment>species chemical symbol such as H, C, Au, etc.</rdfs:comment>
    </owl:DatatypeProperty>
    


    <!-- http://www.semanticweb.org/afshar87/ontologies/2024/3/Laser-Plasma_ontology#species_density_ratio -->

    <owl:DatatypeProperty rdf:about="http://www.semanticweb.org/afshar87/ontologies/2024/3/Laser-Plasma_ontology#species_density_ratio">
        <rdfs:subPropertyOf rdf:resource="http://www.semanticweb.org/afshar87/ontologies/2024/3/Laser-Plasma_ontology#species_properties"/>
        <rdfs:domain rdf:resource="http://www.semanticweb.org/afshar87/ontologies/2024/3/Laser-Plasma_ontology#Species"/>
        <rdfs:range rdf:resource="http://www.w3.org/2001/XMLSchema#float"/>
        <rdfs:comment>the ratio of the density of a particular species in the simulation to a reference density. It is a numerical value that helps in normalizing or scaling the density.</rdfs:comment>
    </owl:DatatypeProperty>
    


    <!-- http://www.semanticweb.org/afshar87/ontologies/2024/3/Laser-Plasma_ontology#species_energyGain -->

    <owl:DatatypeProperty rdf:about="http://www.semanticweb.org/afshar87/ontologies/2024/3/Laser-Plasma_ontology#species_energyGain">
        <rdfs:subPropertyOf rdf:resource="http://www.semanticweb.org/afshar87/ontologies/2024/3/Laser-Plasma_ontology#species_properties"/>
        <rdfs:domain rdf:resource="http://www.semanticweb.org/afshar87/ontologies/2024/3/Laser-Plasma_ontology#Laser_Plasma_Application"/>
        <rdfs:range rdf:resource="http://www.w3.org/2001/XMLSchema#double"/>
        <rdfs:comment>Energy gain refers to the increase in the kinetic energy of the accelerated particles compared to their initial kinetic energy (in case of laser-plasma before the laser interaction with target).

Factors Affecting Energy Gain:

Laser Pulse Parameters: The intensity, duration, and wavelength of the laser pulse significantly influence the acceleration process and the resulting energy gain of the particles.
Plasma Properties: The density and temperature of the target plasma can affect how efficiently the laser pulse interacts with the particles and transfers energy to them.</rdfs:comment>
    </owl:DatatypeProperty>
    


    <!-- http://www.semanticweb.org/afshar87/ontologies/2024/3/Laser-Plasma_ontology#species_mass -->

    <owl:DatatypeProperty rdf:about="http://www.semanticweb.org/afshar87/ontologies/2024/3/Laser-Plasma_ontology#species_mass">
        <rdfs:subPropertyOf rdf:resource="http://www.semanticweb.org/afshar87/ontologies/2024/3/Laser-Plasma_ontology#species_properties"/>
        <rdfs:domain rdf:resource="http://www.semanticweb.org/afshar87/ontologies/2024/3/Laser-Plasma_ontology#Species"/>
        <rdfs:range rdf:resource="http://www.w3.org/2001/XMLSchema#double"/>
        <rdfs:comment>the mass of the species in g, kg etc.</rdfs:comment>
    </owl:DatatypeProperty>
    


    <!-- http://www.semanticweb.org/afshar87/ontologies/2024/3/Laser-Plasma_ontology#species_massDensity -->

    <owl:DatatypeProperty rdf:about="http://www.semanticweb.org/afshar87/ontologies/2024/3/Laser-Plasma_ontology#species_massDensity">
        <rdfs:subPropertyOf rdf:resource="http://www.semanticweb.org/afshar87/ontologies/2024/3/Laser-Plasma_ontology#species_properties"/>
        <rdfs:domain rdf:resource="http://www.semanticweb.org/afshar87/ontologies/2024/3/Laser-Plasma_ontology#Species"/>
        <rdfs:range rdf:resource="http://www.w3.org/2001/XMLSchema#double"/>
        <rdfs:comment>mass density of a species in (e.g. kgm^-3)</rdfs:comment>
    </owl:DatatypeProperty>
    


    <!-- http://www.semanticweb.org/afshar87/ontologies/2024/3/Laser-Plasma_ontology#species_momentum -->

    <owl:DatatypeProperty rdf:about="http://www.semanticweb.org/afshar87/ontologies/2024/3/Laser-Plasma_ontology#species_momentum">
        <rdfs:subPropertyOf rdf:resource="http://www.semanticweb.org/afshar87/ontologies/2024/3/Laser-Plasma_ontology#species_properties"/>
        <rdfs:domain rdf:resource="http://www.semanticweb.org/afshar87/ontologies/2024/3/Laser-Plasma_ontology#Species"/>
        <rdfs:range rdf:resource="http://www.w3.org/2001/XMLSchema#double"/>
        <rdfs:comment>momentum of  a species suchg as electron or proton.</rdfs:comment>
    </owl:DatatypeProperty>
    


    <!-- http://www.semanticweb.org/afshar87/ontologies/2024/3/Laser-Plasma_ontology#species_name -->

    <owl:DatatypeProperty rdf:about="http://www.semanticweb.org/afshar87/ontologies/2024/3/Laser-Plasma_ontology#species_name">
        <rdfs:subPropertyOf rdf:resource="http://www.semanticweb.org/afshar87/ontologies/2024/3/Laser-Plasma_ontology#species_properties"/>
        <rdfs:domain rdf:resource="http://www.semanticweb.org/afshar87/ontologies/2024/3/Laser-Plasma_ontology#Species"/>
        <rdfs:range rdf:resource="http://www.w3.org/2001/XMLSchema#string"/>
        <rdfs:comment>the (human-readable) name of a particle species eg. proton, electron, etc</rdfs:comment>
    </owl:DatatypeProperty>
    


    <!-- http://www.semanticweb.org/afshar87/ontologies/2024/3/Laser-Plasma_ontology#species_numberDensity -->

    <owl:DatatypeProperty rdf:about="http://www.semanticweb.org/afshar87/ontologies/2024/3/Laser-Plasma_ontology#species_numberDensity">
        <rdfs:subPropertyOf rdf:resource="http://www.semanticweb.org/afshar87/ontologies/2024/3/Laser-Plasma_ontology#species_properties"/>
        <rdfs:domain rdf:resource="http://www.semanticweb.org/afshar87/ontologies/2024/3/Laser-Plasma_ontology#Species"/>
        <rdfs:range rdf:resource="http://www.w3.org/2001/XMLSchema#double"/>
        <rdfs:comment>number density of a species (m^-3,  cm^-3, etc).</rdfs:comment>
    </owl:DatatypeProperty>
    


    <!-- http://www.semanticweb.org/afshar87/ontologies/2024/3/Laser-Plasma_ontology#species_particle_shape -->

    <owl:DatatypeProperty rdf:about="http://www.semanticweb.org/afshar87/ontologies/2024/3/Laser-Plasma_ontology#species_particle_shape">
        <rdfs:subPropertyOf rdf:resource="http://www.semanticweb.org/afshar87/ontologies/2024/3/Laser-Plasma_ontology#species_properties"/>
        <rdfs:domain rdf:resource="http://www.semanticweb.org/afshar87/ontologies/2024/3/Laser-Plasma_ontology#Species"/>
        <rdfs:range rdf:resource="http://www.w3.org/2001/XMLSchema#double"/>
    </owl:DatatypeProperty>
    


    <!-- http://www.semanticweb.org/afshar87/ontologies/2024/3/Laser-Plasma_ontology#species_particle_shape_foil -->

    <owl:DatatypeProperty rdf:about="http://www.semanticweb.org/afshar87/ontologies/2024/3/Laser-Plasma_ontology#species_particle_shape_foil">
        <rdfs:subPropertyOf rdf:resource="http://www.semanticweb.org/afshar87/ontologies/2024/3/Laser-Plasma_ontology#species_particle_shape_type"/>
        <rdfs:domain rdf:resource="http://www.semanticweb.org/afshar87/ontologies/2024/3/Laser-Plasma_ontology#Species"/>
        <rdfs:range rdf:resource="http://www.w3.org/2001/XMLSchema#boolean"/>
    </owl:DatatypeProperty>
    


    <!-- http://www.semanticweb.org/afshar87/ontologies/2024/3/Laser-Plasma_ontology#species_particle_shape_gaussian -->

    <owl:DatatypeProperty rdf:about="http://www.semanticweb.org/afshar87/ontologies/2024/3/Laser-Plasma_ontology#species_particle_shape_gaussian">
        <rdfs:subPropertyOf rdf:resource="http://www.semanticweb.org/afshar87/ontologies/2024/3/Laser-Plasma_ontology#species_particle_shape_type"/>
        <rdfs:domain rdf:resource="http://www.semanticweb.org/afshar87/ontologies/2024/3/Laser-Plasma_ontology#Species"/>
        <rdfs:range rdf:resource="http://www.w3.org/2001/XMLSchema#boolean"/>
    </owl:DatatypeProperty>
    


    <!-- http://www.semanticweb.org/afshar87/ontologies/2024/3/Laser-Plasma_ontology#species_particle_shape_type -->

    <owl:DatatypeProperty rdf:about="http://www.semanticweb.org/afshar87/ontologies/2024/3/Laser-Plasma_ontology#species_particle_shape_type">
        <rdfs:subPropertyOf rdf:resource="http://www.semanticweb.org/afshar87/ontologies/2024/3/Laser-Plasma_ontology#species_particle_shape"/>
        <rdfs:domain rdf:resource="http://www.semanticweb.org/afshar87/ontologies/2024/3/Laser-Plasma_ontology#Species"/>
        <rdfs:range rdf:resource="http://www.w3.org/2001/XMLSchema#boolean"/>
        <rdfs:comment>the type of particle shape of a species used in a simulation e.g. &apos;linear&apos;, &quot;gaussian&quot;, &apos;quadratic&apos;, &apos;cubic&apos;.</rdfs:comment>
    </owl:DatatypeProperty>
    


    <!-- http://www.semanticweb.org/afshar87/ontologies/2024/3/Laser-Plasma_ontology#species_particle_shape_uniform -->

    <owl:DatatypeProperty rdf:about="http://www.semanticweb.org/afshar87/ontologies/2024/3/Laser-Plasma_ontology#species_particle_shape_uniform">
        <rdfs:subPropertyOf rdf:resource="http://www.semanticweb.org/afshar87/ontologies/2024/3/Laser-Plasma_ontology#species_particle_shape_type"/>
        <rdfs:domain rdf:resource="http://www.semanticweb.org/afshar87/ontologies/2024/3/Laser-Plasma_ontology#Species"/>
        <rdfs:range rdf:resource="http://www.w3.org/2001/XMLSchema#boolean"/>
    </owl:DatatypeProperty>
    


    <!-- http://www.semanticweb.org/afshar87/ontologies/2024/3/Laser-Plasma_ontology#species_properties -->

    <owl:DatatypeProperty rdf:about="http://www.semanticweb.org/afshar87/ontologies/2024/3/Laser-Plasma_ontology#species_properties"/>
    


    <!-- http://www.semanticweb.org/afshar87/ontologies/2024/3/Laser-Plasma_ontology#species_property -->

    <owl:DatatypeProperty rdf:about="http://www.semanticweb.org/afshar87/ontologies/2024/3/Laser-Plasma_ontology#species_property">
        <rdfs:subPropertyOf rdf:resource="http://www.semanticweb.org/afshar87/ontologies/2024/3/Laser-Plasma_ontology#species_properties"/>
        <rdfs:domain rdf:resource="http://www.semanticweb.org/afshar87/ontologies/2024/3/Laser-Plasma_ontology#Species"/>
        <rdfs:range rdf:resource="http://www.w3.org/2001/XMLSchema#string"/>
        <rdfs:comment>the properties of a species.</rdfs:comment>
    </owl:DatatypeProperty>
    


    <!-- http://www.semanticweb.org/afshar87/ontologies/2024/3/Laser-Plasma_ontology#species_temperature -->

    <owl:DatatypeProperty rdf:about="http://www.semanticweb.org/afshar87/ontologies/2024/3/Laser-Plasma_ontology#species_temperature">
        <rdfs:subPropertyOf rdf:resource="http://www.semanticweb.org/afshar87/ontologies/2024/3/Laser-Plasma_ontology#species_properties"/>
        <rdfs:domain rdf:resource="http://www.semanticweb.org/afshar87/ontologies/2024/3/Laser-Plasma_ontology#Species"/>
        <rdfs:range rdf:resource="http://www.w3.org/2001/XMLSchema#double"/>
        <rdfs:comment>temperature of a species  in Kelvin, Celsius etc.</rdfs:comment>
    </owl:DatatypeProperty>
    


    <!-- http://www.semanticweb.org/afshar87/ontologies/2024/3/Laser-Plasma_ontology#species_temperature_ev -->

    <owl:DatatypeProperty rdf:about="http://www.semanticweb.org/afshar87/ontologies/2024/3/Laser-Plasma_ontology#species_temperature_ev">
        <rdfs:subPropertyOf rdf:resource="http://www.semanticweb.org/afshar87/ontologies/2024/3/Laser-Plasma_ontology#species_properties"/>
        <rdfs:domain rdf:resource="http://www.semanticweb.org/afshar87/ontologies/2024/3/Laser-Plasma_ontology#Species"/>
        <rdfs:range rdf:resource="http://www.w3.org/2001/XMLSchema#double"/>
        <rdfs:comment>temperature of a species  in ev</rdfs:comment>
    </owl:DatatypeProperty>
    


    <!-- http://www.semanticweb.org/afshar87/ontologies/2024/3/Laser-Plasma_ontology#species_trajectory -->

    <owl:DatatypeProperty rdf:about="http://www.semanticweb.org/afshar87/ontologies/2024/3/Laser-Plasma_ontology#species_trajectory">
        <rdfs:subPropertyOf rdf:resource="http://www.semanticweb.org/afshar87/ontologies/2024/3/Laser-Plasma_ontology#species_properties"/>
        <rdfs:domain rdf:resource="http://www.semanticweb.org/afshar87/ontologies/2024/3/Laser-Plasma_ontology#Species"/>
        <rdfs:range rdf:resource="http://www.w3.org/2001/XMLSchema#float"/>
        <rdfs:comment>The trajectories of a species that are output in simulation studies.</rdfs:comment>
    </owl:DatatypeProperty>
    


    <!-- http://www.semanticweb.org/afshar87/ontologies/2024/3/Laser-Plasma_ontology#species_typename -->

    <owl:DatatypeProperty rdf:about="http://www.semanticweb.org/afshar87/ontologies/2024/3/Laser-Plasma_ontology#species_typename">
        <rdfs:subPropertyOf rdf:resource="http://www.semanticweb.org/afshar87/ontologies/2024/3/Laser-Plasma_ontology#species_properties"/>
        <rdfs:domain rdf:resource="http://www.semanticweb.org/afshar87/ontologies/2024/3/Laser-Plasma_ontology#Species"/>
        <rdfs:range rdf:resource="http://www.w3.org/2001/XMLSchema#string"/>
        <rdfs:comment>the (code based-readable) name of a particle species eg. proton, electron, etc. 

In PIConGPU for instance we have : This property defines the name of the C++ species type associated with the species (https://github.com/ComputationalRadiationPhysics/picongpu/blob/dev/share/picongpu/pypicongpu/schema/species/species.Species.json)</rdfs:comment>
    </owl:DatatypeProperty>
    


    <!-- http://www.semanticweb.org/afshar87/ontologies/2024/3/Laser-Plasma_ontology#target_boiling-point -->

    <owl:DatatypeProperty rdf:about="http://www.semanticweb.org/afshar87/ontologies/2024/3/Laser-Plasma_ontology#target_boiling-point">
        <rdfs:subPropertyOf rdf:resource="http://www.semanticweb.org/afshar87/ontologies/2024/3/Laser-Plasma_ontology#target_properties"/>
        <rdfs:domain rdf:resource="http://www.semanticweb.org/afshar87/ontologies/2024/3/Laser-Plasma_ontology#Target"/>
        <rdfs:range rdf:resource="http://www.w3.org/2001/XMLSchema#float"/>
        <rdfs:comment>the temperature at which the vapor pressure of a liquid equals the pressure surrounding the liquid and the liquid changes into a vapor.</rdfs:comment>
    </owl:DatatypeProperty>
    


    <!-- http://www.semanticweb.org/afshar87/ontologies/2024/3/Laser-Plasma_ontology#target_chemical_symbol -->

    <owl:DatatypeProperty rdf:about="http://www.semanticweb.org/afshar87/ontologies/2024/3/Laser-Plasma_ontology#target_chemical_symbol">
        <rdfs:subPropertyOf rdf:resource="http://www.semanticweb.org/afshar87/ontologies/2024/3/Laser-Plasma_ontology#target_properties"/>
        <rdfs:domain rdf:resource="http://www.semanticweb.org/afshar87/ontologies/2024/3/Laser-Plasma_ontology#Target"/>
        <rdfs:range rdf:resource="http://www.w3.org/2001/XMLSchema#string"/>
        <rdfs:comment>chemical formula (e.g., &quot;Au&quot; for gold, &quot;Cu&quot; for copper,  CH2 for polyethylene, and C5O2H8for polymethylmethacrylate).</rdfs:comment>
    </owl:DatatypeProperty>
    


    <!-- http://www.semanticweb.org/afshar87/ontologies/2024/3/Laser-Plasma_ontology#target_density -->

    <owl:DatatypeProperty rdf:about="http://www.semanticweb.org/afshar87/ontologies/2024/3/Laser-Plasma_ontology#target_density">
        <rdfs:subPropertyOf rdf:resource="http://www.semanticweb.org/afshar87/ontologies/2024/3/Laser-Plasma_ontology#target_properties"/>
        <rdfs:domain rdf:resource="http://www.semanticweb.org/afshar87/ontologies/2024/3/Laser-Plasma_ontology#Target"/>
        <rdfs:range rdf:resource="http://www.w3.org/2001/XMLSchema#double"/>
        <rdfs:comment>the density of a target (e.g. kgm^-3)</rdfs:comment>
    </owl:DatatypeProperty>
    


    <!-- http://www.semanticweb.org/afshar87/ontologies/2024/3/Laser-Plasma_ontology#target_electricalConductivity -->

    <owl:DatatypeProperty rdf:about="http://www.semanticweb.org/afshar87/ontologies/2024/3/Laser-Plasma_ontology#target_electricalConductivity">
        <rdfs:subPropertyOf rdf:resource="http://www.semanticweb.org/afshar87/ontologies/2024/3/Laser-Plasma_ontology#target_properties"/>
        <rdfs:domain rdf:resource="http://www.semanticweb.org/afshar87/ontologies/2024/3/Laser-Plasma_ontology#Laser_Plasma_Application"/>
        <rdfs:range rdf:resource="http://www.w3.org/2001/XMLSchema#double"/>
        <rdfs:comment>Electrical conductivity of the target (often expressed in S/m).</rdfs:comment>
    </owl:DatatypeProperty>
    


    <!-- http://www.semanticweb.org/afshar87/ontologies/2024/3/Laser-Plasma_ontology#target_material-name -->

    <owl:DatatypeProperty rdf:about="http://www.semanticweb.org/afshar87/ontologies/2024/3/Laser-Plasma_ontology#target_material-name">
        <rdfs:subPropertyOf rdf:resource="http://www.semanticweb.org/afshar87/ontologies/2024/3/Laser-Plasma_ontology#target_properties"/>
        <rdfs:domain rdf:resource="http://www.semanticweb.org/afshar87/ontologies/2024/3/Laser-Plasma_ontology#Target"/>
        <rdfs:range rdf:resource="http://www.w3.org/2001/XMLSchema#string"/>
        <rdfs:comment>the name of the material of a target (e.g., Gold, Aluminum).</rdfs:comment>
    </owl:DatatypeProperty>
    


    <!-- http://www.semanticweb.org/afshar87/ontologies/2024/3/Laser-Plasma_ontology#target_melting-point -->

    <owl:DatatypeProperty rdf:about="http://www.semanticweb.org/afshar87/ontologies/2024/3/Laser-Plasma_ontology#target_melting-point">
        <rdfs:subPropertyOf rdf:resource="http://www.semanticweb.org/afshar87/ontologies/2024/3/Laser-Plasma_ontology#target_properties"/>
        <rdfs:domain rdf:resource="http://www.semanticweb.org/afshar87/ontologies/2024/3/Laser-Plasma_ontology#Target"/>
        <rdfs:range rdf:resource="http://www.w3.org/2001/XMLSchema#float"/>
        <rdfs:comment>the temperature at which target changes state from solid to liquid.</rdfs:comment>
    </owl:DatatypeProperty>
    


    <!-- http://www.semanticweb.org/afshar87/ontologies/2024/3/Laser-Plasma_ontology#target_phase -->

    <owl:DatatypeProperty rdf:about="http://www.semanticweb.org/afshar87/ontologies/2024/3/Laser-Plasma_ontology#target_phase">
        <rdfs:subPropertyOf rdf:resource="http://www.semanticweb.org/afshar87/ontologies/2024/3/Laser-Plasma_ontology#target_properties"/>
        <rdfs:domain rdf:resource="http://www.semanticweb.org/afshar87/ontologies/2024/3/Laser-Plasma_ontology#Target"/>
        <rdfs:range rdf:resource="http://www.w3.org/2001/XMLSchema#string"/>
        <rdfs:comment>the phase of the target: solid. liquid, gas</rdfs:comment>
    </owl:DatatypeProperty>
    


    <!-- http://www.semanticweb.org/afshar87/ontologies/2024/3/Laser-Plasma_ontology#target_properties -->

    <owl:DatatypeProperty rdf:about="http://www.semanticweb.org/afshar87/ontologies/2024/3/Laser-Plasma_ontology#target_properties"/>
    


    <!-- http://www.semanticweb.org/afshar87/ontologies/2024/3/Laser-Plasma_ontology#target_specificheat_capacity -->

    <owl:DatatypeProperty rdf:about="http://www.semanticweb.org/afshar87/ontologies/2024/3/Laser-Plasma_ontology#target_specificheat_capacity">
        <rdfs:subPropertyOf rdf:resource="http://www.semanticweb.org/afshar87/ontologies/2024/3/Laser-Plasma_ontology#target_properties"/>
        <rdfs:domain rdf:resource="http://www.semanticweb.org/afshar87/ontologies/2024/3/Laser-Plasma_ontology#Target"/>
        <rdfs:range rdf:resource="http://www.w3.org/2001/XMLSchema#double"/>
        <rdfs:comment>the amount of heat that must be added to one unit of mass of the substance in order to cause an increase of one unit in temperature.</rdfs:comment>
    </owl:DatatypeProperty>
    


    <!-- http://www.semanticweb.org/afshar87/ontologies/2024/3/Laser-Plasma_ontology#target_temperature -->

    <owl:DatatypeProperty rdf:about="http://www.semanticweb.org/afshar87/ontologies/2024/3/Laser-Plasma_ontology#target_temperature">
        <rdfs:subPropertyOf rdf:resource="http://www.semanticweb.org/afshar87/ontologies/2024/3/Laser-Plasma_ontology#target_properties"/>
        <rdfs:domain rdf:resource="http://www.semanticweb.org/afshar87/ontologies/2024/3/Laser-Plasma_ontology#Target"/>
        <rdfs:range rdf:resource="http://www.w3.org/2001/XMLSchema#double"/>
        <rdfs:comment>temperature of a target  in Kelvin, Celsius etc.</rdfs:comment>
    </owl:DatatypeProperty>
    


    <!-- http://www.semanticweb.org/afshar87/ontologies/2024/3/Laser-Plasma_ontology#target_thermalConductivity -->

    <owl:DatatypeProperty rdf:about="http://www.semanticweb.org/afshar87/ontologies/2024/3/Laser-Plasma_ontology#target_thermalConductivity">
        <rdfs:subPropertyOf rdf:resource="http://www.semanticweb.org/afshar87/ontologies/2024/3/Laser-Plasma_ontology#target_properties"/>
        <rdfs:domain rdf:resource="http://www.semanticweb.org/afshar87/ontologies/2024/3/Laser-Plasma_ontology#Laser_Plasma_Application"/>
        <rdfs:range rdf:resource="http://www.w3.org/2001/XMLSchema#double"/>
        <rdfs:comment>Thermal conductivity of the target (often expressed in W/m*K).</rdfs:comment>
    </owl:DatatypeProperty>
    


    <!-- http://www.semanticweb.org/afshar87/ontologies/2024/3/Laser-Plasma_ontology#target_thickness -->

    <owl:DatatypeProperty rdf:about="http://www.semanticweb.org/afshar87/ontologies/2024/3/Laser-Plasma_ontology#target_thickness">
        <rdfs:subPropertyOf rdf:resource="http://www.semanticweb.org/afshar87/ontologies/2024/3/Laser-Plasma_ontology#target_properties"/>
        <rdfs:domain rdf:resource="http://www.semanticweb.org/afshar87/ontologies/2024/3/Laser-Plasma_ontology#Target"/>
        <rdfs:range rdf:resource="http://www.w3.org/2001/XMLSchema#double"/>
        <rdfs:comment>target thickness</rdfs:comment>
    </owl:DatatypeProperty>
    


    <!-- http://www.semanticweb.org/afshar87/ontologies/2024/3/Laser-Plasma_ontology#Equation_Of_State_(EOS)_Formula -->

    <owl:DatatypeProperty rdf:about="http://www.semanticweb.org/afshar87/ontologies/2024/3/Laser-Plasma_ontology#Equation_Of_State_(EOS)_Formula">
        <rdfs:subPropertyOf rdf:resource="http://www.semanticweb.org/afshar87/ontologies/2024/3/Laser-Plasma_ontology#plasma_properties"/>
        <rdfs:domain rdf:resource="http://www.semanticweb.org/afshar87/ontologies/2024/3/Laser-Plasma_ontology#Plasma"/>
        <rdfs:range rdf:resource="http://www.w3.org/2001/XMLSchema#string"/>
        <rdfs:comment>Reference to the specific equation of state used to describe the plasma.</rdfs:comment>
    </owl:DatatypeProperty>
    


    <!-- http://www.semanticweb.org/afshar87/ontologies/2024/3/Laser-Plasma_ontology#LG_azimuthal_index_(l) -->

    <owl:DatatypeProperty rdf:about="http://www.semanticweb.org/afshar87/ontologies/2024/3/Laser-Plasma_ontology#LG_azimuthal_index_(l)">
        <rdfs:subPropertyOf rdf:resource="http://www.semanticweb.org/afshar87/ontologies/2024/3/Laser-Plasma_ontology#laser_Laguerre-Gaussian_mode_(LG)"/>
        <rdfs:domain rdf:resource="http://www.semanticweb.org/afshar87/ontologies/2024/3/Laser-Plasma_ontology#Laser"/>
        <rdfs:range rdf:resource="http://www.w3.org/2001/XMLSchema#float"/>
        <rdfs:comment>LG modes are a specific type of spatial mode of a laser beam characterized by a helical phase front, resulting in a doughnut-shaped intensity profile.
The LG modes are defined by two indices: the azimuthal mode index  l (related to the orbital angular momentum) and the radial mode index  p (related to the number of radial nodes).</rdfs:comment>
    </owl:DatatypeProperty>
    


    <!-- http://www.semanticweb.org/afshar87/ontologies/2024/3/Laser-Plasma_ontology#LG_radial_index_(p) -->

    <owl:DatatypeProperty rdf:about="http://www.semanticweb.org/afshar87/ontologies/2024/3/Laser-Plasma_ontology#LG_radial_index_(p)">
        <rdfs:subPropertyOf rdf:resource="http://www.semanticweb.org/afshar87/ontologies/2024/3/Laser-Plasma_ontology#laser_Laguerre-Gaussian_mode_(LG)"/>
        <rdfs:domain rdf:resource="http://www.semanticweb.org/afshar87/ontologies/2024/3/Laser-Plasma_ontology#Laser"/>
        <rdfs:range rdf:resource="http://www.w3.org/2001/XMLSchema#float"/>
        <rdfs:comment>LG modes are a specific type of spatial mode of a laser beam characterized by a helical phase front, resulting in a doughnut-shaped intensity profile.
The LG modes are defined by two indices: the azimuthal mode index  l (related to the orbital angular momentum) and the radial mode index  p (related to the number of radial nodes).</rdfs:comment>
    </owl:DatatypeProperty>
    


    <!-- http://www.semanticweb.org/afshar87/ontologies/2024/3/Laser-Plasma_ontology#current_density_(J) -->

    <owl:DatatypeProperty rdf:about="http://www.semanticweb.org/afshar87/ontologies/2024/3/Laser-Plasma_ontology#current_density_(J)">
        <rdfs:subPropertyOf rdf:resource="http://www.semanticweb.org/afshar87/ontologies/2024/3/Laser-Plasma_ontology#plasma_properties"/>
        <rdfs:domain rdf:resource="http://www.semanticweb.org/afshar87/ontologies/2024/3/Laser-Plasma_ontology#Laser_Plasma_Physics"/>
        <rdfs:range rdf:resource="http://www.w3.org/2001/XMLSchema#double"/>
        <rdfs:comment>Current Density (J):

This quantity represents the flow of electric charge per unit area within the plasma. It&apos;s measured in amperes per square meter (A/m^2).

Generation of J in LPP:

When a high-intensity laser pulse interacts with a target, it ionizes the material, creating a plasma with free electrons and ions.
The intense electric field of the laser pulse can then exert a force on these free electrons, causing them to drift and generate a current within the plasma.
Influence of J on LPP Processes:

J plays a significant role in various LPP phenomena, including:

Magnetic Field Generation: The flow of current creates a magnetic field within the plasma. This magnetic field can influence the propagation of the laser pulse itself and impact the dynamics of particle acceleration (electrons and ions).

Plasma Instabilities: High current densities can lead to the development of various plasma instabilities, which are rapid fluctuations in the plasma density and electric field. These instabilities can further influence particle acceleration and energy transfer processes within the plasma.

Particle Acceleration: The magnetic field generated by J can trap and accelerate charged particles (electrons and ions) within the plasma. This is a crucial aspect of various LPP applications, such as laser wakefield acceleration for electron beams.</rdfs:comment>
    </owl:DatatypeProperty>
    


    <!-- http://www.semanticweb.org/afshar87/ontologies/2024/3/Laser-Plasma_ontology#electric_field_(E) -->

    <owl:DatatypeProperty rdf:about="http://www.semanticweb.org/afshar87/ontologies/2024/3/Laser-Plasma_ontology#electric_field_(E)">
        <rdfs:subPropertyOf rdf:resource="http://www.semanticweb.org/afshar87/ontologies/2024/3/Laser-Plasma_ontology#electromagnetic_fields"/>
        <rdfs:domain rdf:resource="http://www.semanticweb.org/afshar87/ontologies/2024/3/Laser-Plasma_ontology#Plasma"/>
        <rdfs:range rdf:resource="http://www.w3.org/2001/XMLSchema#double"/>
        <rdfs:range rdf:resource="http://www.w3.org/2001/XMLSchema#string"/>
    </owl:DatatypeProperty>
    


    <!-- http://www.semanticweb.org/afshar87/ontologies/2024/3/Laser-Plasma_ontology#laser_Laguerre-Gaussian_mode_(LG) -->

    <owl:DatatypeProperty rdf:about="http://www.semanticweb.org/afshar87/ontologies/2024/3/Laser-Plasma_ontology#laser_Laguerre-Gaussian_mode_(LG)">
        <rdfs:subPropertyOf rdf:resource="http://www.semanticweb.org/afshar87/ontologies/2024/3/Laser-Plasma_ontology#laser_beam"/>
        <rdfs:domain rdf:resource="http://www.semanticweb.org/afshar87/ontologies/2024/3/Laser-Plasma_ontology#Laser"/>
        <rdfs:range rdf:resource="http://www.w3.org/2001/XMLSchema#float"/>
        <rdfs:comment>Laguerre-Gaussian (LG) modes are a family of solutions to the paraxial wave equation in cylindrical coordinates. These modes represent solutions where the electric field intensity and phase vary both radially and azimuthally in the transverse plane. They are named after the Laguerre polynomials which describe their radial dependence.

Characteristics of Laguerre-Gaussian Modes:
Radial and Azimuthal Dependence:
Laguerre-Gaussian modes exhibit both radial and azimuthal dependence in the transverse plane. The radial dependence is described by Laguerre polynomials, while the azimuthal dependence is represented by a phase factor e^(ilÏ•), where ð‘™ is the azimuthal mode index.

Doughnut-Shaped Intensity Profile:
Laguerre-Gaussian modes typically have a doughnut-shaped intensity profile in the transverse plane. The intensity is highest at the outer ring of the doughnut and decreases towards the center.

Non-Zero Orbital Angular Momentum (OAM):
Laguerre-Gaussian modes carry non-zero orbital angular momentum due to their azimuthal phase dependence. The value of  ð‘™ determines the amount of OAM carried by the mode.

Infinite Family of Modes:
Laguerre-Gaussian modes form an infinite family of solutions, characterized by two integers: the radial index p and the azimuthal index ð‘™. Different combinations of 
p and l yield different Laguerre-Gaussian modes, each with its unique intensity and phase distribution.</rdfs:comment>
    </owl:DatatypeProperty>
    


    <!-- http://www.semanticweb.org/afshar87/ontologies/2024/3/Laser-Plasma_ontology#magnetic_field_(B) -->

    <owl:DatatypeProperty rdf:about="http://www.semanticweb.org/afshar87/ontologies/2024/3/Laser-Plasma_ontology#magnetic_field_(B)">
        <rdfs:subPropertyOf rdf:resource="http://www.semanticweb.org/afshar87/ontologies/2024/3/Laser-Plasma_ontology#electromagnetic_fields"/>
        <rdfs:domain rdf:resource="http://www.semanticweb.org/afshar87/ontologies/2024/3/Laser-Plasma_ontology#Plasma"/>
        <rdfs:range rdf:resource="http://www.w3.org/2001/XMLSchema#double"/>
        <rdfs:range rdf:resource="http://www.w3.org/2001/XMLSchema#string"/>
    </owl:DatatypeProperty>
    


    <!-- http://www.semanticweb.org/afshar87/ontologies/2024/3/Laser-Plasma_ontology#project_Principal_Investigator_(PI) -->

    <owl:DatatypeProperty rdf:about="http://www.semanticweb.org/afshar87/ontologies/2024/3/Laser-Plasma_ontology#project_Principal_Investigator_(PI)">
        <rdfs:subPropertyOf rdf:resource="http://www.semanticweb.org/afshar87/ontologies/2024/3/Laser-Plasma_ontology#project_property"/>
        <rdfs:domain rdf:resource="http://www.semanticweb.org/afshar87/ontologies/2024/3/Laser-Plasma_ontology#Project"/>
        <rdfs:range rdf:resource="http://www.w3.org/2001/XMLSchema#string"/>
        <rdfs:comment>The Principal Investigator of a project (either simulation or experiment).</rdfs:comment>
    </owl:DatatypeProperty>
    


    <!-- http://www.w3.org/2002/07/owl#topDataProperty -->

    <rdf:Description rdf:about="http://www.w3.org/2002/07/owl#topDataProperty">
        <rdfs:subPropertyOf rdf:resource="http://www.semanticweb.org/afshar87/ontologies/2024/3/Laser-Plasma_ontology#data_property"/>
    </rdf:Description>
    


    <!-- 
    ///////////////////////////////////////////////////////////////////////////////////////
    //
    // Classes
    //
    ///////////////////////////////////////////////////////////////////////////////////////
     -->

    


    <!-- http://www.semanticweb.org/afshar87/ontologies/2024/3/Laser-Plasma_ontology#Avalanche_Ionization -->

    <owl:Class rdf:about="http://www.semanticweb.org/afshar87/ontologies/2024/3/Laser-Plasma_ontology#Avalanche_Ionization">
        <rdfs:subClassOf rdf:resource="http://www.semanticweb.org/afshar87/ontologies/2024/3/Laser-Plasma_ontology#Ionization"/>
        <rdfs:comment>Secondary electrons from initial ionization events create further ionization.</rdfs:comment>
    </owl:Class>
    


    <!-- http://www.semanticweb.org/afshar87/ontologies/2024/3/Laser-Plasma_ontology#BoundaryConditionType -->

    <owl:Class rdf:about="http://www.semanticweb.org/afshar87/ontologies/2024/3/Laser-Plasma_ontology#BoundaryConditionType">
        <rdfs:subClassOf rdf:resource="http://www.semanticweb.org/afshar87/ontologies/2024/3/Laser-Plasma_ontology#Simulation"/>
    </owl:Class>
    


    <!-- http://www.semanticweb.org/afshar87/ontologies/2024/3/Laser-Plasma_ontology#Cluster_Targets -->

    <owl:Class rdf:about="http://www.semanticweb.org/afshar87/ontologies/2024/3/Laser-Plasma_ontology#Cluster_Targets">
        <rdfs:subClassOf rdf:resource="http://www.semanticweb.org/afshar87/ontologies/2024/3/Laser-Plasma_ontology#solid__target"/>
        <rdfs:comment>Targets made of clusters of atoms are being investigated for potential advantages in terms of controlling the ion beam properties.</rdfs:comment>
    </owl:Class>
    


    <!-- http://www.semanticweb.org/afshar87/ontologies/2024/3/Laser-Plasma_ontology#Customuser_input -->

    <owl:Class rdf:about="http://www.semanticweb.org/afshar87/ontologies/2024/3/Laser-Plasma_ontology#Customuser_input">
        <rdfs:subClassOf rdf:resource="http://www.semanticweb.org/afshar87/ontologies/2024/3/Laser-Plasma_ontology#Simulation"/>
    </owl:Class>
    


    <!-- http://www.semanticweb.org/afshar87/ontologies/2024/3/Laser-Plasma_ontology#Data -->

    <owl:Class rdf:about="http://www.semanticweb.org/afshar87/ontologies/2024/3/Laser-Plasma_ontology#Data"/>
    


    <!-- http://www.semanticweb.org/afshar87/ontologies/2024/3/Laser-Plasma_ontology#Degenerate_Plasmas -->

    <owl:Class rdf:about="http://www.semanticweb.org/afshar87/ontologies/2024/3/Laser-Plasma_ontology#Degenerate_Plasmas">
        <rdfs:subClassOf rdf:resource="http://www.semanticweb.org/afshar87/ontologies/2024/3/Laser-Plasma_ontology#Warm_Dense_Matter_(WDM)"/>
        <rdfs:comment>Plasmas where the pressure is dominated by the degeneracy pressure of electrons due to the Pauli exclusion principle. This can occur at relatively low temperatures in WDM.</rdfs:comment>
    </owl:Class>
    


    <!-- http://www.semanticweb.org/afshar87/ontologies/2024/3/Laser-Plasma_ontology#Dense_Plasmas -->

    <owl:Class rdf:about="http://www.semanticweb.org/afshar87/ontologies/2024/3/Laser-Plasma_ontology#Dense_Plasmas">
        <rdfs:subClassOf rdf:resource="http://www.semanticweb.org/afshar87/ontologies/2024/3/Laser-Plasma_ontology#Warm_Dense_Matter_(WDM)"/>
        <rdfs:comment>Plasmas with high densities (typically exceeding 10^19 - 10^23 cm^-3) but not reaching the extreme densities of inertial confinement fusion plasmas.</rdfs:comment>
    </owl:Class>
    


    <!-- http://www.semanticweb.org/afshar87/ontologies/2024/3/Laser-Plasma_ontology#Diagnostics -->

    <owl:Class rdf:about="http://www.semanticweb.org/afshar87/ontologies/2024/3/Laser-Plasma_ontology#Diagnostics"/>
    


    <!-- http://www.semanticweb.org/afshar87/ontologies/2024/3/Laser-Plasma_ontology#DirectDriveFusion -->

    <owl:Class rdf:about="http://www.semanticweb.org/afshar87/ontologies/2024/3/Laser-Plasma_ontology#DirectDriveFusion">
        <rdfs:subClassOf rdf:resource="http://www.semanticweb.org/afshar87/ontologies/2024/3/Laser-Plasma_ontology#Inertial_Confinement_Fusion_(ICF)"/>
        <owl:disjointWith rdf:resource="http://www.semanticweb.org/afshar87/ontologies/2024/3/Laser-Plasma_ontology#IndirectDriveFusion"/>
    </owl:Class>
    


    <!-- http://www.semanticweb.org/afshar87/ontologies/2024/3/Laser-Plasma_ontology#Direct_Laser_Acceleration -->

    <owl:Class rdf:about="http://www.semanticweb.org/afshar87/ontologies/2024/3/Laser-Plasma_ontology#Direct_Laser_Acceleration">
        <rdfs:subClassOf rdf:resource="http://www.semanticweb.org/afshar87/ontologies/2024/3/Laser-Plasma_ontology#Laser_Particle_Acceleration"/>
        <rdfs:comment>in Direct Laser Acceleration, the laser pulse directly accelerates charged particles via the electric field of the laser.</rdfs:comment>
    </owl:Class>
    


    <!-- http://www.semanticweb.org/afshar87/ontologies/2024/3/Laser-Plasma_ontology#Electron_Beams -->

    <owl:Class rdf:about="http://www.semanticweb.org/afshar87/ontologies/2024/3/Laser-Plasma_ontology#Electron_Beams">
        <rdfs:subClassOf rdf:resource="http://www.semanticweb.org/afshar87/ontologies/2024/3/Laser-Plasma_ontology#Particle_Beam_Generation"/>
        <rdfs:comment>High-energy electron beams produced via LWFA, PWFA, or other mechanisms.</rdfs:comment>
    </owl:Class>
    


    <!-- http://www.semanticweb.org/afshar87/ontologies/2024/3/Laser-Plasma_ontology#Experiment -->

    <owl:Class rdf:about="http://www.semanticweb.org/afshar87/ontologies/2024/3/Laser-Plasma_ontology#Experiment"/>
    


    <!-- http://www.semanticweb.org/afshar87/ontologies/2024/3/Laser-Plasma_ontology#Facility -->

    <owl:Class rdf:about="http://www.semanticweb.org/afshar87/ontologies/2024/3/Laser-Plasma_ontology#Facility"/>
    


    <!-- http://www.semanticweb.org/afshar87/ontologies/2024/3/Laser-Plasma_ontology#Fast_ignition -->

    <owl:Class rdf:about="http://www.semanticweb.org/afshar87/ontologies/2024/3/Laser-Plasma_ontology#Fast_ignition">
        <rdfs:subClassOf rdf:resource="http://www.semanticweb.org/afshar87/ontologies/2024/3/Laser-Plasma_ontology#DirectDriveFusion"/>
        <owl:disjointWith rdf:resource="http://www.semanticweb.org/afshar87/ontologies/2024/3/Laser-Plasma_ontology#Shock_ignition"/>
    </owl:Class>
    


    <!-- http://www.semanticweb.org/afshar87/ontologies/2024/3/Laser-Plasma_ontology#Fourier_Transform_Interferometry -->

    <owl:Class rdf:about="http://www.semanticweb.org/afshar87/ontologies/2024/3/Laser-Plasma_ontology#Fourier_Transform_Interferometry">
        <rdfs:subClassOf rdf:resource="http://www.semanticweb.org/afshar87/ontologies/2024/3/Laser-Plasma_ontology#interferometry"/>
        <rdfs:comment>Fourier Transform Interferometry (FTI):

This technique analyzes the entire interference pattern captured by an interferometer using a mathematical approach called the Fourier transform.
By decomposing the pattern into its constituent frequencies, FTI allows for the retrieval of both the electron density and the plasma thickness information simultaneously.
This offers a more comprehensive analysis compared to traditional fringe shift analysis methods.</rdfs:comment>
    </owl:Class>
    


    <!-- http://www.semanticweb.org/afshar87/ontologies/2024/3/Laser-Plasma_ontology#Harmonic_Generation -->

    <owl:Class rdf:about="http://www.semanticweb.org/afshar87/ontologies/2024/3/Laser-Plasma_ontology#Harmonic_Generation">
        <rdfs:subClassOf rdf:resource="http://www.semanticweb.org/afshar87/ontologies/2024/3/Laser-Plasma_ontology#Laser_Plasma_Application"/>
        <rdfs:comment>Generation of coherent electromagnetic radiation at frequencies much higher than the laser frequency.</rdfs:comment>
    </owl:Class>
    


    <!-- http://www.semanticweb.org/afshar87/ontologies/2024/3/Laser-Plasma_ontology#Hybrid_Acceleration -->

    <owl:Class rdf:about="http://www.semanticweb.org/afshar87/ontologies/2024/3/Laser-Plasma_ontology#Hybrid_Acceleration">
        <rdfs:subClassOf rdf:resource="http://www.semanticweb.org/afshar87/ontologies/2024/3/Laser-Plasma_ontology#Laser_Ion_acceleration"/>
        <rdfs:comment>Combining different acceleration techniques (e.g., TNSA followed by LWFA, RPA followed by TNSA, etc) is being explored to achieve staged acceleration and potentially even higher ion energies.</rdfs:comment>
    </owl:Class>
    


    <!-- http://www.semanticweb.org/afshar87/ontologies/2024/3/Laser-Plasma_ontology#IndirectDriveFusion -->

    <owl:Class rdf:about="http://www.semanticweb.org/afshar87/ontologies/2024/3/Laser-Plasma_ontology#IndirectDriveFusion">
        <rdfs:subClassOf rdf:resource="http://www.semanticweb.org/afshar87/ontologies/2024/3/Laser-Plasma_ontology#Inertial_Confinement_Fusion_(ICF)"/>
    </owl:Class>
    


    <!-- http://www.semanticweb.org/afshar87/ontologies/2024/3/Laser-Plasma_ontology#Ion_Beams -->

    <owl:Class rdf:about="http://www.semanticweb.org/afshar87/ontologies/2024/3/Laser-Plasma_ontology#Ion_Beams">
        <rdfs:subClassOf rdf:resource="http://www.semanticweb.org/afshar87/ontologies/2024/3/Laser-Plasma_ontology#Particle_Beam_Generation"/>
        <rdfs:comment>Acceleration of ions in laser-plasma interactions.</rdfs:comment>
    </owl:Class>
    


    <!-- http://www.semanticweb.org/afshar87/ontologies/2024/3/Laser-Plasma_ontology#Ionization -->

    <owl:Class rdf:about="http://www.semanticweb.org/afshar87/ontologies/2024/3/Laser-Plasma_ontology#Ionization">
        <rdfs:subClassOf rdf:resource="http://www.semanticweb.org/afshar87/ontologies/2024/3/Laser-Plasma_ontology#Laser_Plasma_Physics"/>
    </owl:Class>
    


    <!-- http://www.semanticweb.org/afshar87/ontologies/2024/3/Laser-Plasma_ontology#LWFA_Ionization_Injection -->

    <owl:Class rdf:about="http://www.semanticweb.org/afshar87/ontologies/2024/3/Laser-Plasma_ontology#LWFA_Ionization_Injection">
        <rdfs:subClassOf rdf:resource="http://www.semanticweb.org/afshar87/ontologies/2024/3/Laser-Plasma_ontology#LWFA_(Laser_Wakefield_Acceleration)"/>
        <rdfs:comment>Ionization Injection is a method used in Laser Wakefield Acceleration (LWFA) to introduce electrons into the plasma wakefield for subsequent acceleration. This technique relies on the ionization of a high-Z (high atomic number) gas mixed with a lower-Z background gas within the plasma. The ionization injection process leverages the electric fields of the wake to ionize inner-shell electrons, which are then trapped and accelerated by the wakefield.

Process
Wakefield Creation:

A high-intensity laser pulse travels through a plasma, generating a wakefield. The wakefield is a moving structure of electric fields capable of accelerating charged particles.
Gas Mixture:

The plasma consists of a mixture of low-Z and high-Z gases. The high-Z gas has inner-shell electrons that can be ionized with the appropriate laser intensity.
High-Intensity Laser Pulse:

As the laser pulse propagates through the plasma, its intensity is sufficient to ionize the inner-shell electrons of the high-Z gas.
Ionization and Electron Capture:

The ionization occurs within the high electric fields of the wakefield. The freed electrons are injected into the accelerating phase of the wakefield due to the ionization process, resulting in their capture and subsequent acceleration.
Key Characteristics
Inner-Shell Electron Ionization:
The method involves ionizing inner-shell electrons of the high-Z gas, which are initially bound more tightly than outer-shell electrons.
Controlled Injection:
The timing and position of the electron injection are controlled by the ionization process, leading to precise injection into the accelerating phase of the wakefield.
Single Laser Setup:
Typically requires only one high-intensity laser pulse, simplifying the experimental setup compared to methods that require multiple lasers.
Advantages
Simpler Setup:
Uses a single laser pulse, making the experimental setup less complex and more cost-effective compared to methods requiring synchronized multiple lasers.
Effective Control:
Provides good control over the injection process, leading to high-quality electron beams with desirable properties like low emittance and narrow energy spread.
Disadvantages
Laser Intensity Requirement:
Requires very high-intensity laser pulses to ionize the inner-shell electrons of the high-Z gas effectively.
Precision:
While providing good control, it may not achieve the same level of precision in electron injection as methods like Trojan Horse Injection.
Applications
Advanced Research:
Suitable for experiments in particle physics, where high-quality electron beams are needed.
Medical and Industrial Applications:
Can be used in radiation therapy and material science, where controlled, high-quality electron beams are beneficial.</rdfs:comment>
    </owl:Class>
    


    <!-- http://www.semanticweb.org/afshar87/ontologies/2024/3/Laser-Plasma_ontology#LWFA_Self-Injection -->

    <owl:Class rdf:about="http://www.semanticweb.org/afshar87/ontologies/2024/3/Laser-Plasma_ontology#LWFA_Self-Injection">
        <rdfs:subClassOf rdf:resource="http://www.semanticweb.org/afshar87/ontologies/2024/3/Laser-Plasma_ontology#LWFA_(Laser_Wakefield_Acceleration)"/>
        <rdfs:comment>Self-Injection is a process in Laser Wakefield Acceleration (LWFA) where electrons from the plasma are naturally trapped and accelerated by the wakefield generated by an intense laser pulse. Unlike other methods that require precise timing or additional laser pulses for injection, self-injection relies on the intrinsic dynamics of the plasma wakefield.

Process
Wakefield Generation:

A high-intensity laser pulse propagates through a plasma, creating a wakefield. This wakefield consists of strong electric fields that can accelerate charged particles.
Nonlinear Wakefield Evolution:

As the laser pulse travels through the plasma, it can drive the plasma electrons to such high velocities that they form a bubble-like structure (also known as a &quot;blowout&quot; or &quot;bubble&quot; regime) behind the laser pulse.
Electron Trapping:

In certain conditions, such as when the laser intensity is sufficiently high or the plasma density is optimized, some plasma electrons gain enough energy from the wakefield to become trapped within the accelerating phase of the wake.
These electrons are then continuously accelerated by the wakefield as the laser pulse propagates.
Acceleration:

The trapped electrons are accelerated to high energies within the wakefield, resulting in a high-energy electron beam.
Key Characteristics
Intrinsic Process:
Self-injection occurs naturally without the need for additional lasers or complex setups. It depends on the inherent properties of the plasma and the laser pulse.
Nonlinear Regime:
Typically occurs in the highly nonlinear regime of wakefield generation, where the laser intensity and plasma density create a strong wakefield capable of trapping electrons.
Threshold Conditions:
There are specific conditions (such as laser intensity, plasma density, and pulse duration) that need to be met for effective self-injection to occur.
Advantages
Simplicity:
Requires only a single high-intensity laser pulse, making the experimental setup straightforward and less costly compared to methods requiring synchronized multiple lasers.
Natural Process:
Takes advantage of the natural dynamics of the wakefield, potentially leading to high-energy electron beams without intricate control mechanisms.
Disadvantages
Less Control:
Provides less precise control over the injection process compared to methods like Trojan Horse Injection or Shock-Front Injection. This can result in broader energy spreads and higher emittance in the accelerated electron beam.
Threshold Dependency:
Highly dependent on specific conditions, which means it might be less reliable or reproducible across different experimental setups.</rdfs:comment>
    </owl:Class>
    


    <!-- http://www.semanticweb.org/afshar87/ontologies/2024/3/Laser-Plasma_ontology#LWFA_Trojan_Horse_Injection -->

    <owl:Class rdf:about="http://www.semanticweb.org/afshar87/ontologies/2024/3/Laser-Plasma_ontology#LWFA_Trojan_Horse_Injection">
        <rdfs:subClassOf rdf:resource="http://www.semanticweb.org/afshar87/ontologies/2024/3/Laser-Plasma_ontology#LWFA_(Laser_Wakefield_Acceleration)"/>
        <rdfs:comment>Trojan Horse Injection is an advanced technique used in Laser Wakefield Acceleration (LWFA) to precisely inject electrons into a plasma wakefield for subsequent acceleration. This method leverages the interaction of two laser pulses to achieve highly controlled electron injection, which results in electron beams with superior qualities such as low emittance, narrow energy spread, and high brightness.

Process
Primary Laser Pulse: A high-intensity laser pulse propagates through a plasma, creating a wakefield, which is a traveling electric field capable of accelerating electrons.

Secondary Laser Pulse: A second, lower-intensity laser pulse is introduced at a specific timing and location to ionize inner-shell electrons from a dopant gas (such as helium or nitrogen) that is mixed with the main plasma.

Inner-Shell Ionization: The secondary laser pulse ionizes these inner-shell electrons within the wakefield of the primary laser. The freed electrons are then immediately trapped and accelerated by the wakefield.

Controlled Injection: Because the secondary laser pulse can be precisely timed and positioned, the injection of electrons into the wakefield can be controlled with high precision. This results in the production of electron beams with very desirable properties for various applications.

Key Characteristics
Ionization of Inner-Shell Electrons: Unlike other methods that might ionize outer-shell electrons, the Trojan Horse method focuses on inner-shell electrons. These electrons require more energy to be ionized but offer better control over the injection process.
Precision Control: The use of a secondary laser pulse allows for precise control over the injection process. This enables the creation of electron beams with specific characteristics tailored to the needs of the experiment.
Two-Laser Setup: This method requires two synchronized laser pulses: a primary pulse to create the wakefield and a secondary pulse to ionize the electrons.
Advantages
High Beam Quality: Produces electron beams with low emittance, narrow energy spread, and high brightness, which are ideal for high-precision applications.
Controlled Injection: Provides excellent control over the timing and location of electron injection, leading to better predictability and stability in the accelerated electron beams.
Disadvantages
Complex Setup: Requires a sophisticated experimental setup with two synchronized laser pulses, which can be more complex and expensive than single-laser methods.
Synchronization Requirement: The precise synchronization of the two laser pulses is critical, adding to the technical challenge.</rdfs:comment>
    </owl:Class>
    


    <!-- http://www.semanticweb.org/afshar87/ontologies/2024/3/Laser-Plasma_ontology#LWFA_shock-front_Injection -->

    <owl:Class rdf:about="http://www.semanticweb.org/afshar87/ontologies/2024/3/Laser-Plasma_ontology#LWFA_shock-front_Injection">
        <rdfs:subClassOf rdf:resource="http://www.semanticweb.org/afshar87/ontologies/2024/3/Laser-Plasma_ontology#LWFA_(Laser_Wakefield_Acceleration)"/>
        <rdfs:comment>Laser Wakefield Acceleration (LWFA) with Shock-Front Injection is a method used in the field of particle acceleration, particularly within the context of laser-plasma interactions. In this technique, an intense laser pulse is employed to generate a plasma wakefield, which is then utilized to accelerate charged particles, such as electrons, to high energies over relatively short distances. The &quot;shock-front injection&quot; aspect refers to a specific mechanism for injecting electrons into the wakefield, enhancing the acceleration process and enabling the generation of high-quality, high-energy particle beams.

Key Concepts of LWFA with Shock-Front Injection:
Laser-Plasma Interaction:

Laser Pulse: A high-intensity laser pulse is focused onto a dense plasma, typically created by a gas jet or solid target. The intense electric field of the laser pulse ionizes the plasma, creating a plasma channel or bubble.
Plasma Wakefield: As the laser pulse propagates through the plasma, it drives electrons out of the interaction region, leaving behind a region of positively charged ions. This creates a strong electric field structure called a wakefield.
Shock-Front Injection:

Injection Mechanism: In shock-front injection, a secondary laser pulse or a pre-existing shockwave is employed to inject electrons into the wakefield. This injection process occurs at the front or leading edge of the wakefield.
Enhanced Acceleration: Shock-front injection enhances the acceleration process by providing a source of electrons that can be efficiently trapped and accelerated by the wakefield. This results in the generation of high-quality electron beams with high energies and narrow energy spreads.
Acceleration Dynamics:

Injection Timing: The timing of the injection pulse or shockwave is crucial for efficient electron injection into the wakefield. By synchronizing the injection with the formation of the wakefield, electrons can be injected into the accelerating structure at optimal conditions.
Self-Trapping and Acceleration: Electrons injected via shock-front injection are self-trapped within the wakefield and undergo acceleration to relativistic energies as they travel along the wakefield structure.

Advantages:

Controlled Injection: Shock-front injection allows for localized and controlled injection.
Flexibility: Can be used with various plasma densities and laser parameters.
Disadvantages:

Setup Complexity: Requires precise creation and timing of the shock front.
Synchronization: Needs accurate synchronization between the laser pulse and the shock front.</rdfs:comment>
    </owl:Class>
    


    <!-- http://www.semanticweb.org/afshar87/ontologies/2024/3/Laser-Plasma_ontology#Laboratory_Astrophysics -->

    <owl:Class rdf:about="http://www.semanticweb.org/afshar87/ontologies/2024/3/Laser-Plasma_ontology#Laboratory_Astrophysics">
        <rdfs:subClassOf rdf:resource="http://www.semanticweb.org/afshar87/ontologies/2024/3/Laser-Plasma_ontology#Laser_Plasma_Application"/>
        <rdfs:comment>Laboratory astrophysics in laser plasma refers to the study of astrophysical phenomena through experimental simulations conducted in laboratory settings using high-power lasers and plasma physics techniques.

Key Aspects:
Simulation of Astrophysical Environments: Laboratory astrophysics aims to recreate the extreme conditions found in astrophysical environments, such as those in stars, supernovae, accretion disks, and cosmic jets. High-power lasers are used to generate plasma with temperatures, densities, and magnetic fields similar to those observed in space.

Understanding Fundamental Processes: By recreating astrophysical conditions in the laboratory, scientists can study fundamental processes such as plasma dynamics, particle acceleration, magnetic reconnection, shock formation, and turbulence. These processes play crucial roles in shaping the dynamics and evolution of astrophysical systems.

Probing Cosmic Phenomena: Laboratory experiments allow researchers to probe and validate theoretical models of various astrophysical phenomena. By comparing observational data from space telescopes with laboratory results, scientists can gain insights into the underlying physical mechanisms driving cosmic events.

Applications to Space Missions: Findings from laboratory astrophysics experiments can inform the design and interpretation of space missions. Understanding plasma physics and magnetic fields in extreme environments helps in designing spacecraft, interpreting observational data, and predicting space weather conditions.

Interdisciplinary Collaboration: Laboratory astrophysics involves collaboration between physicists, astronomers, engineers, and computational scientists. It combines expertise from multiple disciplines, including plasma physics, condensed matter physics, nuclear physics, and computational modeling, to address astrophysical questions.</rdfs:comment>
    </owl:Class>
    


    <!-- http://www.semanticweb.org/afshar87/ontologies/2024/3/Laser-Plasma_ontology#Laser -->

    <owl:Class rdf:about="http://www.semanticweb.org/afshar87/ontologies/2024/3/Laser-Plasma_ontology#Laser"/>
    


    <!-- http://www.semanticweb.org/afshar87/ontologies/2024/3/Laser-Plasma_ontology#Laser-Driven_Shocks -->

    <owl:Class rdf:about="http://www.semanticweb.org/afshar87/ontologies/2024/3/Laser-Plasma_ontology#Laser-Driven_Shocks">
        <rdfs:subClassOf rdf:resource="http://www.semanticweb.org/afshar87/ontologies/2024/3/Laser-Plasma_ontology#LaserPlasma_Relativistic"/>
        <rdfs:comment>Generation of shock waves in a target or plasma due to laser interaction.</rdfs:comment>
    </owl:Class>
    


    <!-- http://www.semanticweb.org/afshar87/ontologies/2024/3/Laser-Plasma_ontology#Laser-Gas_Interaction -->

    <owl:Class rdf:about="http://www.semanticweb.org/afshar87/ontologies/2024/3/Laser-Plasma_ontology#Laser-Gas_Interaction">
        <rdfs:subClassOf rdf:resource="http://www.semanticweb.org/afshar87/ontologies/2024/3/Laser-Plasma_ontology#Laser_Target_Interaction"/>
        <rdfs:comment>Interaction of a laser with a gaseous target.</rdfs:comment>
    </owl:Class>
    


    <!-- http://www.semanticweb.org/afshar87/ontologies/2024/3/Laser-Plasma_ontology#Laser-Liquid_Interaction -->

    <owl:Class rdf:about="http://www.semanticweb.org/afshar87/ontologies/2024/3/Laser-Plasma_ontology#Laser-Liquid_Interaction">
        <rdfs:subClassOf rdf:resource="http://www.semanticweb.org/afshar87/ontologies/2024/3/Laser-Plasma_ontology#Laser_Target_Interaction"/>
        <rdfs:comment>Interaction of a laser with a liquid target.</rdfs:comment>
    </owl:Class>
    


    <!-- http://www.semanticweb.org/afshar87/ontologies/2024/3/Laser-Plasma_ontology#Laser-Solid_Interaction -->

    <owl:Class rdf:about="http://www.semanticweb.org/afshar87/ontologies/2024/3/Laser-Plasma_ontology#Laser-Solid_Interaction">
        <rdfs:subClassOf rdf:resource="http://www.semanticweb.org/afshar87/ontologies/2024/3/Laser-Plasma_ontology#Laser_Target_Interaction"/>
        <rdfs:comment>Interaction of a laser with a solid target.</rdfs:comment>
    </owl:Class>
    


    <!-- http://www.semanticweb.org/afshar87/ontologies/2024/3/Laser-Plasma_ontology#LaserPlasma_Nonrelativistic -->

    <owl:Class rdf:about="http://www.semanticweb.org/afshar87/ontologies/2024/3/Laser-Plasma_ontology#LaserPlasma_Nonrelativistic">
        <rdfs:subClassOf rdf:resource="http://www.semanticweb.org/afshar87/ontologies/2024/3/Laser-Plasma_ontology#Laser_Plasma_Physics"/>
        <rdfs:comment>Laser intensity is low enough that electron velocities remain well below the speed of light.</rdfs:comment>
    </owl:Class>
    


    <!-- http://www.semanticweb.org/afshar87/ontologies/2024/3/Laser-Plasma_ontology#LaserPlasma_Relativistic -->

    <owl:Class rdf:about="http://www.semanticweb.org/afshar87/ontologies/2024/3/Laser-Plasma_ontology#LaserPlasma_Relativistic">
        <rdfs:subClassOf rdf:resource="http://www.semanticweb.org/afshar87/ontologies/2024/3/Laser-Plasma_ontology#Laser_Plasma_Physics"/>
        <rdfs:comment>Laser intensity is high enough that electron velocities approach the speed of light.</rdfs:comment>
    </owl:Class>
    


    <!-- http://www.semanticweb.org/afshar87/ontologies/2024/3/Laser-Plasma_ontology#Laser_Ablation -->

    <owl:Class rdf:about="http://www.semanticweb.org/afshar87/ontologies/2024/3/Laser-Plasma_ontology#Laser_Ablation">
        <rdfs:subClassOf rdf:resource="http://www.semanticweb.org/afshar87/ontologies/2024/3/Laser-Plasma_ontology#LaserPlasma_Nonrelativistic"/>
        <rdfs:comment>Removal of material from a target surface due to laser irradiation.</rdfs:comment>
    </owl:Class>
    


    <!-- http://www.semanticweb.org/afshar87/ontologies/2024/3/Laser-Plasma_ontology#Laser_Channeling -->

    <owl:Class rdf:about="http://www.semanticweb.org/afshar87/ontologies/2024/3/Laser-Plasma_ontology#Laser_Channeling">
        <rdfs:subClassOf rdf:resource="http://www.semanticweb.org/afshar87/ontologies/2024/3/Laser-Plasma_ontology#LaserPlasma_Relativistic"/>
        <rdfs:comment>Confining and guiding an intense laser pulse through a pre-formed plasma channel.</rdfs:comment>
    </owl:Class>
    


    <!-- http://www.semanticweb.org/afshar87/ontologies/2024/3/Laser-Plasma_ontology#Laser_Drilling -->

    <owl:Class rdf:about="http://www.semanticweb.org/afshar87/ontologies/2024/3/Laser-Plasma_ontology#Laser_Drilling">
        <rdfs:subClassOf rdf:resource="http://www.semanticweb.org/afshar87/ontologies/2024/3/Laser-Plasma_ontology#LaserPlasma_Nonrelativistic"/>
        <rdfs:comment>Creating small, deep holes in a target using a focused laser beam.</rdfs:comment>
    </owl:Class>
    


    <!-- http://www.semanticweb.org/afshar87/ontologies/2024/3/Laser-Plasma_ontology#Laser_Electron_Acceleration -->

    <owl:Class rdf:about="http://www.semanticweb.org/afshar87/ontologies/2024/3/Laser-Plasma_ontology#Laser_Electron_Acceleration">
        <rdfs:subClassOf rdf:resource="http://www.semanticweb.org/afshar87/ontologies/2024/3/Laser-Plasma_ontology#Laser_Particle_Acceleration"/>
        <rdfs:comment>Comparison PWFA to LWFA
Energy Source:
PWFA: Uses a particle beam (drive beam) to generate wakefields.
LWFA (Laser Wakefield Acceleration): Uses an intense laser pulse to generate wakefields.
Wakefield Medium:
PWFA: Typically uses a plasma medium.
LWFA: Also uses plasma, but the wake is driven by the ponderomotive force of the laser.
Field Strengths:
Both methods can achieve high gradient fields, but the mechanisms of field generation and the resulting beam characteristics may differ.</rdfs:comment>
    </owl:Class>
    


    <!-- http://www.semanticweb.org/afshar87/ontologies/2024/3/Laser-Plasma_ontology#Laser_Electron_Therapy -->

    <owl:Class rdf:about="http://www.semanticweb.org/afshar87/ontologies/2024/3/Laser-Plasma_ontology#Laser_Electron_Therapy">
        <rdfs:subClassOf rdf:resource="http://www.semanticweb.org/afshar87/ontologies/2024/3/Laser-Plasma_ontology#Laser_Therapy"/>
        <rdfs:comment>Laser Electron Therapy, also known as laser-driven electron therapy, is an advanced technique in cancer treatment that utilizes high-power lasers to accelerate electrons to therapeutic energies, which are then used for radiotherapy. This innovative approach aims to take advantage of the precise control and targeting capabilities of laser systems to deliver effective and localized cancer treatment.

Key Concepts of Laser Electron Therapy:
Traditional Electron Therapy:

Mechanism: In conventional electron therapy, electrons are accelerated using linear accelerators (linacs) and directed at the tumor. The electrons deposit their energy over a relatively short distance, making this therapy effective for treating superficial tumors.
Benefits: Electron therapy is particularly useful for treating cancers located near the surface of the body, such as skin cancers and certain types of head and neck cancers.
Laser-Driven Electron Acceleration:

Mechanism: In laser-driven electron therapy, ultra-intense laser pulses are focused onto a gas or solid target, creating a plasma. The interaction between the laser and the plasma generates strong electric fields that can accelerate electrons to high energies.
Techniques: There are several mechanisms for laser-driven electron acceleration, including Laser Wakefield Acceleration (LWFA), where the laser pulse creates a plasma wave that accelerates the electrons, and Direct Laser Acceleration (DLA).
Advantages:

Compact Systems: Laser-driven accelerators have the potential to be more compact and less expensive than traditional linacs.
Precision: The precise control over laser parameters allows for fine-tuning of the electron beam, which could lead to better targeting of tumors and sparing of healthy tissues.
Short Pulse Duration: Laser-driven electron beams can be generated in extremely short pulses (femtoseconds to picoseconds), potentially reducing radiation damage to healthy tissue.
Challenges:

Beam Quality: Achieving the necessary beam quality, including energy spread, beam divergence, and dose rate, for effective clinical application remains a significant challenge.
Energy Requirements: Producing electron beams with sufficient energy for deep-seated tumors is technically challenging and requires further development.
Infrastructure: Integrating laser-driven systems into clinical settings and ensuring their reliability and safety for patient treatments are ongoing areas of research.</rdfs:comment>
    </owl:Class>
    


    <!-- http://www.semanticweb.org/afshar87/ontologies/2024/3/Laser-Plasma_ontology#Laser_Facility -->

    <owl:Class rdf:about="http://www.semanticweb.org/afshar87/ontologies/2024/3/Laser-Plasma_ontology#Laser_Facility">
        <rdfs:subClassOf rdf:resource="http://www.semanticweb.org/afshar87/ontologies/2024/3/Laser-Plasma_ontology#Facility"/>
    </owl:Class>
    


    <!-- http://www.semanticweb.org/afshar87/ontologies/2024/3/Laser-Plasma_ontology#Laser_HeavyIon_Therapy -->

    <owl:Class rdf:about="http://www.semanticweb.org/afshar87/ontologies/2024/3/Laser-Plasma_ontology#Laser_HeavyIon_Therapy">
        <rdfs:subClassOf rdf:resource="http://www.semanticweb.org/afshar87/ontologies/2024/3/Laser-Plasma_ontology#Laser_Therapy"/>
        <rdfs:comment>therapy using heavier ions (e.g., carbon ions) for potentially improved dose localization compared to protons</rdfs:comment>
    </owl:Class>
    


    <!-- http://www.semanticweb.org/afshar87/ontologies/2024/3/Laser-Plasma_ontology#Laser_Ion_acceleration -->

    <owl:Class rdf:about="http://www.semanticweb.org/afshar87/ontologies/2024/3/Laser-Plasma_ontology#Laser_Ion_acceleration">
        <rdfs:subClassOf rdf:resource="http://www.semanticweb.org/afshar87/ontologies/2024/3/Laser-Plasma_ontology#Laser_Particle_Acceleration"/>
    </owl:Class>
    


    <!-- http://www.semanticweb.org/afshar87/ontologies/2024/3/Laser-Plasma_ontology#Laser_Material_Processing -->

    <owl:Class rdf:about="http://www.semanticweb.org/afshar87/ontologies/2024/3/Laser-Plasma_ontology#Laser_Material_Processing">
        <rdfs:subClassOf rdf:resource="http://www.semanticweb.org/afshar87/ontologies/2024/3/Laser-Plasma_ontology#Laser_Plasma_Application"/>
        <rdfs:comment>Modifying material properties (e.g., surface morphology, micromachining) through laser interaction.</rdfs:comment>
    </owl:Class>
    


    <!-- http://www.semanticweb.org/afshar87/ontologies/2024/3/Laser-Plasma_ontology#Laser_Particle_Acceleration -->

    <owl:Class rdf:about="http://www.semanticweb.org/afshar87/ontologies/2024/3/Laser-Plasma_ontology#Laser_Particle_Acceleration">
        <rdfs:subClassOf rdf:resource="http://www.semanticweb.org/afshar87/ontologies/2024/3/Laser-Plasma_ontology#Laser_Plasma_Application"/>
    </owl:Class>
    


    <!-- http://www.semanticweb.org/afshar87/ontologies/2024/3/Laser-Plasma_ontology#Laser_Photon_Therapy -->

    <owl:Class rdf:about="http://www.semanticweb.org/afshar87/ontologies/2024/3/Laser-Plasma_ontology#Laser_Photon_Therapy">
        <rdfs:subClassOf rdf:resource="http://www.semanticweb.org/afshar87/ontologies/2024/3/Laser-Plasma_ontology#Laser_Therapy"/>
        <rdfs:comment>Laser Photon Therapy, also known as laser-based radiotherapy or laser-driven photon therapy, is an advanced form of cancer treatment that uses high-power lasers to generate photon beams for radiotherapy. This innovative approach aims to take advantage of the precise control and high intensity of laser systems to improve the delivery of radiation therapy.

Key Concepts of Laser Photon Therapy:
Traditional Photon Therapy:

Mechanism: Conventional photon therapy uses X-rays or gamma rays generated by linear accelerators (linacs) to treat cancer. The high-energy photons penetrate the body and deposit energy in the tumor, causing damage to cancer cells.
Benefits: Photon therapy is widely used due to its ability to treat deep-seated tumors with precision and its availability in many clinical settings.
Laser-Driven Photon Generation:

Mechanism: In laser photon therapy, ultra-intense laser pulses are used to accelerate electrons, which then interact with a target material to produce high-energy photons through processes such as bremsstrahlung radiation (braking radiation).
Techniques: One method involves using a laser to create a plasma, which accelerates electrons to high energies. These electrons are then directed to strike a high-Z target material (like tungsten), producing a beam of X-ray photons.
Advantages:

Compact Systems: Laser-driven systems have the potential to be more compact and cost-effective than traditional linacs, making advanced radiotherapy more accessible.
Precision and Control: The high degree of control over laser parameters allows for precise tuning of the photon beam, potentially improving the targeting of tumors and minimizing damage to surrounding healthy tissues.
Short Pulse Duration: Laser-driven photons can be produced in extremely short pulses, which may reduce the duration of treatment sessions and enhance the precision of dose delivery.
Challenges:

Beam Quality and Energy: Achieving the necessary photon energy and beam quality for effective clinical treatment is a significant technical challenge. Ensuring a consistent and reliable beam is crucial for patient safety and treatment efficacy.
Technical Complexity: The integration of high-power laser systems into clinical settings requires overcoming technical and engineering hurdles, such as beam stability, safety protocols, and system maintenance.
Clinical Validation: Extensive research, clinical trials, and regulatory approval are necessary to validate the effectiveness and safety of laser-driven photon therapy.</rdfs:comment>
    </owl:Class>
    


    <!-- http://www.semanticweb.org/afshar87/ontologies/2024/3/Laser-Plasma_ontology#Laser_Plasma_Application -->

    <owl:Class rdf:about="http://www.semanticweb.org/afshar87/ontologies/2024/3/Laser-Plasma_ontology#Laser_Plasma_Application"/>
    


    <!-- http://www.semanticweb.org/afshar87/ontologies/2024/3/Laser-Plasma_ontology#Laser_Plasma_Physics -->

    <owl:Class rdf:about="http://www.semanticweb.org/afshar87/ontologies/2024/3/Laser-Plasma_ontology#Laser_Plasma_Physics"/>
    


    <!-- http://www.semanticweb.org/afshar87/ontologies/2024/3/Laser-Plasma_ontology#Laser_Proton_Therapy -->

    <owl:Class rdf:about="http://www.semanticweb.org/afshar87/ontologies/2024/3/Laser-Plasma_ontology#Laser_Proton_Therapy">
        <rdfs:subClassOf rdf:resource="http://www.semanticweb.org/afshar87/ontologies/2024/3/Laser-Plasma_ontology#Laser_Therapy"/>
        <rdfs:comment>Laser Proton Therapy, also known as Laser-Driven Proton Therapy, is an emerging technique in the field of cancer treatment that leverages high-power lasers to accelerate protons, which are then used for radiotherapy. This method aims to harness the advantages of proton therapy, such as precise targeting of tumors with minimal damage to surrounding healthy tissues, while potentially reducing the size and cost of proton therapy facilities.

Key Concepts of Laser Proton Therapy:
Proton Therapy:

Traditional Proton Therapy: In conventional proton therapy, protons are accelerated using large and expensive cyclotrons or synchrotrons. The protons are directed into the patient&apos;s body, where they deposit most of their energy at a specific depth (the Bragg peak), minimizing damage to healthy tissues beyond the tumor.
Benefits: Proton therapy is particularly effective for treating tumors located near critical structures, pediatric cancers, and radioresistant tumors.
Laser-Driven Proton Acceleration:

Mechanism: In laser-driven proton therapy, ultra-intense laser pulses are focused onto a thin target, creating a plasma. The rapid expansion of the plasma generates electric fields that can accelerate protons to high energies.
Advantages: This method has the potential to reduce the size and cost of proton accelerators, making proton therapy more accessible. Laser systems are typically smaller and less expensive than traditional particle accelerators.
Current Challenges:

Energy and Control: Achieving the necessary proton energies (typically 70-250 MeV for cancer therapy) and controlling the proton beam precisely are major technical challenges. Research is ongoing to improve the efficiency and stability of laser-driven proton acceleration.
Beam Quality: The proton beams generated by laser acceleration need to have appropriate energy spread, divergence, and dose rate for effective clinical use.
Infrastructure and Technology: Developing reliable and practical laser systems and integrating them into clinical settings require significant advancements and validation through clinical trials.</rdfs:comment>
    </owl:Class>
    


    <!-- http://www.semanticweb.org/afshar87/ontologies/2024/3/Laser-Plasma_ontology#Laser_Target_Interaction -->

    <owl:Class rdf:about="http://www.semanticweb.org/afshar87/ontologies/2024/3/Laser-Plasma_ontology#Laser_Target_Interaction">
        <rdfs:subClassOf rdf:resource="http://www.semanticweb.org/afshar87/ontologies/2024/3/Laser-Plasma_ontology#Laser_Plasma_Application"/>
        <rdfs:comment>Warm dense matter (WDM) plays a crucial role in understanding the dynamics of laser-plasma interactions. It represents a specific state of matter that arises when a laser interacts with a target material. Here&apos;s a breakdown of WDM in this context:

Characteristics of WDM:

Partially Ionized: Atoms in WDM lose some electrons due to the intense laser field, but they aren&apos;t fully stripped like in a high-temperature plasma.
High Density: The material remains relatively dense, comparable to its solid state, unlike the low-density plasmas typically created at high laser intensities.
Intermediate Temperature: Electrons in WDM have temperatures ranging from a few electron volts (eV) to tens of eV, higher than a solid but not reaching the extreme temperatures of high-energy-density plasmas.
Unique Properties: The combination of partial ionization and high density leads to unique electrical, thermal, and optical properties not found in solids or high-temperature plasmas.

Creation of WDM in Laser Plasmas:

When a laser pulse interacts with a solid target, the initial interaction can involve various mechanisms like multiphoton ionization and tunnel ionization, leading to the ejection of electrons.
However, the remaining ions are still close together due to the high density of the material.
As the laser energy is absorbed, the remaining electrons and ions in the target get heated, pushing the material towards the WDM state.

Importance of WDM in Laser Plasma Interactions:

Understanding WDM is crucial for accurately modeling the behavior of laser-produced plasmas, particularly in regimes where complete ionization isn&apos;t achieved.
The properties of WDM can significantly affect the propagation and absorption of the laser pulse within the target material.
WDM plays a role in various laser-plasma applications, including:
Laser Ablation: The removal of material from a target surface by laser irradiation. The dynamics of ablation and the properties of the ejected material are influenced by WDM.
Laser-Driven Shocks: The generation of shock waves in a target by a laser pulse can create WDM regions behind the shock front.
X-ray Generation: The emission of X-rays from laser-plasma interactions can be influenced by the electronic structure of WDM.

Challenges of Studying WDM:

Due to its short-lived nature and complex properties, studying WDM in laser-plasma interactions presents challenges.
Advanced diagnostic techniques, such as time-resolved X-ray spectroscopy and ultrafast electron beams, are required to probe the properties of WDM on its short timescales.
Theoretical models also need to be developed to accurately describe the behavior of WDM under these extreme conditions.</rdfs:comment>
    </owl:Class>
    


    <!-- http://www.semanticweb.org/afshar87/ontologies/2024/3/Laser-Plasma_ontology#Laser_Therapy -->

    <owl:Class rdf:about="http://www.semanticweb.org/afshar87/ontologies/2024/3/Laser-Plasma_ontology#Laser_Therapy">
        <rdfs:subClassOf rdf:resource="http://www.semanticweb.org/afshar87/ontologies/2024/3/Laser-Plasma_ontology#Laser_Plasma_Application"/>
    </owl:Class>
    


    <!-- http://www.semanticweb.org/afshar87/ontologies/2024/3/Laser-Plasma_ontology#Liquid_Films_Targets -->

    <owl:Class rdf:about="http://www.semanticweb.org/afshar87/ontologies/2024/3/Laser-Plasma_ontology#Liquid_Films_Targets">
        <rdfs:subClassOf rdf:resource="http://www.semanticweb.org/afshar87/ontologies/2024/3/Laser-Plasma_ontology#liquid_target"/>
        <rdfs:comment>Liquid Films: These consist of a thin layer of liquid formed on a substrate or created by the collision of two liquid jets. They offer similar advantages to liquid jets but with potentially better control over film thickness.</rdfs:comment>
    </owl:Class>
    


    <!-- http://www.semanticweb.org/afshar87/ontologies/2024/3/Laser-Plasma_ontology#Liquid_Jets_Target -->

    <owl:Class rdf:about="http://www.semanticweb.org/afshar87/ontologies/2024/3/Laser-Plasma_ontology#Liquid_Jets_Target">
        <rdfs:subClassOf rdf:resource="http://www.semanticweb.org/afshar87/ontologies/2024/3/Laser-Plasma_ontology#liquid_target"/>
        <rdfs:comment>Liquid Jets: These involve a thin stream of liquid focused by a nozzle. The jet can be intersected by the laser pulse for particle acceleration. Research is focused on:
Jet stability and control: Maintaining a stable and uniform jet is crucial for reproducible results.
Liquid selection: Different liquids (e.g., water, ethanol) offer varying properties for laser-plasma interaction.</rdfs:comment>
    </owl:Class>
    


    <!-- http://www.semanticweb.org/afshar87/ontologies/2024/3/Laser-Plasma_ontology#Mach-Zehnder_Interferometer -->

    <owl:Class rdf:about="http://www.semanticweb.org/afshar87/ontologies/2024/3/Laser-Plasma_ontology#Mach-Zehnder_Interferometer">
        <rdfs:subClassOf rdf:resource="http://www.semanticweb.org/afshar87/ontologies/2024/3/Laser-Plasma_ontology#interferometry"/>
        <rdfs:comment>Mach-Zehnder Interferometry (MZI):

This is a popular choice due to its flexibility and ability to handle large plasma volumes.
In MZI, a laser beam is split into two paths:
Reference Beam: This path travels outside the plasma region and remains undisturbed.
Probe Beam: This path passes through the target plasma.
The recombined beams after traversing their respective paths create an interference pattern.
The variations in the plasma&apos;s refractive index due to its density and temperature affect the probe beam, leading to a shift in the interference pattern compared to the reference beam.
By analyzing this fringe shift, information about the plasma&apos;s electron density profile can be obtained.</rdfs:comment>
    </owl:Class>
    


    <!-- http://www.semanticweb.org/afshar87/ontologies/2024/3/Laser-Plasma_ontology#Macroparticle -->

    <owl:Class rdf:about="http://www.semanticweb.org/afshar87/ontologies/2024/3/Laser-Plasma_ontology#Macroparticle">
        <rdfs:subClassOf rdf:resource="http://www.semanticweb.org/afshar87/ontologies/2024/3/Laser-Plasma_ontology#Simulation"/>
    </owl:Class>
    


    <!-- http://www.semanticweb.org/afshar87/ontologies/2024/3/Laser-Plasma_ontology#Material_Properties_at_High_Pressure -->

    <owl:Class rdf:about="http://www.semanticweb.org/afshar87/ontologies/2024/3/Laser-Plasma_ontology#Material_Properties_at_High_Pressure">
        <rdfs:subClassOf rdf:resource="http://www.semanticweb.org/afshar87/ontologies/2024/3/Laser-Plasma_ontology#High_Energy_Density_Physics_(HEDP)"/>
        <rdfs:comment>Understanding the behavior of materials under extreme pressures relevant to planetary science and astrophysics.</rdfs:comment>
    </owl:Class>
    


    <!-- http://www.semanticweb.org/afshar87/ontologies/2024/3/Laser-Plasma_ontology#Michelson_Interferometer -->

    <owl:Class rdf:about="http://www.semanticweb.org/afshar87/ontologies/2024/3/Laser-Plasma_ontology#Michelson_Interferometer">
        <rdfs:subClassOf rdf:resource="http://www.semanticweb.org/afshar87/ontologies/2024/3/Laser-Plasma_ontology#interferometry"/>
        <rdfs:comment>A classic setup used for measuring lengths and studying optical properties. It splits a light beam, sends it along two paths, and then recombines the beams to observe the resulting interference pattern. 

This classic interferometer setup can also be used for plasma diagnostics, although it&apos;s less common than MZI for large plasmas.
Similar to MZI, a laser beam is split into a reference and probe beam.
The probe beam traverses the plasma, while the reference beam might travel a different path length outside the plasma.
The recombined beams create an interference pattern, and the fringe shift caused by the plasma&apos;s refractive index allows for electron density profile reconstruction.</rdfs:comment>
    </owl:Class>
    


    <!-- http://www.semanticweb.org/afshar87/ontologies/2024/3/Laser-Plasma_ontology#Multi-Layer_Targets -->

    <owl:Class rdf:about="http://www.semanticweb.org/afshar87/ontologies/2024/3/Laser-Plasma_ontology#Multi-Layer_Targets">
        <rdfs:subClassOf rdf:resource="http://www.semanticweb.org/afshar87/ontologies/2024/3/Laser-Plasma_ontology#solid__target"/>
        <rdfs:comment>These targets consist of a thin layer of high-Z material (heavy element) on a low-Z material base. The interaction with the laser pulse can lead to efficient proton acceleration from the low-Z layer. Ongoing research aims to optimize the target design and laser parameters for this approach.</rdfs:comment>
    </owl:Class>
    


    <!-- http://www.semanticweb.org/afshar87/ontologies/2024/3/Laser-Plasma_ontology#Multiphoton_Ionization -->

    <owl:Class rdf:about="http://www.semanticweb.org/afshar87/ontologies/2024/3/Laser-Plasma_ontology#Multiphoton_Ionization">
        <rdfs:subClassOf rdf:resource="http://www.semanticweb.org/afshar87/ontologies/2024/3/Laser-Plasma_ontology#Ionization"/>
        <rdfs:comment>Absorption of multiple photons by an atom or molecule to overcome its ionization potential.</rdfs:comment>
    </owl:Class>
    


    <!-- http://www.semanticweb.org/afshar87/ontologies/2024/3/Laser-Plasma_ontology#Nanoparticle_Targets -->

    <owl:Class rdf:about="http://www.semanticweb.org/afshar87/ontologies/2024/3/Laser-Plasma_ontology#Nanoparticle_Targets">
        <rdfs:subClassOf rdf:resource="http://www.semanticweb.org/afshar87/ontologies/2024/3/Laser-Plasma_ontology#solid__target"/>
        <rdfs:comment>These targets consist of microscopic particles clustered together. They offer promise for improved control over ion energy distribution due to their unique properties.  Research is focused on optimizing nanoparticle size, composition, and laser interaction for efficient particle generation:

Nanoparticle size: Smaller size can lead to narrower ion energy spread.
Nanoparticle composition: Different materials offer varying acceleration characteristics.</rdfs:comment>
    </owl:Class>
    


    <!-- http://www.semanticweb.org/afshar87/ontologies/2024/3/Laser-Plasma_ontology#Non-Equilibrium_Dynamics -->

    <owl:Class rdf:about="http://www.semanticweb.org/afshar87/ontologies/2024/3/Laser-Plasma_ontology#Non-Equilibrium_Dynamics">
        <rdfs:subClassOf rdf:resource="http://www.semanticweb.org/afshar87/ontologies/2024/3/Laser-Plasma_ontology#High_Energy_Density_Physics_(HEDP)"/>
        <rdfs:comment>Studying the rapid changes and instabilities that occur in HED matter due to high energy deposition.</rdfs:comment>
    </owl:Class>
    


    <!-- http://www.semanticweb.org/afshar87/ontologies/2024/3/Laser-Plasma_ontology#Opacity_Studies -->

    <owl:Class rdf:about="http://www.semanticweb.org/afshar87/ontologies/2024/3/Laser-Plasma_ontology#Opacity_Studies">
        <rdfs:subClassOf rdf:resource="http://www.semanticweb.org/afshar87/ontologies/2024/3/Laser-Plasma_ontology#High_Energy_Density_Physics_(HEDP)"/>
        <rdfs:comment>nvestigations of how HED matter absorbs and scatters radiation.</rdfs:comment>
    </owl:Class>
    


    <!-- http://www.semanticweb.org/afshar87/ontologies/2024/3/Laser-Plasma_ontology#Optical_Diagnostics -->

    <owl:Class rdf:about="http://www.semanticweb.org/afshar87/ontologies/2024/3/Laser-Plasma_ontology#Optical_Diagnostics">
        <rdfs:subClassOf rdf:resource="http://www.semanticweb.org/afshar87/ontologies/2024/3/Laser-Plasma_ontology#Diagnostics"/>
        <rdfs:comment>Techniques using various optical methods to study laser-matter interactions (e.g., interferometry, schlieren imaging).</rdfs:comment>
    </owl:Class>
    


    <!-- http://www.semanticweb.org/afshar87/ontologies/2024/3/Laser-Plasma_ontology#Output -->

    <owl:Class rdf:about="http://www.semanticweb.org/afshar87/ontologies/2024/3/Laser-Plasma_ontology#Output">
        <rdfs:subClassOf rdf:resource="http://www.semanticweb.org/afshar87/ontologies/2024/3/Laser-Plasma_ontology#Simulation"/>
    </owl:Class>
    


    <!-- http://www.semanticweb.org/afshar87/ontologies/2024/3/Laser-Plasma_ontology#Owner -->

    <owl:Class rdf:about="http://www.semanticweb.org/afshar87/ontologies/2024/3/Laser-Plasma_ontology#Owner"/>
    


    <!-- http://www.semanticweb.org/afshar87/ontologies/2024/3/Laser-Plasma_ontology#Partially_Ionized_Materials -->

    <owl:Class rdf:about="http://www.semanticweb.org/afshar87/ontologies/2024/3/Laser-Plasma_ontology#Partially_Ionized_Materials">
        <rdfs:subClassOf rdf:resource="http://www.semanticweb.org/afshar87/ontologies/2024/3/Laser-Plasma_ontology#Warm_Dense_Matter_(WDM)"/>
        <rdfs:comment>Materials where some atoms have lost electrons but still retain some atomic structure. This is a key characteristic of WDM.</rdfs:comment>
    </owl:Class>
    


    <!-- http://www.semanticweb.org/afshar87/ontologies/2024/3/Laser-Plasma_ontology#Particle_Beam_Generation -->

    <owl:Class rdf:about="http://www.semanticweb.org/afshar87/ontologies/2024/3/Laser-Plasma_ontology#Particle_Beam_Generation">
        <rdfs:subClassOf rdf:resource="http://www.semanticweb.org/afshar87/ontologies/2024/3/Laser-Plasma_ontology#Laser_Plasma_Application"/>
    </owl:Class>
    


    <!-- http://www.semanticweb.org/afshar87/ontologies/2024/3/Laser-Plasma_ontology#Particle_spectroscopy -->

    <owl:Class rdf:about="http://www.semanticweb.org/afshar87/ontologies/2024/3/Laser-Plasma_ontology#Particle_spectroscopy">
        <rdfs:subClassOf rdf:resource="http://www.semanticweb.org/afshar87/ontologies/2024/3/Laser-Plasma_ontology#Diagnostics"/>
        <rdfs:comment>Measuring the energy and number of particles emitted from a laser-matter interaction.</rdfs:comment>
    </owl:Class>
    


    <!-- http://www.semanticweb.org/afshar87/ontologies/2024/3/Laser-Plasma_ontology#Plasma -->

    <owl:Class rdf:about="http://www.semanticweb.org/afshar87/ontologies/2024/3/Laser-Plasma_ontology#Plasma"/>
    


    <!-- http://www.semanticweb.org/afshar87/ontologies/2024/3/Laser-Plasma_ontology#Plasma_Heating -->

    <owl:Class rdf:about="http://www.semanticweb.org/afshar87/ontologies/2024/3/Laser-Plasma_ontology#Plasma_Heating">
        <rdfs:subClassOf rdf:resource="http://www.semanticweb.org/afshar87/ontologies/2024/3/Laser-Plasma_ontology#LaserPlasma_Nonrelativistic"/>
        <rdfs:comment>Transfer of laser energy to the target material, increasing its temperature and creating a plasma.</rdfs:comment>
    </owl:Class>
    


    <!-- http://www.semanticweb.org/afshar87/ontologies/2024/3/Laser-Plasma_ontology#Project -->

    <owl:Class rdf:about="http://www.semanticweb.org/afshar87/ontologies/2024/3/Laser-Plasma_ontology#Project">
        <rdfs:comment>A project addresses a specific laser plasma study either simulation or experiment.</rdfs:comment>
    </owl:Class>
    


    <!-- http://www.semanticweb.org/afshar87/ontologies/2024/3/Laser-Plasma_ontology#Radiation_Hydrodynamics -->

    <owl:Class rdf:about="http://www.semanticweb.org/afshar87/ontologies/2024/3/Laser-Plasma_ontology#Radiation_Hydrodynamics">
        <rdfs:subClassOf rdf:resource="http://www.semanticweb.org/afshar87/ontologies/2024/3/Laser-Plasma_ontology#High_Energy_Density_Physics_(HEDP)"/>
    </owl:Class>
    


    <!-- http://www.semanticweb.org/afshar87/ontologies/2024/3/Laser-Plasma_ontology#Shadowgraphy -->

    <owl:Class rdf:about="http://www.semanticweb.org/afshar87/ontologies/2024/3/Laser-Plasma_ontology#Shadowgraphy">
        <rdfs:subClassOf rdf:resource="http://www.semanticweb.org/afshar87/ontologies/2024/3/Laser-Plasma_ontology#Optical_Diagnostics"/>
        <rdfs:comment>shadowgraphy is an optical technique used to visualize non-uniformities or variations in transparent media like air, water, or glass. Here&apos;s a breakdown of this scientific application:

Principle: Shadowgraphy relies on the principle that light rays travel in straight lines unless they encounter a medium with a varying refractive index.
Refractive Index: The refractive index is a material property that determines how much light bends as it passes through the material. In a uniform medium, light propagates in a straight line.
Non-Uniformities: When there are variations in density, temperature, or composition within a transparent medium, its refractive index becomes non-uniform. These non-uniformities cause light rays to bend slightly as they traverse the medium.
Shadow Formation: When a light source illuminates the non-uniform medium, the bent light rays no longer follow a straight path and create a shadow on a screen placed behind the medium. This shadow represents the projected image of the non-uniformities within the medium.

In laser plasma research, shadowgraphy refers to  ** the optical technique for observing non-uniformities **. It&apos;s a valuable tool for visualizing the density profiles and structures within the laser-generated plasma.

Here&apos;s how shadowgraphy works in laser-plasma context:

* Principle: As a high-intensity laser pulse interacts with a target material, it ionizes atoms, creating a hot, ionized gas known as plasma. The density and temperature within the plasma can vary significantly.
* Light Source: A separate, relatively weak light source (often a laser) illuminates the plasma.
* Non-Uniformities: Due to variations in plasma density and temperature, the refractive index becomes non-uniform. Denser regions have a slightly higher refractive index, causing the light rays to bend as they pass through the plasma.
* Shadow Formation: The bent light rays no longer travel in straight lines and cast a shadow on a screen or detector placed behind the plasma. This shadow represents the projected image of the plasma&apos;s density variations.

Information Obtained:

By analyzing the shadowgram (the recorded shadow image), researchers can gain insights into the plasma&apos;s:

* Overall Shape and Size: The basic outline of the plasma is visible in the shadowgram.
* Density Variations: Denser regions within the plasma appear darker or more pronounced in the shadow, while less dense regions cast a lighter shadow.
* Shockwave Formation: In some cases, the interaction can generate shockwaves within the plasma, which can be visualized as distinct features in the shadowgram.

Advantages:

- Simple and Cost-Effective: Shadowgraphy is a relatively simple and inexpensive technique compared to more sophisticated diagnostic methods.
- Real-Time Visualization: It offers real-time visualization of dynamic phenomena occurring within the transparent medium.

Limitations:

- Quantitative Information: Shadowgraphy primarily provides qualitative information about the presence and location of non-uniformities. It might not provide precise quantitative data on the magnitude of the variations.
- Sensitivity: The sensitivity of shadowgraphy depends on the degree of non-uniformity in the medium. Subtle variations might be difficult to visualize.

Applications of Shadowgraphy:

- Fluid Dynamics: Visualizing airflows around objects, shockwaves, and turbulence patterns in wind tunnels or water channels.
- Combustion Research: Observing flame propagation, temperature variations, and density fluctuations within a burning mixture.
- Material Testing: Detecting flaws, cracks, or internal stress distributions in transparent materials like glass or plastic.
- Plasma Diagnostics: Visualizing the density profiles and structures of hot, ionized gases (plasmas) used in fusion research.</rdfs:comment>
    </owl:Class>
    


    <!-- http://www.semanticweb.org/afshar87/ontologies/2024/3/Laser-Plasma_ontology#Shock_ignition -->

    <owl:Class rdf:about="http://www.semanticweb.org/afshar87/ontologies/2024/3/Laser-Plasma_ontology#Shock_ignition">
        <rdfs:subClassOf rdf:resource="http://www.semanticweb.org/afshar87/ontologies/2024/3/Laser-Plasma_ontology#DirectDriveFusion"/>
    </owl:Class>
    


    <!-- http://www.semanticweb.org/afshar87/ontologies/2024/3/Laser-Plasma_ontology#Simulation -->

    <owl:Class rdf:about="http://www.semanticweb.org/afshar87/ontologies/2024/3/Laser-Plasma_ontology#Simulation"/>
    


    <!-- http://www.semanticweb.org/afshar87/ontologies/2024/3/Laser-Plasma_ontology#Single-Layer_Targets -->

    <owl:Class rdf:about="http://www.semanticweb.org/afshar87/ontologies/2024/3/Laser-Plasma_ontology#Single-Layer_Targets">
        <rdfs:subClassOf rdf:resource="http://www.semanticweb.org/afshar87/ontologies/2024/3/Laser-Plasma_ontology#solid__target"/>
        <rdfs:comment>Solid Targets: These are the most traditional and widely used targets. They come in various materials, with common choices including:

Plastics (e.g., CH targets): Simple and readily available, but offer limited control over ion energy distribution.
Metals (e.g., Cu, Al): Can generate high-energy ions, but often lead to broader energy distributions.
Dielectric materials (e.g., LiF): Offer potential advantages in terms of tailoring ion energy spectra.
Nanoparticle Targets: These targets consist of microscopic particles clustered together.

 They offer promise for improved control over ion energy distribution due to their unique properties. Research is ongoing to optimize:
Nanoparticle size: Smaller size can lead to narrower ion energy spread.
Nanoparticle composition: Different materials offer varying acceleration characteristics.</rdfs:comment>
    </owl:Class>
    


    <!-- http://www.semanticweb.org/afshar87/ontologies/2024/3/Laser-Plasma_ontology#Species -->

    <owl:Class rdf:about="http://www.semanticweb.org/afshar87/ontologies/2024/3/Laser-Plasma_ontology#Species"/>
    


    <!-- http://www.semanticweb.org/afshar87/ontologies/2024/3/Laser-Plasma_ontology#Strongly_Coupled_Plasmas -->

    <owl:Class rdf:about="http://www.semanticweb.org/afshar87/ontologies/2024/3/Laser-Plasma_ontology#Strongly_Coupled_Plasmas">
        <rdfs:subClassOf rdf:resource="http://www.semanticweb.org/afshar87/ontologies/2024/3/Laser-Plasma_ontology#Warm_Dense_Matter_(WDM)"/>
        <rdfs:comment>Plasmas where the average distance between particles is comparable to their de Broglie wavelength, leading to strong correlations between particles.</rdfs:comment>
    </owl:Class>
    


    <!-- http://www.semanticweb.org/afshar87/ontologies/2024/3/Laser-Plasma_ontology#Supercomputer_Facility -->

    <owl:Class rdf:about="http://www.semanticweb.org/afshar87/ontologies/2024/3/Laser-Plasma_ontology#Supercomputer_Facility">
        <rdfs:subClassOf rdf:resource="http://www.semanticweb.org/afshar87/ontologies/2024/3/Laser-Plasma_ontology#Facility"/>
    </owl:Class>
    


    <!-- http://www.semanticweb.org/afshar87/ontologies/2024/3/Laser-Plasma_ontology#Target -->

    <owl:Class rdf:about="http://www.semanticweb.org/afshar87/ontologies/2024/3/Laser-Plasma_ontology#Target"/>
    


    <!-- http://www.semanticweb.org/afshar87/ontologies/2024/3/Laser-Plasma_ontology#Target_Structure -->

    <owl:Class rdf:about="http://www.semanticweb.org/afshar87/ontologies/2024/3/Laser-Plasma_ontology#Target_Structure">
        <rdfs:subClassOf rdf:resource="http://www.semanticweb.org/afshar87/ontologies/2024/3/Laser-Plasma_ontology#Target"/>
        <rdfs:comment>This subclass defines the structure of targets that are used in laser-plasma experiments.</rdfs:comment>
    </owl:Class>
    


    <!-- http://www.semanticweb.org/afshar87/ontologies/2024/3/Laser-Plasma_ontology#Thomson_scattering -->

    <owl:Class rdf:about="http://www.semanticweb.org/afshar87/ontologies/2024/3/Laser-Plasma_ontology#Thomson_scattering">
        <rdfs:subClassOf rdf:resource="http://www.semanticweb.org/afshar87/ontologies/2024/3/Laser-Plasma_ontology#Diagnostics"/>
        <rdfs:comment>Thomson Scattering:  Scattering of laser light by free electrons in a plasma, providing information on electron properties such as electron density.</rdfs:comment>
    </owl:Class>
    


    <!-- http://www.semanticweb.org/afshar87/ontologies/2024/3/Laser-Plasma_ontology#Time-Resolved_Interferometry -->

    <owl:Class rdf:about="http://www.semanticweb.org/afshar87/ontologies/2024/3/Laser-Plasma_ontology#Time-Resolved_Interferometry">
        <rdfs:subClassOf rdf:resource="http://www.semanticweb.org/afshar87/ontologies/2024/3/Laser-Plasma_ontology#interferometry"/>
        <rdfs:comment>This approach incorporates techniques like MZI or Michelson interferometry with pulsed lasers for time-dependent measurements.
By rapidly recording interferograms (interference patterns) at different time points after the laser pulse interacts with the plasma, researchers can track the evolution of the plasma density profile over time.
This provides valuable insights into the dynamics of laser-plasma interactions, such as the expansion and heating of the plasma.</rdfs:comment>
    </owl:Class>
    


    <!-- http://www.semanticweb.org/afshar87/ontologies/2024/3/Laser-Plasma_ontology#Tunnel_Ionization -->

    <owl:Class rdf:about="http://www.semanticweb.org/afshar87/ontologies/2024/3/Laser-Plasma_ontology#Tunnel_Ionization">
        <rdfs:subClassOf rdf:resource="http://www.semanticweb.org/afshar87/ontologies/2024/3/Laser-Plasma_ontology#Ionization"/>
        <rdfs:comment>Electrons tunnel through the potential barrier of an atom or molecule due to the strong laser field.</rdfs:comment>
    </owl:Class>
    


    <!-- http://www.semanticweb.org/afshar87/ontologies/2024/3/Laser-Plasma_ontology#Warm_Dense_Metals -->

    <owl:Class rdf:about="http://www.semanticweb.org/afshar87/ontologies/2024/3/Laser-Plasma_ontology#Warm_Dense_Metals">
        <rdfs:subClassOf rdf:resource="http://www.semanticweb.org/afshar87/ontologies/2024/3/Laser-Plasma_ontology#Warm_Dense_Matter_(WDM)"/>
        <rdfs:comment>Metals in the WDM state, exhibiting unique electronic and transport properties compared to their solid or fully ionized states.</rdfs:comment>
    </owl:Class>
    


    <!-- http://www.semanticweb.org/afshar87/ontologies/2024/3/Laser-Plasma_ontology#Warm_Dense_Semiconductors -->

    <owl:Class rdf:about="http://www.semanticweb.org/afshar87/ontologies/2024/3/Laser-Plasma_ontology#Warm_Dense_Semiconductors">
        <rdfs:subClassOf rdf:resource="http://www.semanticweb.org/afshar87/ontologies/2024/3/Laser-Plasma_ontology#Warm_Dense_Matter_(WDM)"/>
        <rdfs:comment>Semiconductors in the WDM state, with potential applications in high-power electronics.</rdfs:comment>
    </owl:Class>
    


    <!-- http://www.semanticweb.org/afshar87/ontologies/2024/3/Laser-Plasma_ontology#X-Ray_Emission -->

    <owl:Class rdf:about="http://www.semanticweb.org/afshar87/ontologies/2024/3/Laser-Plasma_ontology#X-Ray_Emission">
        <rdfs:subClassOf rdf:resource="http://www.semanticweb.org/afshar87/ontologies/2024/3/Laser-Plasma_ontology#Laser_Plasma_Application"/>
        <rdfs:comment>the emission of X-rays due to laser-plasma interactions such as bremsstrahlung, recombination, and other processes.</rdfs:comment>
    </owl:Class>
    


    <!-- http://www.semanticweb.org/afshar87/ontologies/2024/3/Laser-Plasma_ontology#X-ray_radiography -->

    <owl:Class rdf:about="http://www.semanticweb.org/afshar87/ontologies/2024/3/Laser-Plasma_ontology#X-ray_radiography">
        <rdfs:subClassOf rdf:resource="http://www.semanticweb.org/afshar87/ontologies/2024/3/Laser-Plasma_ontology#Diagnostics"/>
        <rdfs:comment>X-ray radiography uses X-rays to create images based on density differences, revealing the internal structure of an object.

Purpose:  Imaging the interior of a target or plasma using X-rays.

Process: X-rays are passed through the object. Denser regions absorb more X-rays, while less dense regions allow more X-rays to pass through. A detector on the other side of the object records the transmitted X-rays, creating an image where denser areas appear darker and less dense areas appear lighter.

Information Obtained: Provides information about the overall density distribution within the object, allowing for visualization of internal features, cracks, or hidden objects.

Applications: Widely used in medical imaging (X-rays of bones and organs), security screening (detecting contraband in luggage), and non-destructive testing (inspecting welds or internal structures in materials).</rdfs:comment>
    </owl:Class>
    


    <!-- http://www.semanticweb.org/afshar87/ontologies/2024/3/Laser-Plasma_ontology#X-ray_spectroscopy -->

    <owl:Class rdf:about="http://www.semanticweb.org/afshar87/ontologies/2024/3/Laser-Plasma_ontology#X-ray_spectroscopy">
        <rdfs:subClassOf rdf:resource="http://www.semanticweb.org/afshar87/ontologies/2024/3/Laser-Plasma_ontology#Diagnostics"/>
        <rdfs:comment>X-ray spectroscopy uses X-rays to analyze the elemental composition of a material by studying its interaction with X-rays.

Purpose: Analyzes the elemental composition of a material by studying the X-rays it emits or absorbs.

Process: The material is bombarded with X-rays or other high-energy radiation (electrons, protons). This can cause the material to emit its own characteristic X-rays or absorb X-rays of specific energies. The emitted or absorbed X-rays are then measured by a spectrometer.

Information Obtained: Provides information about the types and quantities of elements present in the material by analyzing the energy distribution of the emitted or absorbed X-rays.

Applications: Used in material science for elemental analysis, forensics for identifying materials in evidence, and astrophysics for studying the composition of stars and other celestial objects.</rdfs:comment>
    </owl:Class>
    


    <!-- http://www.semanticweb.org/afshar87/ontologies/2024/3/Laser-Plasma_ontology#accelerator_facility -->

    <owl:Class rdf:about="http://www.semanticweb.org/afshar87/ontologies/2024/3/Laser-Plasma_ontology#accelerator_facility">
        <rdfs:subClassOf rdf:resource="http://www.semanticweb.org/afshar87/ontologies/2024/3/Laser-Plasma_ontology#Facility"/>
    </owl:Class>
    


    <!-- http://www.semanticweb.org/afshar87/ontologies/2024/3/Laser-Plasma_ontology#electron -->

    <owl:Class rdf:about="http://www.semanticweb.org/afshar87/ontologies/2024/3/Laser-Plasma_ontology#electron">
        <rdfs:subClassOf rdf:resource="http://www.semanticweb.org/afshar87/ontologies/2024/3/Laser-Plasma_ontology#Species"/>
    </owl:Class>
    


    <!-- http://www.semanticweb.org/afshar87/ontologies/2024/3/Laser-Plasma_ontology#gas__target -->

    <owl:Class rdf:about="http://www.semanticweb.org/afshar87/ontologies/2024/3/Laser-Plasma_ontology#gas__target">
        <rdfs:subClassOf rdf:resource="http://www.semanticweb.org/afshar87/ontologies/2024/3/Laser-Plasma_ontology#Target_Structure"/>
        <rdfs:comment>Gas Targets: These are thin layers of gas, often hydrogen or helium, used to create a plasma for wakefield generation. The properties of the plasma (density, temperature) are crucial for efficient electron acceleration. Research is focused on:
Gas selection and density optimization: Different gases offer varying plasma characteristics for LWFA/PWFA.
Gas jet targets: Precise control over gas flow and density profile is important for stable wakefield generation.</rdfs:comment>
    </owl:Class>
    


    <!-- http://www.semanticweb.org/afshar87/ontologies/2024/3/Laser-Plasma_ontology#interferometry -->

    <owl:Class rdf:about="http://www.semanticweb.org/afshar87/ontologies/2024/3/Laser-Plasma_ontology#interferometry">
        <rdfs:subClassOf rdf:resource="http://www.semanticweb.org/afshar87/ontologies/2024/3/Laser-Plasma_ontology#Optical_Diagnostics"/>
        <rdfs:comment>Interferometry is a powerful technique that utilizes the phenomenon of wave superposition to extract information. It primarily works with electromagnetic waves (like light), but can also be applied to sound waves and even atomic particles. Here&apos;s a breakdown of the key concepts:

Wave Superposition:

When two or more waves encounter each other, their properties (amplitude and phase) can combine to create a new wave pattern. This is called superposition.
The resulting pattern depends on the characteristics of the original waves, including their amplitudes, frequencies, and phases.
Interference:

In interferometry, we deliberately combine waves to create an interference pattern. This pattern can be constructive (waves reinforce each other, leading to high intensity) or destructive (waves cancel each other out, leading to low intensity).
By analyzing the interference pattern, we can extract information about the original waves, such as their:
Relative phases
Wavelengths
Presence of minute variations
Applications of Interferometry:

The specific type of interferometry used in a laser plasma experiment depends on several factors, including:

Desired Information: Whether the focus is on electron density profiles, time-dependent behavior, or additional plasma parameters.
Plasma Size and Geometry: Mach-Zehnder Interferometry is better suited for larger plasmas, while Michelson might be used for smaller, well-defined plasma regions.
Temporal Resolution Requirements: Time-resolved interferometry is necessary for capturing rapid changes in the plasma density.

Interferometry has a wide range of applications across various scientific and technological fields. Here are some prominent examples:

Astronomy: Measuring the positions and movements of stars and galaxies with incredible precision. Techniques like optical interferometry combine light from multiple telescopes to act as a giant virtual telescope, achieving much higher resolution than any single telescope.
Material Science: Studying the properties of materials at the atomic level. Interferometry can reveal details about surface topography, thin film thickness, and material composition.
Optometry: Measuring the refractive index of the eye to determine corrective lenses for vision problems.
Plasma Physics: Diagnosing the properties of hot, ionized gases (plasmas) used in fusion research.
Metrology: Precisely measuring distances, lengths, and other physical parameters with unmatched accuracy.</rdfs:comment>
    </owl:Class>
    


    <!-- http://www.semanticweb.org/afshar87/ontologies/2024/3/Laser-Plasma_ontology#ion -->

    <owl:Class rdf:about="http://www.semanticweb.org/afshar87/ontologies/2024/3/Laser-Plasma_ontology#ion">
        <rdfs:subClassOf rdf:resource="http://www.semanticweb.org/afshar87/ontologies/2024/3/Laser-Plasma_ontology#Species"/>
    </owl:Class>
    


    <!-- http://www.semanticweb.org/afshar87/ontologies/2024/3/Laser-Plasma_ontology#laser_propagation_direction -->

    <owl:Class rdf:about="http://www.semanticweb.org/afshar87/ontologies/2024/3/Laser-Plasma_ontology#laser_propagation_direction">
        <rdfs:subClassOf rdf:resource="http://www.semanticweb.org/afshar87/ontologies/2024/3/Laser-Plasma_ontology#Laser"/>
    </owl:Class>
    


    <!-- http://www.semanticweb.org/afshar87/ontologies/2024/3/Laser-Plasma_ontology#liquid_target -->

    <owl:Class rdf:about="http://www.semanticweb.org/afshar87/ontologies/2024/3/Laser-Plasma_ontology#liquid_target">
        <rdfs:subClassOf rdf:resource="http://www.semanticweb.org/afshar87/ontologies/2024/3/Laser-Plasma_ontology#Target_Structure"/>
        <rdfs:comment>Liquid targets are indeed an emerging area of research in laser-plasma interaction for particle acceleration. Here&apos;s a breakdown of their potential and considerations:

Advantages of Liquid Targets:

Replenishment: Unlike solid targets that get damaged after each laser shot, liquid targets offer the advantage of being continuously replenished. This allows for high repetition rate experiments, crucial for some applications.
Uniformity: Liquids can provide a more uniform and clean target compared to solid targets, which can have imperfections or surface irregularities. This uniformity can lead to more consistent laser-plasma interaction and potentially improve beam quality.
Tailorable Properties: The properties of the liquid target can be tailored by using different liquids or mixtures. This allows researchers to potentially optimize the target for specific acceleration mechanisms (e.g., TNSA, RPA) or particle species (protons, ions).
Types of Liquid Targets:

Liquid Jets: These involve a thin stream of liquid focused by a nozzle. The jet can be intersected by the laser pulse for particle acceleration. Research is focused on:
Jet stability and control: Maintaining a stable and uniform jet is crucial for reproducible results.
Liquid selection: Different liquids (e.g., water, ethanol) offer varying properties for laser-plasma interaction.
Liquid Films: These consist of a thin layer of liquid formed on a substrate or created by the collision of two liquid jets. They offer similar advantages to liquid jets but with potentially better control over film thickness.
Challenges of Liquid Targets:

Target Delivery System: Designing a reliable system for delivering and replenishing the liquid target within the vacuum chamber of a laser system can be complex.
Hydrodynamic Effects: The liquid&apos;s motion due to the laser pulse or jet flow could introduce instabilities that affect the laser-plasma interaction. Research is ongoing to minimize these effects.
Target Contamination: Maintaining a clean and contaminant-free liquid is important for consistent results.
Overall:

Liquid targets hold promise for advancing laser-driven particle acceleration, particularly for high repetition rate applications. While challenges exist, ongoing research is addressing these issues to improve the reliability and effectiveness of liquid targets in this field.

Incorporating liquid targets as a subclass within your LaserPlasmaOntology can enhance its comprehensiveness and reflect the latest developments in particle acceleration techniques. Remember to link them appropriately to the relevant particle acceleration processes (e.g., TNSATherapy with LiquidJetTarget).</rdfs:comment>
    </owl:Class>
    


    <!-- http://www.semanticweb.org/afshar87/ontologies/2024/3/Laser-Plasma_ontology#neutron -->

    <owl:Class rdf:about="http://www.semanticweb.org/afshar87/ontologies/2024/3/Laser-Plasma_ontology#neutron">
        <rdfs:subClassOf rdf:resource="http://www.semanticweb.org/afshar87/ontologies/2024/3/Laser-Plasma_ontology#Species"/>
    </owl:Class>
    


    <!-- http://www.semanticweb.org/afshar87/ontologies/2024/3/Laser-Plasma_ontology#proton -->

    <owl:Class rdf:about="http://www.semanticweb.org/afshar87/ontologies/2024/3/Laser-Plasma_ontology#proton">
        <rdfs:subClassOf rdf:resource="http://www.semanticweb.org/afshar87/ontologies/2024/3/Laser-Plasma_ontology#Species"/>
    </owl:Class>
    


    <!-- http://www.semanticweb.org/afshar87/ontologies/2024/3/Laser-Plasma_ontology#recombination -->

    <owl:Class rdf:about="http://www.semanticweb.org/afshar87/ontologies/2024/3/Laser-Plasma_ontology#recombination">
        <rdfs:subClassOf rdf:resource="http://www.semanticweb.org/afshar87/ontologies/2024/3/Laser-Plasma_ontology#Laser_Plasma_Physics"/>
    </owl:Class>
    


    <!-- http://www.semanticweb.org/afshar87/ontologies/2024/3/Laser-Plasma_ontology#solid__target -->

    <owl:Class rdf:about="http://www.semanticweb.org/afshar87/ontologies/2024/3/Laser-Plasma_ontology#solid__target">
        <rdfs:subClassOf rdf:resource="http://www.semanticweb.org/afshar87/ontologies/2024/3/Laser-Plasma_ontology#Target_Structure"/>
        <rdfs:comment>These are the most traditional and widely used targets. They come in various materials, with common choices including:
Plastics (e.g., CH targets): Simple and readily available, but offer limited control over ion energy distribution.
Metals (e.g., Cu, Al): Can generate high-energy ions, but often lead to broader energy distributions.
Dielectric materials (e.g., LiF): Offer potential advantages in terms of tailoring ion energy spectra.</rdfs:comment>
    </owl:Class>
    


    <!-- http://www.semanticweb.org/afshar87/ontologies/2024/3/Laser-Plasma_ontology#Breakout_Afterburner_(BOA) -->

    <owl:Class rdf:about="http://www.semanticweb.org/afshar87/ontologies/2024/3/Laser-Plasma_ontology#Breakout_Afterburner_(BOA)">
        <rdfs:subClassOf rdf:resource="http://www.semanticweb.org/afshar87/ontologies/2024/3/Laser-Plasma_ontology#Laser_Ion_acceleration"/>
        <rdfs:comment>BOA Principle:

Solid-Density Target: The BOA technique starts with a target material in a solid-density state.
Relativistically Induced Transparency: When a high-intensity laser pulse interacts with the solid target, a phenomenon called &quot;relativistically induced transparency&quot; occurs.
In simpler terms, the intense laser pulse alters the properties of the target material, making it more transparent to the laser light at a specific time during the interaction.
Enhanced Ion Acceleration: This induced transparency allows the laser pulse to penetrate deeper into the target. This deeper interaction creates a stronger electric field region behind the initially irradiated surface.
This stronger electric field then leads to a period of enhanced ion acceleration for ions within the target material.
Advantages of BOA:

Higher Energy Gains: Compared to other laser-ion acceleration mechanisms like TNSA, BOA can theoretically achieve higher energy gains for ions. This is due to the extended interaction time with the stronger electric field.
Monoenergetic Beams: BOA has the potential to produce more monoenergetic ion beams, meaning the ions have a narrower range of velocities compared to broader distributions seen in other techniques. This can be beneficial for certain applications.
Challenges and Considerations:

Experimental Complexity: Implementing and controlling the BOA process requires precise control over laser pulse parameters and target properties. Achieving the optimal conditions for BOA can be experimentally challenging.
Target Modifications: The relativistically induced transparency can lead to modifications in the target material itself, which can affect the overall efficiency and reproducibility of the acceleration process.
Applications:

BOA research holds promise for various applications requiring high-energy ion beams, such as:

Particle Therapy: Potentially offering a more compact and tunable source of protons for cancer treatment compared to traditional accelerators.
Fast Ignition: A concept for inertial confinement fusion where high-energy ions could be used to ignite a thermonuclear reaction within a compressed fuel target.
Material Science: Studying material properties under extreme conditions achievable with high-energy ion beams.
Overall, Breakout Afterburner (BOA) is a promising technique for laser-driven ion acceleration with the potential to achieve higher energy gains and more control over the ion beam characteristics. However, further research is needed to overcome the experimental challenges and optimize the BOA process for various applications.</rdfs:comment>
    </owl:Class>
    


    <!-- http://www.semanticweb.org/afshar87/ontologies/2024/3/Laser-Plasma_ontology#Equation_of_State_(EOS) -->

    <owl:Class rdf:about="http://www.semanticweb.org/afshar87/ontologies/2024/3/Laser-Plasma_ontology#Equation_of_State_(EOS)">
        <rdfs:subClassOf rdf:resource="http://www.semanticweb.org/afshar87/ontologies/2024/3/Laser-Plasma_ontology#High_Energy_Density_Physics_(HEDP)"/>
        <rdfs:comment>Measurements and theoretical calculations of the pressure, density, and temperature relationship in HED matter.</rdfs:comment>
    </owl:Class>
    


    <!-- http://www.semanticweb.org/afshar87/ontologies/2024/3/Laser-Plasma_ontology#High_Energy_Density_Physics_(HEDP) -->

    <owl:Class rdf:about="http://www.semanticweb.org/afshar87/ontologies/2024/3/Laser-Plasma_ontology#High_Energy_Density_Physics_(HEDP)">
        <rdfs:subClassOf rdf:resource="http://www.semanticweb.org/afshar87/ontologies/2024/3/Laser-Plasma_ontology#Laser_Plasma_Application"/>
        <rdfs:comment>High-energy-density physics (HED physics) deals with matter under extreme conditions of pressure and temperature, often created by lasers or other high-energy sources.</rdfs:comment>
    </owl:Class>
    


    <!-- http://www.semanticweb.org/afshar87/ontologies/2024/3/Laser-Plasma_ontology#Inertial_Confinement_Fusion_(ICF) -->

    <owl:Class rdf:about="http://www.semanticweb.org/afshar87/ontologies/2024/3/Laser-Plasma_ontology#Inertial_Confinement_Fusion_(ICF)">
        <rdfs:subClassOf rdf:resource="http://www.semanticweb.org/afshar87/ontologies/2024/3/Laser-Plasma_ontology#Laser_Plasma_Application"/>
        <rdfs:comment>Plasmas created by imploding a target with high-power lasers or particle beams to achieve conditions necessary for fusion reactions.</rdfs:comment>
    </owl:Class>
    


    <!-- http://www.semanticweb.org/afshar87/ontologies/2024/3/Laser-Plasma_ontology#LWFA_(Laser_Wakefield_Acceleration) -->

    <owl:Class rdf:about="http://www.semanticweb.org/afshar87/ontologies/2024/3/Laser-Plasma_ontology#LWFA_(Laser_Wakefield_Acceleration)">
        <rdfs:subClassOf rdf:resource="http://www.semanticweb.org/afshar87/ontologies/2024/3/Laser-Plasma_ontology#Laser_Electron_Acceleration"/>
        <owl:disjointWith rdf:resource="http://www.semanticweb.org/afshar87/ontologies/2024/3/Laser-Plasma_ontology#PWFA_(Plasma_Wakefield_Acceleration)"/>
        <rdfs:comment>In Laser Wakefield Acceleration (LWFA), different injection mechanisms are used to introduce electrons into the accelerating wakefield. The primary types of injection mechanisms include Ionization Injection, Shock-Front Injection, Self-Injection, and Trojan Horse Injection. Each mechanism has its unique process, advantages, and disadvantages.

### 1. Ionization Injection
**Process**: Ionization injection involves ionizing a high-Z gas (e.g., nitrogen or argon) within the wakefield created by the laser pulse. This releases electrons at precise locations and times, allowing them to be captured by the wakefield for acceleration.

**Advantages**:
- **Precision**: Allows for precise control over electron injection.
- **Beam Quality**: Produces high-quality beams with narrow energy spread and low emittance.

**Disadvantages**:
- **Complexity**: Requires careful tuning of laser parameters and gas composition.
- **High Laser Intensity**: Requires high-intensity lasers to ionize the gas.

**Illustration**:
```
Laser Pulse --&gt; High-Z Gas Ionization --&gt; Electron Injection --&gt; Acceleration in Wakefield
```

### 2. Shock-Front Injection
**Process**: A density shock (sharp density gradient) is created in the plasma, usually by a laser-induced shock wave. When the laser pulse encounters this shock, the abrupt change in plasma density enhances electron trapping and injection into the wakefield.

**Advantages**:
- **Controlled Injection**: Shock-front injection allows for localized and controlled injection.
- **Flexibility**: Can be used with various plasma densities and laser parameters.

**Disadvantages**:
- **Setup Complexity**: Requires precise creation and timing of the shock front.
- **Synchronization**: Needs accurate synchronization between the laser pulse and the shock front.

**Illustration**:
```
Laser Pulse --&gt; Density Shock --&gt; Electron Trapping --&gt; Acceleration in Wakefield
```

### 3. Self-Injection
**Process**: In self-injection, the wakefield amplitude becomes large enough to trap electrons from the surrounding plasma. This usually occurs when the laser intensity and plasma density reach a threshold where wave-breaking or self-trapping conditions are met.

**Advantages**:
- **Simplicity**: Simplest setup with no need for additional ionization stages or shock creation.
- **Cost-Effective**: Generally requires fewer resources and simpler equipment.

**Disadvantages**:
- **Less Control**: Less control over the injection process, leading to broader energy spreads.
- **Beam Quality**: The quality of the electron beam is generally lower than with controlled injection methods.

**Illustration**:
```
Laser Pulse --&gt; High Wakefield Amplitude --&gt; Wave-Breaking --&gt; Electron Injection
```

### 4. Trojan Horse Injection
**Process**: Trojan Horse Injection involves using a secondary laser pulse to ionize inner-shell electrons of a gas (like helium) within the wakefield of the primary laser pulse. The secondary laser precisely controls the timing and location of electron release.

**Advantages**:
- **Precision Control**: Highly precise injection control.
- **High Beam Quality**: Can produce beams with very low emittance and high brightness.

**Disadvantages**:
- **Complex Setup**: Requires two synchronized laser pulses.
- **Advanced Equipment**: Needs sophisticated equipment for synchronization and control.

**Illustration**:
```
Primary Laser Pulse --&gt; Wakefield Creation --&gt; Secondary Laser Ionization --&gt; Electron Injection
```

### Comparative Summary

| Feature                           |             Ionization Injection                     |          Shock-Front Injection        |             Self-Injection             |      Trojan Horse Injection           |
|------------------------------- |-------------------------------------------------- |------------------------------------------|-------------------------------------|-------------------------------------------|
| **Control**                          | High                                                              | High                                                     | Low                                                    | Very High                            |
| **Beam Quality**               | High (low emittance, narrow spread)    | High (localized injection)                 | Moderate (broad spread)               | Very High (low emittance, high brightness) |
| **Complexity**                   | High                                                              | Moderate to High                               | Low                                                    | Very High                            |
| **Laser Requirements** | High-intensity laser                                   | Precise synchronization                   | Threshold intensity                         | Two synchronized lasers              |
| **Typical Use**                 | High-precision experiments                     | Controlled injection scenarios       | Simpler, cost-effective setups      | Advanced research requiring precise beams |
 
 
Below is a conceptual illustration of the different injection mechanisms. While I can&apos;t provide actual plots here, this diagram summarizes the processes:

```
 Ionization Injection
 --------------------
 Laser Pulse ----&gt; High-Z Gas Ionization ---&gt; Electron Injection ----&gt; Acceleration in Wakefield
 
 Shock-Front Injection
 ---------------------
 Laser Pulse ----&gt; Density Shock (Sharp Gradient) ---&gt; Electron Trapping ----&gt; Acceleration in Wakefield
 
 Self-Injection
 --------------
 Laser Pulse ----&gt; High Wakefield Amplitude (Wave-Breaking) ---&gt; Electron Injection
 
 Trojan Horse Injection
 ----------------------
 Primary Laser Pulse ----&gt; Wakefield Creation ---&gt; Secondary Laser Pulse (Inner-Shell Ionization) ---&gt; Electron Injection
```

Each mechanism has its specific conditions and requirements, making them suitable for different experimental setups and research goals in laser wakefield acceleration.</rdfs:comment>
    </owl:Class>
    


    <!-- http://www.semanticweb.org/afshar87/ontologies/2024/3/Laser-Plasma_ontology#Laser_Channeling_Acceleration_(LCA) -->

    <owl:Class rdf:about="http://www.semanticweb.org/afshar87/ontologies/2024/3/Laser-Plasma_ontology#Laser_Channeling_Acceleration_(LCA)">
        <rdfs:subClassOf rdf:resource="http://www.semanticweb.org/afshar87/ontologies/2024/3/Laser-Plasma_ontology#Laser_Ion_acceleration"/>
        <rdfs:comment>An intense laser pulse can create a channel in a pre-formed plasma through which the laser light propagates.
The strong electric fields within the channel can accelerate ions to high energies.
LCA is a promising approach for achieving high-quality ion beams.</rdfs:comment>
    </owl:Class>
    


    <!-- http://www.semanticweb.org/afshar87/ontologies/2024/3/Laser-Plasma_ontology#Magnetic_Reconnection_Acceleration_(MRA) -->

    <owl:Class rdf:about="http://www.semanticweb.org/afshar87/ontologies/2024/3/Laser-Plasma_ontology#Magnetic_Reconnection_Acceleration_(MRA)">
        <rdfs:subClassOf rdf:resource="http://www.semanticweb.org/afshar87/ontologies/2024/3/Laser-Plasma_ontology#Laser_Ion_acceleration"/>
        <rdfs:comment>This mechanism involves the reconnection of magnetic field lines within the laser-produced plasma.
The reconnection process can accelerate ions to high energies.
MRA is an area of ongoing research with potential for future applications.</rdfs:comment>
    </owl:Class>
    


    <!-- http://www.semanticweb.org/afshar87/ontologies/2024/3/Laser-Plasma_ontology#PWFA_(Plasma_Wakefield_Acceleration) -->

    <owl:Class rdf:about="http://www.semanticweb.org/afshar87/ontologies/2024/3/Laser-Plasma_ontology#PWFA_(Plasma_Wakefield_Acceleration)">
        <rdfs:subClassOf rdf:resource="http://www.semanticweb.org/afshar87/ontologies/2024/3/Laser-Plasma_ontology#Laser_Electron_Acceleration"/>
        <rdfs:comment>Plasma Wakefield Acceleration (PWFA) is a technique used to accelerate charged particles, such as electrons or positrons, using the electric fields generated in a plasma wake. This method leverages the interaction between a high-energy particle beam (often referred to as the drive beam) and a plasma to create strong accelerating fields.

Process
Drive Beam Introduction:

A high-energy particle beam, typically consisting of electrons or protons, is injected into a plasma. This beam is known as the drive beam.
Wakefield Generation:

As the drive beam travels through the plasma, it displaces plasma electrons due to its strong electric fields, creating a region of positive charge (the wake).
The displaced electrons then oscillate back toward the positive region, forming a series of electric fields, or wakefields, that trail behind the drive beam.
Trailing Beam Injection:

A second particle beam, known as the witness or trailing beam, is injected into the accelerating phase of the wakefield generated by the drive beam.
This witness beam is accelerated by the strong electric fields in the wake.
Key Characteristics
High Gradient Fields:
PWFA can produce extremely high gradient accelerating fields, often several orders of magnitude higher than conventional radio-frequency accelerators.
Efficiency:
The method is highly efficient because the energy transfer from the drive beam to the wakefield, and subsequently to the trailing beam, is direct and rapid.
Versatility:
Can be used with different types of drive beams (electrons, protons) and is adaptable to various plasma densities and configurations.
Advantages
High Acceleration Gradients:
Capable of generating accelerating fields in the range of gigavolts per meter (GV/m), significantly higher than traditional accelerators.
Cost-Effective:
Reduces the need for long accelerator structures, potentially lowering costs for large-scale accelerator facilities.
Scalability:
Can be scaled to different lengths and plasma densities to suit various experimental and practical needs.
Disadvantages
Complexity:
The interaction between the drive beam and plasma requires precise control and understanding of plasma dynamics.
Beam Quality:
Maintaining high beam quality (low emittance, narrow energy spread) can be challenging due to instabilities and other effects within the plasma.</rdfs:comment>
    </owl:Class>
    


    <!-- http://www.semanticweb.org/afshar87/ontologies/2024/3/Laser-Plasma_ontology#Radiation_Pressure_Acceleration_(RPA) -->

    <owl:Class rdf:about="http://www.semanticweb.org/afshar87/ontologies/2024/3/Laser-Plasma_ontology#Radiation_Pressure_Acceleration_(RPA)">
        <rdfs:subClassOf rdf:resource="http://www.semanticweb.org/afshar87/ontologies/2024/3/Laser-Plasma_ontology#Laser_Ion_acceleration"/>
        <rdfs:comment>Radiation Pressure Acceleration (RPA) is another technique used in laser-driven ion acceleration to achieve high-speed ion beams. Here&apos;s a detailed explanation of RPA:

Principle:

RPA relies on the transfer of momentum from the laser pulse to ions in the target material through the concept of radiation pressure. Imagine the laser light as a stream of photons (particles of light). When these photons collide with the target, they transfer some of their momentum to the ions within the material. This momentum transfer pushes the ions forward, accelerating them to high velocities.

Key Points of RPA:

Target: RPA typically utilizes ultra-thin targets, often just a few nanometers thick. This allows the laser pulse to penetrate the target more effectively and interact with a larger portion of the ions.
Circularly Polarized Laser: RPA benefits from using a circularly polarized laser pulse. This type of laser creates a rotating electric field that interacts with the ions and enhances their acceleration compared to a linearly polarized pulse.
Light Sail Effect: The process is sometimes referred to as the &quot;light sail effect&quot; because the ions behave like a miniature sail pushed forward by the momentum of the photons in the laser light.
Advantages of RPA:

High Efficiency: RPA offers a potentially highly efficient method for laser-driven ion acceleration. A significant portion of the laser energy can be transferred to the ions, resulting in energetic beams.
Monoenergetic Beams: Similar to BOA, RPA has the potential to produce more monoenergetic ion beams, which can be advantageous for specific applications requiring a well-defined ion energy distribution.
Challenges of RPA:

Target Fabrication: Creating and handling ultra-thin targets with precise thicknesses can be challenging and requires specialized techniques.
Laser Requirements: RPA works best with high-contrast laser pulses, meaning a clear separation between the pre-pulse and the main high-intensity pulse. Achieving this contrast is crucial for efficient acceleration.
Target Expansion: During the interaction, the target can begin to expand due to the laser heating. This expansion can limit the effectiveness of RPA as the laser light becomes less efficient in pushing the ions.
Comparison with BOA:

While both BOA and RPA aim for high-energy ion beams, they achieve it through different mechanisms:

BOA: Relies on relativistically induced transparency to create a stronger electric field for acceleration within the target.
RPA: Focuses on directly transferring momentum from the laser light to the ions via radiation pressure.
Applications of RPA:

RPA research holds promise for similar applications as BOA, including:

Particle Therapy: Potentially offering a compact and tunable source of protons for cancer treatment.
Fast Ignition: Providing a method for high-energy ion beam generation for potential use in inertial confinement fusion.
Material Science: Studying material behavior under extreme conditions created by high-energy ion beams.</rdfs:comment>
    </owl:Class>
    


    <!-- http://www.semanticweb.org/afshar87/ontologies/2024/3/Laser-Plasma_ontology#Target_Normal_Sheath_Acceleration_(TNSA) -->

    <owl:Class rdf:about="http://www.semanticweb.org/afshar87/ontologies/2024/3/Laser-Plasma_ontology#Target_Normal_Sheath_Acceleration_(TNSA)">
        <rdfs:subClassOf rdf:resource="http://www.semanticweb.org/afshar87/ontologies/2024/3/Laser-Plasma_ontology#Laser_Ion_acceleration"/>
        <rdfs:comment>Target Normal Sheath Acceleration, is one of the most common and well-studied mechanisms for laser-driven ion acceleration. Here&apos;s a breakdown of the key concepts:

Principle:

Laser-Target Interaction: A high-intensity laser pulse strikes a target material.
Plasma Formation: The intense laser light ionizes the target atoms, stripping away electrons and creating a hot, ionized gas called plasma.
Electric Field Generation: As the electrons are rapidly ejected from the target due to the laser pulse, a strong electric field is generated at the front surface of the plasma, pointing inwards towards the target. This region is called the Target Normal Sheath.
Ion Acceleration: Ions within the target material, particularly protons (hydrogen nuclei) and heavier ions depending on the target composition, are pulled by this electric field. This pulls them away from the target and accelerates them to high velocities in a direction normal (perpendicular) to the target surface, hence the name &quot;Target Normal Sheath Acceleration.&quot;
Characteristics of TNSA:

Broad Energy Distribution: TNSA typically produces ion beams with a broad distribution of energies. This means ions within the beam have a range of velocities, unlike some other acceleration techniques that can achieve more monoenergetic beams.
Scalability: TNSA can be achieved with a wider range of laser parameters and target materials compared to some other techniques. This makes it a more versatile approach.
Advantages of TNSA:

Simple Setup: TNSA requires a relatively simpler experimental setup compared to other laser-driven ion acceleration methods.
High Brightness: TNSA can generate ion beams with a high number of ions per unit time and solid angle, making them &quot;bright&quot; sources. This can be beneficial for certain applications.
Challenges of TNSA:

Limited Energy: Compared to newer techniques like BOA and RPA, TNSA generally achieves lower maximum ion energies.
Beam Quality: The broad energy distribution of TNSA beams can be a drawback for applications requiring a well-defined ion energy. Additional techniques might be needed to improve the beam quality.
Applications of TNSA:

Despite the limitations, TNSA remains a valuable tool due to its simplicity and scalability. Here are some potential applications:

Ion Beam Diagnostics: Utilizing TNSA-generated ion beams to study material properties and diagnose plasma behavior in other experiments.
Material Processing: TNSA beams can be used for surface modification, micromachining, and other material processing applications.
Development of New Acceleration Techniques: Studying TNSA processes can provide valuable insights for the development of more advanced laser-driven ion acceleration methods.</rdfs:comment>
    </owl:Class>
    


    <!-- http://www.semanticweb.org/afshar87/ontologies/2024/3/Laser-Plasma_ontology#Warm_Dense_Matter_(WDM) -->

    <owl:Class rdf:about="http://www.semanticweb.org/afshar87/ontologies/2024/3/Laser-Plasma_ontology#Warm_Dense_Matter_(WDM)">
        <rdfs:subClassOf rdf:resource="http://www.semanticweb.org/afshar87/ontologies/2024/3/Laser-Plasma_ontology#Laser_Plasma_Application"/>
        <rdfs:comment>Warm dense matter (WDM) is a state of matter where electrons are partially ionized but remain bound to their atoms, and the ions are close together but not completely ordered like a solid.

Warm dense matter (WDM) plays a crucial role in understanding the dynamics of laser-plasma interactions. It represents a specific state of matter that arises when a laser interacts with a target material. Here&apos;s a breakdown of WDM in this context:

Characteristics of WDM:

Partially Ionized: Atoms in WDM lose some electrons due to the intense laser field, but they aren&apos;t fully stripped like in a high-temperature plasma.
High Density: The material remains relatively dense, comparable to its solid state, unlike the low-density plasmas typically created at high laser intensities.
Intermediate Temperature: Electrons in WDM have temperatures ranging from a few electron volts (eV) to tens of eV, higher than a solid but not reaching the extreme temperatures of high-energy-density plasmas.
Unique Properties: The combination of partial ionization and high density leads to unique electrical, thermal, and optical properties not found in solids or high-temperature plasmas.
Creation of WDM in Laser Plasmas:

When a laser pulse interacts with a solid target, the initial interaction can involve various mechanisms like multiphoton ionization and tunnel ionization, leading to the ejection of electrons.
However, the remaining ions are still close together due to the high density of the material.
As the laser energy is absorbed, the remaining electrons and ions in the target get heated, pushing the material towards the WDM state.
Importance of WDM in Laser Plasma Interactions:

Understanding WDM is crucial for accurately modeling the behavior of laser-produced plasmas, particularly in regimes where complete ionization isn&apos;t achieved.
The properties of WDM can significantly affect the propagation and absorption of the laser pulse within the target material.
WDM plays a role in various laser-plasma applications, including:
Laser Ablation: The removal of material from a target surface by laser irradiation. The dynamics of ablation and the properties of the ejected material are influenced by WDM.
Laser-Driven Shocks: The generation of shock waves in a target by a laser pulse can create WDM regions behind the shock front.
X-ray Generation: The emission of X-rays from laser-plasma interactions can be influenced by the electronic structure of WDM.
Challenges of Studying WDM:

Due to its short-lived nature and complex properties, studying WDM in laser-plasma interactions presents challenges.
Advanced diagnostic techniques, such as time-resolved X-ray spectroscopy and ultrafast electron beams, are required to probe the properties of WDM on its short timescales.
Theoretical models also need to be developed to accurately describe the behavior of WDM under these extreme conditions.</rdfs:comment>
    </owl:Class>
    


    <!-- 
    ///////////////////////////////////////////////////////////////////////////////////////
    //
    // Individuals
    //
    ///////////////////////////////////////////////////////////////////////////////////////
     -->

    


    <!-- http://www.semanticweb.org/afshar87/ontologies/2024/3/Laser-Plasma_ontology#absorbing_silver_mueller -->

    <owl:NamedIndividual rdf:about="http://www.semanticweb.org/afshar87/ontologies/2024/3/Laser-Plasma_ontology#absorbing_silver_mueller">
        <rdf:type rdf:resource="http://www.semanticweb.org/afshar87/ontologies/2024/3/Laser-Plasma_ontology#BoundaryConditionType"/>
    </owl:NamedIndividual>
    


    <!-- http://www.semanticweb.org/afshar87/ontologies/2024/3/Laser-Plasma_ontology#dirichlet -->

    <owl:NamedIndividual rdf:about="http://www.semanticweb.org/afshar87/ontologies/2024/3/Laser-Plasma_ontology#dirichlet">
        <rdf:type rdf:resource="http://www.semanticweb.org/afshar87/ontologies/2024/3/Laser-Plasma_ontology#BoundaryConditionType"/>
        <Laser-Plasma_ontology:simulation_bc_xmax></Laser-Plasma_ontology:simulation_bc_xmax>
        <Laser-Plasma_ontology:simulation_bc_xmin></Laser-Plasma_ontology:simulation_bc_xmin>
        <Laser-Plasma_ontology:simulation_bc_ymax></Laser-Plasma_ontology:simulation_bc_ymax>
        <Laser-Plasma_ontology:simulation_bc_ymin></Laser-Plasma_ontology:simulation_bc_ymin>
        <Laser-Plasma_ontology:simulation_bc_zmax></Laser-Plasma_ontology:simulation_bc_zmax>
        <Laser-Plasma_ontology:simulation_bc_zmin></Laser-Plasma_ontology:simulation_bc_zmin>
    </owl:NamedIndividual>
    


    <!-- http://www.semanticweb.org/afshar87/ontologies/2024/3/Laser-Plasma_ontology#open -->

    <owl:NamedIndividual rdf:about="http://www.semanticweb.org/afshar87/ontologies/2024/3/Laser-Plasma_ontology#open">
        <rdf:type rdf:resource="http://www.semanticweb.org/afshar87/ontologies/2024/3/Laser-Plasma_ontology#BoundaryConditionType"/>
        <Laser-Plasma_ontology:simulation_bc_xmax></Laser-Plasma_ontology:simulation_bc_xmax>
        <Laser-Plasma_ontology:simulation_bc_xmin></Laser-Plasma_ontology:simulation_bc_xmin>
        <Laser-Plasma_ontology:simulation_bc_ymax></Laser-Plasma_ontology:simulation_bc_ymax>
        <Laser-Plasma_ontology:simulation_bc_ymin></Laser-Plasma_ontology:simulation_bc_ymin>
        <Laser-Plasma_ontology:simulation_bc_zmax></Laser-Plasma_ontology:simulation_bc_zmax>
        <Laser-Plasma_ontology:simulation_bc_zmin></Laser-Plasma_ontology:simulation_bc_zmin>
    </owl:NamedIndividual>
    


    <!-- 
    ///////////////////////////////////////////////////////////////////////////////////////
    //
    // Annotations
    //
    ///////////////////////////////////////////////////////////////////////////////////////
     -->

    <rdf:Description rdf:about="http://www.semanticweb.org/afshar87/ontologies/2024/3/Laser-Plasma_ontology#Simulation">
        <rdfs:comment>The &quot;Simulation&quot; class encompasses all computational and numerical methods used to model and analyze phenomena in laser-plasma interactions, including but not limited to laser ion acceleration, electron acceleration, and various plasma behaviors under different conditions. This class includes attributes describing the parameters, methodologies, and outcomes of simulations.</rdfs:comment>
    </rdf:Description>
    <rdf:Description rdf:about="http://www.semanticweb.org/afshar87/ontologies/2024/3/Laser-Plasma_ontology#liquid">
        <rdfs:comment>Liquid targets are indeed an emerging area of research in laser-plasma interaction for particle acceleration. Here&apos;s a breakdown of their potential and considerations:

Advantages of Liquid Targets:

Replenishment: Unlike solid targets that get damaged after each laser shot, liquid targets offer the advantage of being continuously replenished. This allows for high repetition rate experiments, crucial for some applications.
Uniformity: Liquids can provide a more uniform and clean target compared to solid targets, which can have imperfections or surface irregularities. This uniformity can lead to more consistent laser-plasma interaction and potentially improve beam quality.
Tailorable Properties: The properties of the liquid target can be tailored by using different liquids or mixtures. This allows researchers to potentially optimize the target for specific acceleration mechanisms (e.g., TNSA, RPA) or particle species (protons, ions).
 
Types of Liquid Targets:

Liquid Jets: These involve a thin stream of liquid focused by a nozzle. The jet can be intersected by the laser pulse for particle acceleration. Research is focused on:
Jet stability and control: Maintaining a stable and uniform jet is crucial for reproducible results.
Liquid selection: Different liquids (e.g., water, ethanol) offer varying properties for laser-plasma interaction.
Liquid Films: These consist of a thin layer of liquid formed on a substrate or created by the collision of two liquid jets. They offer similar advantages to liquid jets but with potentially better control over film thickness.

Challenges of Liquid Targets:

Target Delivery System: Designing a reliable system for delivering and replenishing the liquid target within the vacuum chamber of a laser system can be complex.
Hydrodynamic Effects: The liquid&apos;s motion due to the laser pulse or jet flow could introduce instabilities that affect the laser-plasma interaction. Research is ongoing to minimize these effects.
Target Contamination: Maintaining a clean and contaminant-free liquid is important for consistent results.
Overall:

Liquid targets hold promise for advancing laser-driven particle acceleration, particularly for high repetition rate applications. While challenges exist, ongoing research is addressing these issues to improve the reliability and effectiveness of liquid targets in this field.

Incorporating liquid targets as a subclass within your LaserPlasmaOntology can enhance its comprehensiveness and reflect the latest developments in particle acceleration techniques. Remember to link them appropriately to the relevant particle acceleration processes (e.g., TNSATherapy with LiquidJetTarget).</rdfs:comment>
    </rdf:Description>
    


    <!-- 
    ///////////////////////////////////////////////////////////////////////////////////////
    //
    // General axioms
    //
    ///////////////////////////////////////////////////////////////////////////////////////
     -->

    <rdf:Description>
        <rdf:type rdf:resource="http://www.w3.org/2002/07/owl#AllDisjointClasses"/>
        <owl:members rdf:parseType="Collection">
            <rdf:Description rdf:about="http://www.semanticweb.org/afshar87/ontologies/2024/3/Laser-Plasma_ontology#Particle_spectroscopy"/>
            <rdf:Description rdf:about="http://www.semanticweb.org/afshar87/ontologies/2024/3/Laser-Plasma_ontology#Thomson_scattering"/>
            <rdf:Description rdf:about="http://www.semanticweb.org/afshar87/ontologies/2024/3/Laser-Plasma_ontology#X-ray_radiography"/>
        </owl:members>
    </rdf:Description>
    <rdf:Description>
        <rdf:type rdf:resource="http://www.w3.org/2002/07/owl#AllDisjointClasses"/>
        <owl:members rdf:parseType="Collection">
            <rdf:Description rdf:about="http://www.semanticweb.org/afshar87/ontologies/2024/3/Laser-Plasma_ontology#electron"/>
            <rdf:Description rdf:about="http://www.semanticweb.org/afshar87/ontologies/2024/3/Laser-Plasma_ontology#ion"/>
            <rdf:Description rdf:about="http://www.semanticweb.org/afshar87/ontologies/2024/3/Laser-Plasma_ontology#proton"/>
        </owl:members>
    </rdf:Description>
    <rdf:Description>
        <rdf:type rdf:resource="http://www.w3.org/2002/07/owl#AllDisjointClasses"/>
        <owl:members rdf:parseType="Collection">
            <rdf:Description rdf:about="http://www.semanticweb.org/afshar87/ontologies/2024/3/Laser-Plasma_ontology#gas__target"/>
            <rdf:Description rdf:about="http://www.semanticweb.org/afshar87/ontologies/2024/3/Laser-Plasma_ontology#liquid_target"/>
            <rdf:Description rdf:about="http://www.semanticweb.org/afshar87/ontologies/2024/3/Laser-Plasma_ontology#solid__target"/>
        </owl:members>
    </rdf:Description>
</rdf:RDF>



<!-- Generated by the OWL API (version 4.5.29.2024-05-13T12:11:03Z) https://github.com/owlcs/owlapi -->

